@prefix mod: <https://w3id.org/mod#> .
@prefix cc: <http://creativecommons.org/ns#> .
@prefix sd: <http://www.w3.org/ns/sparql-service-description#> .
@prefix dcterms: <http://purl.org/dc/terms/> .
@prefix omv: <http://omv.ontoware.org/2005/05/ontology#> .
@prefix owl: <http://www.w3.org/2002/07/owl#> .
@prefix pav: <http://purl.org/pav/> .
@prefix rdf: <http://www.w3.org/1999/02/22-rdf-syntax-ns#> .
@prefix xml: <http://www.w3.org/XML/1998/namespace/> .
@prefix xsd: <http://www.w3.org/2001/XMLSchema#> .
@prefix adms: <http://www.w3.org/ns/adms#> .
@prefix dcat: <http://www.w3.org/ns/dca#> .
@prefix dcmi: <http://purl.org/dc/dcmitype/> .
@prefix doap: <http://usefulinc.com/ns/doap#> .
@prefix foaf: <http://xmlns.com/foaf/0.1/> .
@prefix idot: <http://identifiers.org/idot/> .
@prefix nkos: <http://w3id.org/nkos#> .
@prefix odrl: <http://www.w3.org/ns/odrl/2/> .
@prefix prov: <http://www.w3.org/ns/prov#> .
@prefix rdfs: <http://www.w3.org/2000/01/rdf-schema#> .
@prefix sioc: <http://rdfs.org/sioc/> .
@prefix skos: <http://www.w3.org/2004/02/skos/core#> .
@prefix vann: <https://vocab.org/vann/> .
@prefix void: <http://rdfs.org/ns/void#> .
@prefix frbr: <http://purl.org/vocab/frbr/core#> .
@prefix schema: <https://schema.org/> .
@prefix oboinowl: <http://www.geneontology.org/formats/oboInOwl#> .
@base <https://w3id.org/mod> .

<https://w3id.org/mod> rdf:type owl:Ontology ;
                        owl:versionIRI <https://w3id.org/mod/2.0> ;

#################################################################
#    MOD2.0 description with MOD2 properties
#################################################################

# This section is a description of MOD using each of the MOD2.0 properties. 
# Properties are sorted and grouped as in GSheet working document.
# Texttual descriptions are available in English and French. 
# Properties from MOD2 thata re not used to described MOD2 are commented.

  ########## Intrinsic properties ##########
    mod:acronym                     "MOD" ;
    dcterms:title                   "MOD: Metadata for Ontology Description and publication"@en,
                                    "MOD: Metadonnées pour la Description et la publication d'Ontologies"@fr ;
    dcterms:alternative             "MOD Vocabulary"@en ,
                                    "Vocabulaire MOD"@fr ,
                                    "MOD Ontology Metadata model"@en ,
                                    "Modèle de métadonnées d'ontologie MOD"@fr ;
    skos:hiddenLabel                "MOD-Ontology"@en;
    owl:ontologyIRI                 <https://w3id.org/mod> ;
    owl:versionIRI                  <https://w3id.org/mod/2.0> ;
##  dcterms:identifier              ;
    owl:versionInfo                 "2.0.1" ;
    mod:status                      "alpha" ;
    owl:deprecated                  false ;
    dcterms:license                 <https://creativecommons.org/licenses/by/4.0> ; 
    mod:hasRepresentationLanguage   omv:OWL ;
    mod:hasFormalityLevel           omv:Vocabulary ;
    mod:hasSyntax                   <http://www.w3.org/ns/formats/Turtle> ;
    dcterms:language                <http://lexvo.org/id/iso639-3/eng> ,
                                    <http://lexvo.org/id/iso639-3/fra> ;

  ########## Description properties ##########
    dcterms:description        
                    "MOD (Metadata for Ontology Description and publication) is a project to define a standard way to capture metadata descriptions for ontologies or semantic resources/artefacts in general (thesaurus, terminologies, vocabularies, etc.). The MOD OWL file can be used to create knowledge bases consisting of metadata records of ontologies/vocabularies as instances. The MOD vocabulary can also be used to define specific profiles for recommended metadata properties (e.g., H2020 project FAIRsFAIR semantic artefact minimum metadata profile). Users can go through MOD and pickup the required properties to describe their ontology."@en, 
                    "MOD (Metadonnées pour la Description et la publication d'Ontologie) est un projet visant à définir un moyen standard pour capturer des descriptions de métadonnées pour les ontologies ou les ressources/artefacts sémantiques en général (thésaurus, terminologies, vocabulaires, etc.). Le fichier MOD OWL peut être utilisé pour créer des bases de connaissances composées d’instances d’ontologies / vocabulaires décrites avec MOD. Le vocabulaire MOD peut également être utilisé pour définir des profils de métadonnées (e.g., le profil de métadonnées minimale pour les artefacts sémanttique du projet H2020 FAIRsFAIR). Les utilisateurs peuvent consulter la spécification et récupérer les propriétés requises pour décrire leur ontologie."@fr ;
    dcterms:abstract
                    "MOD provides a set of properties which can be used by ontology developers, ontology libraries (e.g., ontology registry, ontology repository, ontology portal), to describe and publish ontologies. The enriched description of ontologies, in turn, will help users to search, discover, identify and select ontologies."@en ,
                    "MOD fournit un ensemble de propriétés pouvant être utilisées par les développeurs d’ontologies ou les portails d’ontologies (registre, bibliothèques), pour décrire et publier des ontologies. La description enrichie des ontologies aidera les utilisateurs à rechercher, découvrir, identifier et sélectionner des ontologies."@fr ;
    cc:morePermissions              "https://github.com/sifrproject/MOD-Ontology/blob/master/LICENSE" ;
    cc:useGuidelines                "MOD is free of use; feedback is welcome."@en ,
                                    "MOD peut être utilisée de manière libre; les retours sont appréciés"@fr ;
    dcterms:bibliographicCitation   <https://dx.doi.org/10.1007/978-3-319-70863-8_17> ;
    foaf:page                       <https://www.isibang.ac.in/ns/mod/index.html> ;
    dcat:accessURL                  <https://www.isibang.ac.in/ns/mod/ontology.ttl> ;
    rdfs:comment            
                                    "This project is connected to the work done within AgroPortal (with MOD1.4). MOD 2.0 is work in progress."@en ,
                                    "Ce projet est lié au travail mis en œuvre dans AgroPortal (avec MOD1.4). MOD2.0 est en cours de développement."@fr ;
    omv:keywords                    "metadata description, metadata vocabularies, ontology description, ontology profile"@en ,
                                    "description de métadonnées, vocabulaires de métadonnées, description d'ontologie, profil d'ontologie"@fr ;
    dcterms:type                    omv:TaskOntology ;
    mod:designedForTask             omv:ConfigurationTask ;
    pav:createdWith                 <https://protege.stanford.edu> ;
    mod:usedEngineeringMethodology  
                                    "MOD 1 has been designed by reviewing in total 23 standard existing metadata vocabularies (e.g., Dublin Core, OMV, DCAT, VoID) and selecting relevant properties for describing ontologies. Then, we studied metadata usage analytics within ontologies and ontology repositories. MOD 2 abandon the integration approach of MOD 1 but re-incorporates properties of several obsolete metadata vocabularies inside its own namespace (DOOR, OMV, VOAF). MOD 2 is designed as an extension of the DCAT 2 metadata vocabulary."@en ,
                                    "MOD 1 a été conçue en examinant au total 23 vocabulaires de métadonnées standard existants (e.g., Dublin Core, OMV, DCAT, VoID) et en sélectionnant des propriétés pertinentes pour la description des ontologies. Nous avons ensuite étudié l’analyse de l’utilisation des métadonnées au sein d’ontologies et de portail d’ontologies. MOD 2 abandonne l'approche d'intégration de MOD 1 mais réincorpore les propriétés de plusieurs vocabulaires de métadonnées obsolètes dans son propre espace de nolmage (DOOR, OMV, VOAF). MOD 2 est conçue comme une extension du vocabulaire des métadonnées DCAT 2."@fr ;
    mod:conformsToKnowledgeRepresentationParadigm "OWL Ontology" ;
    dcterms:coverage    
                                    "Ontologies or semantic resources/artefacts in general (thesaurus, terminologies, vocabularies, etc.)"@en ,
                                    "Les ontologies ou les ressources/artefacts sémantiques en général (thésaurus, terminologies, vocabulaires, etc.)"@fr ;
    mod:competencyQuestion
                                    "How to standardly and semantically capture the description of an ontology while relying on other existing metadata vocabularies?"@en ,
                                    "Comment capturer de manière standard et sémantique la description d'une ontologie en s'appuyant sur d'autres vocabulaires de métadonnées existants?"@fr ;
    foaf:depiction                  <https://github.com/sifrproject/MOD-Ontology/raw/master/figures/MOD2.0_summary.png> ;
 ## foaf:logo                        ;
    foaf:homepage                   <https://github.com/sifrproject/MOD-Ontology> ;
    dcterms:accessRights        
                                    "MOD is licensed under the Creative Commons Attribution 4.0 ; For details, see here: https://github.com/sifrproject/MOD-Ontology/blob/master/LICENSE"@en ,
                                    "MOD est disponible sous Licence Creative Commons Attribution 4.0 ; pour plus de details voir https://github.com/sifrproject/MOD-Ontology/blob/master/LICENSE"@fr ;
    vann:changes                    
                                    "From MOD 1.2: (i) added description of properties, (ii) extended number of properties (from 88 to 128), (iii) separation of profile and ontology files, (iv) new URIs scheme. From MOD2.0: (i) use of w3id URIs, (ii) integration of DOOR, OMV, VOAF properties within MOD namespace, (iii) compliant with DCAT2."@en ,
                                    "Depuis MOD 1.2 : (i) ajout de la description des propriétés, (ii) nombre étendu de propriétés (de 88 à 128), (iii) séparation des fichiers de profil et d’ontologie, (iv) nouveaux URI. Depuis MOD2.O : (i) utilisation de w3id pour les URIs, (ii) intégration des propriétés de DOOR, OMV et VOAF dans l'espace de nommage de MOD, (iii) compatible avec DCAT2. "@fr ;
    vann:example                    
                                    "An adaptation of MOD1.4 is used within AgroPortal, since 2017. MOD2 is the baseline for H2020 project FAIRsFAIR semantic artefact minimum metadata profile."@en ,
                                    "Une adaptation de MOD est utilisée dans AgroPortal, depuis 2017. MOD2 est réutilisée par le profil de métadonnées minimale pour les artefacts sémanttique du projet H2020 FAIRsFAIR."@fr ;
    vann:preferredNamespaceUri      <https://w3id.org/mod> ;
    vann:preferredNamespacePrefix   "mod" ;
    mod:prefLabelProperty           rdfs:label ;
    mod:synonymProperty             skos:altLabel ;
    mod:definitionProperty          dcterms:description ;
    mod:authorProperty              pav:importedBy ;
    mod:obsoleteProperty            owl:deprecated ;
    mod:hierarchyProperty           rdfs:subClassOf ;
##  mod:obsoleteParent              ;
    void:uriRegexPattern            "OriginalURI | BaseURI+ShortName" ;
    mod:toDoList                   "https://github.com/sifrproject/MOD-Ontology/raw/master/mod-v2.0_todos.txt" ;
    idot:exampleIdentifier          <https://w3id.org/mod#analytics> ;
    schema:award                    "Published at MTSR 2017"@en ,
                                    "Publiée a MTSR 2017"@fr ;
    schema:associatedMedia          <https://drive.google.com/drive/folders/1kSF0XuSr9mwBk-daR6RYut_1Dzzko33v> ;
##  schema:includedInDataCatalog    ;

  ########## People properties ##########
  
    dcterms:creator                 "Biswanath Dutta (https://orcid.org/0000-0003-3059-8202)" ,
                                    "Clement Jonquet (https://orcid.org/0000-0002-2404-1582)" ; 
    dcterms:contributor             "Anne Toulet (https://orcid.org/0000-0003-0463-0854)" ,
                                    "Luiz Bonino (https://orcid.org/0000-0002-1164-1351)" ,
                                    "Yann Le Franc (https://orcid.org/0000-0003-4631-418X)" ,
                                    "Udaya Varadarajan (https://orcid.org/0000-0002-4936-0272)" ; 
    dcterms:publisher               "Indian Statistical Institute, Bangalore Centre, India (https://www.isibang.ac.in)" ,
                                    "LIRMM, University of Montpellier, France (http://www.lirmm.fr)" ;
    pav:curatedBy                   "Anne Toulet" ;
    schema:translator               "Clement Jonquet" ;
    dcterms:rightsHolder            "Indian Statistical Institute and University of Montpellier"@en ,
                                    "Institut Indien de la Statistique et Université de Montpellier"@fr;

  ########## Grouping properties ##########

    dcterms:subject                 "Metadata descriptions"@en ;
    mod:group                       "Metadata vocabularies"@en ;

  ########## Relation properties ##########

##  owl:imports                     ;  
    owl:priorVersion                <https://www.isibang.ac.in/ns/mod/1.4/> ,
                                    <https://www.isibang.ac.in/ns/mod/1.2/> ,
                                    <https://www.isibang.ac.in/ns/mod/1.1/> ,
                                    <https://www.isibang.ac.in/ns/mod/1.0/> ;
    owl:backwardCompatibleWith      <http://omv.ontoware.org/2005/05/ontology> ;
    owl:incompatibleWith            <http://kannel.open.ac.uk/ontology> ;
##  dcterms:isPartOf                ;
##  dcterms:hasPart                 ;  
##  dcterms:hasVersion              ;
##  dcterms:isFormatOf              ;
##  dcterms:hasFormat               ;
    dcterms:relation              
                                    "MOD uses or relates to each of these vocabularies: ADMS,CC,DCAT,DC,DCT,DOAP,DOOR,FOAF,IDOT,OBOINOWL,OMV,OWL,NKOS,PAV,PROV,RDFS,SCHEMA,SD,SKOS,VANN,VOAF,VOID."@en ,
                                    "MOD utilise ou se repose sur chacun des vocabulaires suivants : ADMS,CC,DCAT,DC,DCT,DOAP,DOOR,FOAF,IDOT,OBOINOWL,OMV,OWL,NKOS,PAV,PROV,RDFS,SCHEMA,SD,SKOS,VANN,VOAF,VOID."@fr ;
    mod:specializes                 <http://omv.ontoware.org/2005/05/ontology>;
##  schema:workTranslation          ;
##  schema:translationOfWork        ;
    mod:comesFromTheSameDomain      "OBOINOWL,OMV,OWL,NKOS,RDFS,SKOS,VANN,VOAF,VOID" ;
    mod:similar                     "OMV,VANN,VOAF,VOID" ;
    mod:hasEquivalencesWith      
                                    "MOD properties are 'reused' from properties in each these vocabularies: ADMS,CC,DCAT,DC,DCT,DOAP,FOAF,IDOT,OBOINOWL,OWL,NKOS,PAV,PROV,RDFS,SCHEMA,SD,SKOS,VANN,VOID. Reuses are formalized by a dcterms:relation. MOD2 redefines properties from DOOR, OMV, VOAF."@en ,  
                                    "Les propriétés de MOD sont 'importées' à partir des vocabulaires suivants : ADMS,CC,DCAT,DC,DCT,DOAP,FOAF,IDOT,OBOINOWL,OWL,NKOS,PAV,PROV,RDFS,SCHEMA,SD,SKOS,VANN,VOID. Les réutilisations soont formalisées par une propriété dcterms:relation. MOD2 re-définie les propriétés dans DOOR, OMV, VOAF."@fr ;
    mod:hasDisparateModelling  
                                    "DOAP (MOD reuses properties from both objects doap:Project and foaf:Document that are disjoincts.)"@en ,
                                    "DOAP (MOD réutilise des propriétés de des objets doap:Project et foaf:Document qui sont disjointes.)"@fr ;
##  mod:usedBy                      ;
    mod:generalizes                 "DOOR,OMV,VOAF"  ;
##  mod:hasDisjunctionsWith    ;

  ########## Content properties ##########

    foaf:primaryTopic       mod:Ontology ;
    void:rootResource       mod:Ontology ;
    mod:browsingUI          "https://www.isibang.ac.in/ns/mod/index.html" ;
##  sd:endpoint             ;
    mod:vocabularyUsed      <http://creativecommons.org/ns#> ,
                            <http://www.w3.org/ns/sparql-service-description#> ,
                            <http://purl.org/dc/terms/> ,
                            <http://omv.ontoware.org/2005/05/ontology#> ,
                            <http://www.w3.org/2002/07/owl#> ,
                            <http://purl.org/pav/> ,
                            <http://www.w3.org/1999/02/22-rdf-syntax-ns#> ,
                            <http://www.w3.org/XML/1998/namespace> ,
                            <http://www.w3.org/2001/XMLSchema#> ,
                            <http://usefulinc.com/ns/doap/> ,
                            <http://xmlns.com/foaf/0.1/> ,
                            <http://identifiers.org/idot/> ,
                            <http://www.w3.org/ns/prov#> ,
                            <http://www.w3.org/2000/01/rdf-schema#> ,
                            <http://www.w3.org/2004/02/skos/core#> ,
                            <http://purl.org/vocab/vann/> ,
                            <http://rdfs.org/ns/void#> ,
                            <https://schema.org/> ;
    mod:sampleQueries       
                            "For sample SPARQL queries to query MOD OWL knowledge base, see here: https://github.com/sifrproject/MOD-Ontology/blob/master/SPARQL_Queries_on_MOD_1.2.3-with-instances.txt"@en ,
                            "Pour des examples de requêtes SPARQL sur la base de connaissances MOD, voir ici : https://github.com/sifrproject/MOD-Ontology/blob/master/SPARQL_Queries_on_MOD_1.2.3-with-instances.txt"@fr ;
##  void:propertyPartition  ;
##  void:classPartition     ;
    void:dataDump           "https://www.isibang.ac.in/ns/mod/ontology.ttl" ,
                            "https://www.isibang.ac.in/ns/mod/ontology.json" ,
                            "https://www.isibang.ac.in/ns/mod/ontology.xml" ,
                            "https://www.isibang.ac.in/ns/mod/ontology.nt" ,
                            "https://www.isibang.ac.in/ns/mod/ontology.ttl" ;
##  void:openSearchDescription    ;
##  void:uriLookupEndpoint        ;

  ########## Community properties ##########

    mod:knownUsage          
                            "MOD is used for instance in AgroPortal (http://agroportal.lirmm.fr) to provide equivalences in AgroPortal's ontology metadata model. Other uses will be documented here in the future."@en ,
                            "MOD est utilisée par exemple dans AgroPortal (http://agroportal.lirmm.fr) pour fournir des equivalences au sein du modèle de métadonnées d'ontologies. D'autres usages seront documentés ici dans le futur."@fr ;
    mod:endorsedBy          "No organization is currenlty officially endorsing MOD."@en ,
                            "MOD n'est encore officiellement recommandée par aucune organization."@fr ;
    mod:usedInProject       "AgroPortal (http://agroportal.lirmm.fr)" ;
    dcterms:audience            
                            "MOD primary targets ontology (or semantic resource/artefact) developers and ontology library, repository or service providers."@en ,
                            "MOD s'adresse en priorité aux dévelopeurs d'ontologies (ou de ressource/artefact sémantiques) ainsi qu'au dévelopeurs de bibliothèque, de portail ou de service pour des ontologies."@fr ;
    foaf:fundedBy           
                            "Indian Statistical Institute, University of Montpellier, European French National Research Agency (under grant ANR-10-LABX-20, ANR-11-BINF-0002, ANR-19-DATA-0019), European Union’s Horizon 2020 research and innovation programme under the Marie Sklodowska-Curie grant agreement No 701771 and H2020 FAIRsFAIR project No 831558."@en ;
    doap:repository         <https://github.com/sifrproject/MOD-Ontology> ;
    doap:bugDatabase        <https://github.com/sifrproject/MOD-Ontology/issues> ;
##  doap:mailingList        ;
##  mod:hasEvaluation       ;
##  schema:comment          ;
##  mod:analytics           ;

  ########## Date properties ##########

    dcterms:created         "2021-12-01" ;
    dcterms:modified        "2022-02-14" ;
##  dcterms:valid           ;
##  pav:curatedOn           ;

  ########## Metrics properties ##########

##  mod:metrics                       ;
    mod:numberOfClasses               79 ;
    mod:numberOfIndividuals           7 ;
    mod:numberOfProperties            260 ;
    mod:numberOfObjectProperties      149 ;
    mod:numberOfDataProperties        111 ;
    mod:numberOfAxioms                1507 ;   
##  mod:numberOfLabels                ;
##  mod:byteSize                      ;
##  mod:maxDepth                      ;
##  mod:maxChildCount                 ;
##  mod:averageChildCount             ;
##  mod:classesWithOneChild           ;
##  mod:classesWithMoreThan25Children ; 
##  mod:classesWithNoDefinition       ;

  ########## Provenance properties ##########

    dcterms:source            
                            "MOD source is described in https://dx.doi.org/10.1007/978-3-319-70863-8_17 and https://doi.org/10.1007/s13740-018-0091-5"@en ,
                            "L'origine de MOD est décrite dans https://dx.doi.org/10.1007/978-3-319-70863-8_17 et https://doi.org/10.1007/s13740-018-0091-5"@fr ;
    prov:wasGeneratedBy     
                            "MOD is the result of a manual process of identifying, reviewing, and selecting candidate properties from standards metadata vocabularies if relevant to describe an ontology or any kind of semantic resource. When a property cannot be identified, it could be created in the MOD namespace. Since MCD2, it has been created as an extension of DCAT2."@en ,
                            "MOD est le résultat d'un processus manuel d'identification, de révision et de sélection des propriétés candidates à partir de vocabulaires de métadonnées standards, pour décrire une ontologie ou tout type de ressource sémantique. Lorsqu'une propriété ne peut pas être identifiée, elle peut être créée dans l'espace de noms MOD. Depuis MOD2, MOD est construote comme une extension de DCAT2"@fr ;
##  prov:wasInvalidatedBy   ;
    dcterms:accrualMethod       
                            "When a need of a new property is identified by the developer team, we review classic/standards metadata vocabularies to identifiy if the desire property already exists. If it exists in several metadata vocabularies we give priorities to consitency with previous MOD choices, then W3C Recommendations, then community standards."@en ,
                            "Lorsqu'un besoin d'une nouvelle propriété est identifié par l'équipe de développeurs, nous passons en revue les vocabulaires de métadonnées classiques / standards pour identifier si la propriété désirée existe déjà. Si elle existe dans plusieurs vocabulaires de métadonnées, nous donnons la priorité à la cohérence avec les choix précédents dans MOD, puis aux recommandations du W3C, puis aux normes de la communauté."@fr ;
    dcterms:accrualPeriodicity  
                            "New properties are added on demand with no specific periodicity."@en ,
                            "Les nouvelles propriétés sont ajoutées à la demande sans périodicité particulière."@fr ;
    dcterms:accrualPolicy       
                            "Editorial choice of the developer team."@en ,
                            "Choix éditorial de l'équipe de développeurs."@fr .


#################################################################
# Pattern to respect for each MOD properties
#################################################################
#
#### PropertyURI
#originalns:xx      rdf:type                rdf:Property ;
#                   rdfs:subPropertyOf      SUPER PROPERTY IF ANY
#                   rdfs:label              ""@en ,
#                                           ""@fr ;
#                   rdfs:domain             DOMAIN INFO IF ANY
#                   rdfs:range              RANGE INFO IF ANY
#                   dcterms:description     DESCCRIPTION FROM ORIGINAL SOURCE ;
#                   rdfs:isDefinedBy        URI OF ORIGINAL SOURCE ;
#                   dcterms:issued          "DATE OF THE FIRST CREATION OF THE PROPERTY BY ORIGINAL RESOURCE"^^xsd:date ;
#                   owl:equivalentProperty  EQUIVALENT PROPERTY (Equivalent properties have the same "values" (i.e., the same property extension))
#                   pav:derivedFrom         URI OF FIRST MOD VERSION INCLUDING" ;
#                   pav:importedOn          "DATE OF FIRST MOD VERSION INCLUDING"^^xsd:dateTime ;
#                    
#            #OPTIONAL STATEMENTS
#                   prov:wasInfluencedBy    "MIRO guidelines: ...." ;
#            
#            #OTHER ORIGINAL STATEMENTS IF ANY 
#            
#################################################################


#################################################################
#  Properties (sorted as in GSheet working document)
#################################################################

##########################################
########## Intrinsic properties ##########
##########################################


###  https://w3id.org/mod#acronym
mod:acronym         rdf:type                owl:DatatypeProperty ;
                    rdfs:subPropertyOf      rdfs:label ;
                    rdfs:label              "acronym"@en ,
                                            "acronyme"@fr ;
                    rdfs:domain             mod:SemanticArtefact ;
                    rdfs:range              xsd:string ;
                    dcterms:description     "MOD: Short acronym label, often used as an identifier within some ontology platforms such as BioPortal or OBO Foundry. OMV: A short name by which an ontology is formally known."@en ;
                    rdfs:isDefinedBy        <http://omv.ontoware.org/2005/05/ontology> ;
                    dcterms:issued          "2009-12-24"^^xsd:date ;
                    owl:equivalentProperty  <http://www.isibang.ac.in/ns/mod/1.0/acronym> ;
                    pav:derivedFrom         <http://www.isibang.ac.in/ns/mod/1.0> ;
                    pav:importedOn          "2015-08-05"^^xsd:dateTime ;
            
#            #OPTIONAL STATEMENTS
                    skos:historyNote        "This property has been adopted from OMV Ontology Metadata Vocabulary and redefined in the MOD namespace."@en ;
                    prov:wasInfluencedBy    "MIRO guidelines: A.1" ,
                                            "FAIR principle: F2" .
            


### http://purl.org/dc/terms/title
dcterms:title       rdf:type                rdf:Property ;
                    rdfs:subPropertyOf      <http://purl.org/dc/elements/1.1/title> ;
                    rdfs:label              "title"@en ,
                                            "titre"@fr ;
                    rdfs:range              rdfs:Literal ;
                    dcterms:description     "DCTERMS: A name given to the resource. OMV: The name by which an ontology is formally known. RDFS: A human-readable name for the subject. FOAF:  A name for some thing. SKOS: The preferred and alternative labels are useful when generating or creating human-readable representations of a knowledge organization system. SCHEMA: The name of the item."@en ;
                    rdfs:isDefinedBy        <http://purl.org/dc/terms/> ;
                    dcterms:issued          "2008-01-14"^^xsd:date ;
                    owl:equivalentProperty  cc:attributionName ,
                                            omv:name ,
                                            schema:name ,
                                            skos:prefLabel ,
                                            foaf:name ;
                    pav:derivedFrom         <http://www.isibang.ac.in/ns/mod/1.2> ;
                    pav:importedOn          "2017-07-06"^^xsd:dateTime ;
                    
            #OPTIONAL STATEMENTS
                    prov:wasInfluencedBy    "MIRO guidelines: A.1" ,
                                            "FAIR principle: F2" .
     


### http://purl.org/dc/terms/alternative
dcterms:alternative rdf:type                rdf:Property ;
                    rdfs:subPropertyOf      <http://purl.org/dc/elements/1.1/title>, dcterms:title ;
                    rdfs:label              "alternative name"@en ,
                                            "nom alternatif"@fr ;
                    rdfs:range              rdfs:Literal ;
                    dcterms:description     "DCTERMS: An alternative name for the resource. The distinction between titles and alternative titles is application-specific. SKOS: The preferred and alternative labels are useful when generating or creating human-readable representations of a knowledge organization system. SCHEMA: An alias for the item."@en ;
                    rdfs:isDefinedBy        <http://purl.org/dc/terms/> ;
                    dcterms:issued          "2000-07-11"^^xsd:date ;
                    owl:equivalentProperty  idot:alternatePrefix ,
                                            schema:alternateName ,
                                            skos:altLabel ;
                    pav:derivedFrom         <http://www.isibang.ac.in/ns/mod/1.2> ;
                    pav:importedOn          "2017-07-06"^^xsd:dateTime ;
                    
            #OPTIONAL STATEMENTS
                    prov:wasInfluencedBy    "MIRO guidelines: A.1" ,
                                            "FAIR principle: F2" .
            


### http://www.w3.org/2004/02/skos/core#hiddenLabel
skos:hiddenLabel    rdf:type                rdfs:Property ,
                                            owl:AnnotationProperty ;
                    rdfs:subPropertyOf      rdfs:label ;
                    rdfs:label              "hidden label"@en ,
                                            "nom caché"@fr ;

                    rdfs:range              rdfs:Literal ;
                    dcterms:description     "MOD: Hidden or past name. SKOS: A lexical label for a resource that should be hidden when generating visual displays of the resource, but should still be accessible to free text search operations."@en;
                    rdfs:isDefinedBy        <http://www.w3.org/2004/02/skos/core> ;
                    dcterms:issued          "2009-08-18"^^xsd:date ;
                    pav:derivedFrom         <http://www.isibang.ac.in/ns/mod/1.4> ;
                    pav:importedOn          "2018-08-02"^^xsd:dateTime ;
                    
            #OPTIONAL STATEMENTS
                    prov:wasInfluencedBy    "MIRO guidelines: A.1" ,
                                            "FAIR principle: F2" ;
            
            #OTHER ORIGINAL STATEMENTS IF ANY 
                    rdfs:comment            "S12 (not formally stated): The range of skos:hiddenLabel is the class of RDF plain literals. S13 (not formally stated): skos:prefLabel, skos:altLabel and skos:hiddenLabel are pairwise disjoint properties."@en .


    
###  https://w3id.org/mod#URI
mod:URI             rdf:type                owl:DatatypeProperty ;
                    rdfs:label              "URI"@en ,
                                            "URI"@fr ;
                    rdfs:domain             mod:SemanticArtefact ;
                    rdfs:range              xsd:anyURI ;
                    dcterms:description     "OMV: The URI of the ontology which is described by this metadata."@en ;
                    rdfs:isDefinedBy        <http://omv.ontoware.org/2005/05/ontology> ;
                    dcterms:issued          "2009-12-24"^^xsd:date ;
                    owl:equivalentProperty  omv:URI ;
                    pav:derivedFrom         <http://www.isibang.ac.in/ns/mod/1.2> ;
                    pav:importedOn          "2017-07-06"^^xsd:dateTime ;
            
#            #OPTIONAL STATEMENTS
                    skos:historyNote        "This property has been adopted from OMV Ontology Metadata Vocabulary and redefined in the MOD namespace."@en ;
                    prov:wasInfluencedBy    "MIRO guidelines: A.4" ,
                                            "FAIR principle: F1" .   
  


### http://www.w3.org/2002/07/owl#versionIRI
owl:versionIRI      rdf:type                owl:OntologyProperty ;
                    rdfs:label              "version IRI"@en ,
                                            "IRI de la version"@fr ;
                    rdfs:domain             owl:Ontology ;
                    rdfs:range              owl:Ontology ;
                    dcterms:description     "OWL: The property that identifies the version IRI of an ontology."@en ;  
                    rdfs:isDefinedBy        <http://www.w3.org/2002/07/owl#> ;
                    dcterms:issued          "2004-02-10"^^xsd:date ;
                    pav:derivedFrom         <http://www.isibang.ac.in/ns/mod/1.2> ;
                    pav:importedOn          "2017-07-06"^^xsd:dateTime ;
                    
            #OPTIONAL STATEMENTS
                    prov:wasInfluencedBy    "MIRO guidelines: A.4" ,
                                            "FAIR principle: F1" .
            


### http://purl.org/dc/terms/identifier
dcterms:identifier  rdf:type                rdf:Property ;
                    rdfs:subPropertyOf      <http://purl.org/dc/elements/1.1/identifier> ;
                    rdfs:label              "Other identifier"@en ,
                                            "Autre identifiant"@fr ;
                    rdfs:range              rdfs:Literal ;
                    dcterms:description     "DCTERMS: An unambiguous reference to the resource within a given context. Recommended practice is to identify the resource by means of a string conforming to an identification system. Examples include International Standard Book Number (ISBN), Digital Object Identifier (DOI), and Uniform Resource Name (URN).  Persistent identifiers should be provided as HTTP URIs. SKOS: A notation is a string of characters such as 'T58.5 or '303.4833' used to uniquely identify a concept within the scope of a given concept scheme. ADMS: adms:identifier is used to link any resource to an instance of adms:Identifier which is its range. N.B. it is not appropriate to use dcterms:identifer to link to the Identifier class as its range is rdfs:Literal. ADMS uses this to provide any identifier for the Asset."@en ;
                    rdfs:isDefinedBy        <http://purl.org/dc/terms/> ;
                    dcterms:issued          "2008-01-14"^^xsd:date ;
                    owl:equivalentProperty  skos:notation ,
                                            adms:identifier 
                                            shema:identifier;
                    pav:derivedFrom         <http://www.isibang.ac.in/ns/mod/1.0> ;
                    pav:importedOn          "2015-08-05"^^xsd:dateTime ;
                    
            #OPTIONAL STATEMENTS
                    prov:wasInfluencedBy    "FAIR principle: F1,A1" .
            


### http://www.w3.org/2002/07/owl#versionInfo
owl:versionInfo     rdf:type                owl:AnnotationProperty  ;
                    rdfs:label              "version information"@en ,
                                            "information de version"@fr ;
                    rdfs:domain             rdfs:Resource ;
                    rdfs:range              rdfs:Resource ;
                    dcterms:description     "MOD: The version of the released ontology. OMV: The version information of the ontology. OWL: The annotation property that provides version information for an ontology or another OWL construct. PAV: The version number of a resource. This is a freetext string, typical values are '1.5' or '21'. DOAP: A project release."@en ;  
                    rdfs:isDefinedBy        <http://www.w3.org/2002/07/owl#> ;
                    dcterms:issued          "2004-02-10"^^xsd:date ;
                    owl:equivalentProperty  omv:version ,
                                            pav:version ,
                                            doap:release ,
                                            oboinowl:data-version ,
                                            oboinowl:hasVersion ,
                                            schema:version ,
                                            <http://www.isibang.ac.in/ns/mod/1.0/version> ;
                    pav:derivedFrom         <http://www.isibang.ac.in/ns/mod/1.0> ;
                    pav:importedOn          "2015-08-05"^^xsd:dateTime ;
        
            #OPTIONAL STATEMENTS
                    prov:wasInfluencedBy    "MIRO guidelines: A.1" ,
                                            "FAIR principle: R1.2" .
            


###  https://w3id.org/mod#status
mod:status          rdf:type                owl:DatatypeProperty ;
                    rdfs:label              "status"@en ,
                                            "statut"@fr ;
                    rdfs:domain             mod:SemanticArtefact ;
                    rdfs:range              xsd:string ;
                    dcterms:description     "OMV: It specifies the tracking information for the contents of the ontology. Pre-defined values."@en ;
                    rdfs:isDefinedBy        <http://omv.ontoware.org/2005/05/ontology> ;
                    dcterms:issued          "2009-12-24"^^xsd:date ;
                    owl:equivalentProperty  idot:state ,
                                            adms:adms-status ;
                    pav:derivedFrom         <http://www.isibang.ac.in/ns/mod/1.0> ;
                    pav:importedOn          "2015-08-05"^^xsd:dateTime ;
            
#            #OPTIONAL STATEMENTS
                    skos:historyNote        "This property has been adopted from OMV Ontology Metadata Vocabulary and redefined in the MOD namespace."@en ;
                    prov:wasInfluencedBy    "FAIR principle: A2" .



### http://www.w3.org/2002/07/owl#Deprecated
owl:deprecated     rdf:type                owl:AnnotationProperty ; 
                   rdfs:label              "deprecated"@en ,
                                           "obsolète"@fr ;
                   rdfs:domain             rdfs:Resource ;
                   rdfs:range              rdfs:Resource ;
                   dcterms:description     "OWL: The annotation property that indicates that a given entity has been deprecated. IDOT: Indicates if the current dataset is obsolete (not provided any more to the public community). Value can either be 'true' or 'false' (xsd:boolean). The statement is usually omitted if 'false'."@en ;
                   rdfs:isDefinedBy        <http://www.w3.org/2002/07/owl#> ;
                   dcterms:issued          "2004-02-10"^^xsd:date ;
                   owl:equivalentProperty  idot:obsolete ,
                                           <http://www.isibang.ac.in/ns/mod/1.1/deprecated> ;                                         
                   pav:derivedFrom         <http://www.isibang.ac.in/ns/mod/1.1> ;
                   pav:importedOn          "2016-09-02"^^xsd:dateTime ; 
                                       
            #OPTIONAL STATEMENTS
                    prov:wasInfluencedBy   "FAIR principle: A2" .
            
     

### http://purl.org/dc/terms/license
dcterms:license     rdf:type                rdf:Property ;
                    rdfs:subPropertyOf      <http://purl.org/dc/elements/1.1/rights>, dcterms:rights ;
                    rdfs:label              "license"@en ,
                                            "licence"@fr ;
                    dcterms:description     "DCTERMS: A legal document giving official permission to do something with the resource. Recommended practice is to identify the license document with a URI. If this is not possible or feasible, a literal value that identifies the license may be provided. DCTERMS:rights Information about rights held in and over the resource. OMV: Underlying license model. SCHEMA: A license document that applies to this content, typically indicated by URL."@en ;
                    rdfs:isDefinedBy        <http://purl.org/dc/terms/> ;
                    dcterms:issued          "2004-06-14"^^xsd:date ;
                    owl:equivalentProperty  cc:license ,
                                            omv:license ,
                                            schema:license ;
                    pav:derivedFrom         <http://www.isibang.ac.in/ns/mod/1.0> ;
                    pav:importedOn          "2015-08-05"^^xsd:dateTime ;
                    
            #OPTIONAL STATEMENTS
                    prov:wasInfluencedBy    "MIRO guidelines: A.3" ,
                                            "FAIR principle: A2" ;
            
            #OTHER ORIGINAL STATEMENTS IF ANY 
                    <http://purl.org/dc/dcam/rangeIncludes>     dcterms:LicenseDocument .



###  https://w3id.org/mod#hasRepresentationLanguage
mod:hasRepresentationLanguage   
                    rdf:type                owl:DatatypeProperty ;
                    rdfs:label              "representation language"@en ,
                                            "language de représentation"@fr ;
                    rdfs:domain             mod:SemanticArtefactDistribution ;
                    rdfs:range              xsd:anyURI ;
                    dcterms:description     "MOD: A language that is used to create an ontology. OMV: The ontology language."@en ;
                    rdfs:isDefinedBy        <http://omv.ontoware.org/2005/05/ontology> ;
                    dcterms:issued          "2009-12-24"^^xsd:date ;
                    owl:equivalentProperty  omv:hasOntologyLanguage ,
                                            schema:fileFormat ,
                                            <http://www.isibang.ac.in/ns/mod/1.0/ontologyDesignLanguage> ;
                    pav:derivedFrom         <http://www.isibang.ac.in/ns/mod/1.0> ;
                    pav:importedOn          "2015-08-05"^^xsd:dateTime ;
                    
            #OPTIONAL STATEMENTS
                    skos:historyNote        "This property has been adopted from OMV Ontology Metadata Vocabulary and redefined in the MOD namespace."@en ;
                    prov:wasInfluencedBy    "MIRO guidelines: E.1" ,
                                            "FAIR principle: I1" .
                


###  https://w3id.org/mod#hasFormalityLevel
mod:hasFormalityLevel   
                    rdf:type                owl:DatatypeProperty ;
                    rdfs:label              "formality level"@en ,
                                            "niveau de formalisme"@fr ;
                    rdfs:domain             mod:SemanticArtefact ;
                    rdfs:range              xsd:string ;
                    dcterms:description     "MOD: The level of formality of an ontology. OMV: Level of formality of the ontology."@en ;
                    rdfs:isDefinedBy        <http://omv.ontoware.org/2005/05/ontology> ;
                    dcterms:issued          "2009-12-24"^^xsd:date ;
                    owl:equivalentProperty  omv:hasFormalityLevel ,
                                            schema:fileFormat ,
                                            <http://www.isibang.ac.in/ns/mod/1.0/formalityLevel> ;
                    pav:derivedFrom         <http://www.isibang.ac.in/ns/mod/1.0> ;
                    pav:importedOn          "2015-08-05"^^xsd:dateTime ;
                    
            #OPTIONAL STATEMENTS
                    skos:historyNote        "This property has been adopted from OMV Ontology Metadata Vocabulary and redefined in the MOD namespace."@en ;
                    prov:wasInfluencedBy    "MIRO guidelines: E.1" ,
                                            "FAIR principle: I1" .
              


###  https://w3id.org/mod#hasSyntax
mod:hasSyntax       rdf:type                owl:DatatypeProperty ;
                    rdfs:label              "syntax"@en ,
                                            "syntaxe"@fr ;
                    rdfs:domain             mod:SemanticArtefactDistribution ;
                    rdfs:range              xsd:anyURI ;
                    dcterms:description     "MOD: The syntax followed in the creation of an ontology. OMV: The presentation syntax for the ontology langage."@en ;
                    rdfs:isDefinedBy        <http://omv.ontoware.org/2005/05/ontology> ;
                    dcterms:issued          "2009-12-24"^^xsd:date ;
                    owl:equivalentProperty  omv:hasOntologySyntax ,
                                            dcterms:format ,
                                            <http://www.isibang.ac.in/ns/mod/1.0/syntax> ;
                    pav:derivedFrom         <http://www.isibang.ac.in/ns/mod/1.0> ;
                    pav:importedOn          "2015-08-05"^^xsd:dateTime ;
            
#            #OPTIONAL STATEMENTS
                    skos:historyNote        "This property has been adopted from OMV Ontology Metadata Vocabulary and redefined in the MOD namespace."@en ;
                    prov:wasInfluencedBy    "MIRO guidelines: E.1" ,
                                            "FAIR principle: I1" .
    


### http://purl.org/dc/terms/language
dcterms:language    rdf:type                rdf:Property ;
                    rdfs:subPropertyOf      <http://purl.org/dc/elements/1.1/language> ;
                    rdfs:label              "natural language"@en ,
                                            "langage naturel"@fr ;
                    dcterms:description     "DCTERMS: A language of the resource. Recommended practice is to use either a non-literal value representing a language from a controlled vocabulary such as ISO 639-2 or ISO 639-3, or a literal value consisting of an IETF Best Current Practice 47 [[IETF-BCP47](https://tools.ietf.org/html/bcp47)] language tag. OMV: The language of the content of the ontology, i.e. English, French, etc. DOAP: ISO language code a project has been translated into."@en ;
                    rdfs:isDefinedBy        <http://purl.org/dc/terms/> ;
                    dcterms:issued          "2008-01-14"^^xsd:date ;
                    owl:equivalentProperty  omv:naturalLanguage ,
                                            schema:inLanguage ,
                                            doap:language ;
                    pav:derivedFrom         <http://www.isibang.ac.in/ns/mod/1.0> ;
                    pav:importedOn          "2015-08-05"^^xsd:dateTime ;
                    
            #OPTIONAL STATEMENTS
                    prov:wasInfluencedBy    "FAIR principle: F2" ;
            
            #OTHER ORIGINAL STATEMENTS IF ANY 
                    <http://purl.org/dc/dcam/rangeIncludes>     dcterms:LinguisticSystem .

    
##########################################
######## Description properties ##########
##########################################
      

### http://purl.org/dc/terms/description
dcterms:description rdf:type                rdf:Property ;
                    rdfs:subPropertyOf      <http://purl.org/dc/elements/1.1/description> ;
                    rdfs:label              "description"@en ,
                                            "description"@fr ;
                    dcterms:description     "DCTERMS: An account of the resource. Description may include but is not limited to: an abstract, a table of contents, a graphical representation, or a free-text account of the resource. OMV: Free text description of an ontology. SCHEMA: A description of the item. DOAP: Plain text description of a project, of 2-4 sentences in length."@en ;
                    rdfs:isDefinedBy        <http://purl.org/dc/terms/> ;
                    dcterms:issued          "2008-01-14"^^xsd:date ;
                    owl:equivalentProperty  omv:description ,
                                            schema:description ,
                                            doap:description ;
                    pav:derivedFrom         <http://www.isibang.ac.in/ns/mod/1.0> ;
                    pav:importedOn          "2015-08-05"^^xsd:dateTime ;
                    
            #OPTIONAL STATEMENTS
                    prov:wasInfluencedBy    "MIRO guidelines: C.3" ,
                                            "FAIR principle: F2" .
            


### http://purl.org/dc/terms/abstract
dcterms:abstract    rdf:type                rdf:Property ;
                    rdfs:subPropertyOf      <http://purl.org/dc/elements/1.1/description>, dcterms:description ;
                    rdfs:label              "abstract"@en ,
                                            "résumé"@fr ;
                    dcterms:description     "DCTERMS: A summary of the resource."@en ;
                    rdfs:isDefinedBy        <http://purl.org/dc/terms/> ;
                    dcterms:issued          "2000-07-11"^^xsd:date ;
                    pav:derivedFrom         <http://www.isibang.ac.in/ns/mod/1.2> ;
                    pav:importedOn          "2017-07-06"^^xsd:dateTime ;
                    
            #OPTIONAL STATEMENTS
                    prov:wasInfluencedBy    "FAIR principle: F2" .
            


### http://creativecommons.org/ns#morePermissions
cc:morePermissions  rdf:type                rdf:Property ;
                    rdfs:subPropertyOf      dcterms:relation ; 
                    rdfs:label              "more permissions"@en ,
                                            "droits d'accès détaillés"@fr ;
                    rdfs:domain             cc:Work ;
                    rdfs:range              rdfs:Resource ;
                    dcterms:description     "CC: A related resource which describes additional permissions or alternative licenses for a Work which may be available."@en ;     
                    rdfs:isDefinedBy        <http://creativecommons.org/ns#> ;
                    dcterms:issued          "2008-03-03"^^xsd:date ;
                    pav:derivedFrom         <http://www.isibang.ac.in/ns/mod/1.4> ;
                    pav:importedOn          "2018-08-02"^^xsd:dateTime ;
                    
            #OPTIONAL STATEMENTS
                    prov:wasInfluencedBy    "FAIR principle: R1.1" .
  


### http://creativecommons.org/ns#useGuidelines
cc:useGuidelines    rdf:type                rdf:Property ;
                    rdfs:subPropertyOf      dcterms:relation ; 
                    rdfs:label              "use guidelines"@en ,
                                            "guide d'utilisation"@fr ;
                    rdfs:domain             cc:Work ;
                    rdfs:range              rdfs:Resource ;
                    dcterms:description     "CC: A related resource which defines non-binding use guidelines for the work."@en ;     
                    rdfs:isDefinedBy        <http://creativecommons.org/ns#> ;
                    dcterms:issued          "2008-03-03"^^xsd:date ;
                    pav:derivedFrom         <http://www.isibang.ac.in/ns/mod/1.4> ;
                    pav:importedOn          "2018-08-02"^^xsd:dateTime ;
                    
            #OPTIONAL STATEMENTS
                    prov:wasInfluencedBy    "FAIR principle: R1.1" .
  

### http://purl.org/dc/terms/bibliographicCitation
dcterms:bibliographicCitation
                    rdf:type                rdf:Property ;
                    rdfs:subPropertyOf      <http://purl.org/dc/elements/1.1/identifier> , dcterms:identifier;
                    rdfs:label              "bibliographic reference"@en ,
                                            "référence bibliographique";
                    rdfs:range              rdfs:Literal ;
                    dcterms:description     "DCTERMS: A bibliographic reference for the resource. Recommended practice is to include sufficient bibliographic detail to identify the resource as unambiguously as possible. OMV: List of bibliographic references describing the ontology and its applications. FOAF: A document that this thing is the primary topic of"@en ;
                    rdfs:isDefinedBy        <http://purl.org/dc/terms/> ;
                    dcterms:issued          "2003-02-15"^^xsd:date ;
                    owl:equivalentProperty  omv:reference ,
                                            foaf:isPrimaryTopicOf ,
                                            schema:citation ;
                    pav:derivedFrom         <http://www.isibang.ac.in/ns/mod/1.2> ;
                    pav:importedOn          "2017-07-06"^^xsd:dateTime ;
                    
            #OPTIONAL STATEMENTS
                    prov:wasInfluencedBy    "FAIR principle: F2" .



###  http://www.w3.org/ns/dcat#landingPage
dcat:landingPage    rdf:type                rdf:Property , owl:ObjectProperty ;
                    rdfs:subPropertyOf      foaf:page ; 
                    rdfs:label              "landing page"@en ,
                                            "page d'atterrissage"@fr ;
                    rdfs:range              foaf:Document ;
                    dcterms:description     "DCAT: A Web page that can be navigated to in a Web browser to gain access to the dataset, its distributions and/or additional information. MOD: A link to the documentation page on a thing. OMV: URL for further documentation. RDFS: Further information about the subject resource. DOAP: URL of Wiki for collaborative discussion of project. VANN: A reference to a resource that provides information on how this resource is to be used."@en ;
                    rdfs:isDefinedBy        <http://www.w3.org/TR/vocab-dcat/> ;
                    dcterms:issued          "2014-01-16"^^xsd:date ;
                    owl:equivalentProperty  omv:documentation ,
                                            vann:usageNote ,
                                            doap:wiki ,
                                            rdfs:seeAlso ,
                                            <http://www.isibang.ac.in/ns/mod/1.0/document> ;
                    pav:derivedFrom         <http://www.isibang.ac.in/ns/mod/1.0> ;
                    pav:importedOn          "2015-08-05"^^xsd:dateTime ;
                    
            #OPTIONAL STATEMENTS
                    prov:wasInfluencedBy    "MIRO guidelines: C.3, F.1" ,
                                            "FAIR principle: F2" ;
            
            #OTHER ORIGINAL STATEMENTS IF ANY 
                    skos:scopeNote          "If the distribution(s) are accessible only through a landing page (i.e. direct download URLs are not known), then the landing page link should be duplicated as accessURL on a distribution."@en .


###  http://www.w3.org/ns/dcat#accessURL
dcat:accessURL      rdf:type                rdf:Property , owl:ObjectProperty ;
                    rdfs:label              "access URL"@en ,
                                            "URL d'accès"@fr ;
                    rdfs:domain             dcat:Distribution ;
                    rdfs:range              rdfs:Resource ;
                    dcterms:description     "DCAT: A URL of a resource that gives access to a distribution of the dataset. E.g. landing page, feed, SPARQL endpoint. Use for all cases except a simple download link, in which case downloadURL is preferred. OMV: The location where the ontology can be found. It should be accessible via a URL. It can be the same as the value for URI property. DOAP:  Web page from which the project software can be downloaded."@en ;
                    rdfs:isDefinedBy        <http://www.w3.org/TR/vocab-dcat/> ;
                    dcterms:issued          "2014-01-16"^^xsd:date ;
                    owl:equivalentProperty  omv:resourceLocator ,
                                            doap:download-page ;
                    pav:derivedFrom         <http://www.isibang.ac.in/ns/mod/1.2> ;
                    pav:importedOn          "2017-07-06"^^xsd:dateTime ;
                    
            #OPTIONAL STATEMENTS
                    prov:wasInfluencedBy    "MIRO guidelines: A.4" ,
                                            "FAIR principle: F2" ;
            
            #OTHER ORIGINAL STATEMENTS IF ANY 
                     skos:scopeNote         "If the distribution(s) are accessible only through a landing page (i.e. direct download URLs are not known), then the landing page link should be duplicated as accessURL on a distribution."@en .
 
 

### http://www.w3.org/2000/01/rdf-schema#Comment
rdfs:comment        rdf:type                rdf:Property ;
                    rdfs:label              "notes or comments"@en ,
                                            "notes ou commentaires"@fr ;
                    rdfs:domain             rdfs:Resource ;
                    rdfs:range              rdfs:Literal ;           
                    dcterms:description     "RDFS: A description of the subject resource. OMV: Additional information about the ontology that is not included somewhere else (e.g. information that you do not want to include in the documentation)."@en ;
                    rdfs:isDefinedBy        <http://www.w3.org/2000/01/rdf-schema#> ;
                    dcterms:issued          "2002-04-30"^^xsd:date ;
                    owl:equivalentProperty  omv:notes ,
                                            dcterms:description ,
                                            adms:versionNotes ;
                    pav:derivedFrom         <http://www.isibang.ac.in/ns/mod/1.2> ;
                    pav:importedOn          "2017-07-06"^^xsd:dateTime ;
                    
            #OPTIONAL STATEMENTS
                    prov:wasInfluencedBy    "FAIR principle: F2" .
        


###  http://www.w3.org/ns/dcat#keyword
dcat:keyword        rdf:type                rdf:Property , owl:DatatypeProperty ;
                    rdfs:subPropertyOf      dcterms:subject ; 
                    rdfs:label              "keyword"@en ,
                                            "motclé"@fr ;
                    rdfs:range              rdfs:Literal ;
                    dcterms:description     "DCAT: A keyword or tag describing a resource. MOD: A keyword(s) is used to describe the content of an ontology. OMV: List of keywords related to an ontology. SCHEMA: Keywords or tags used to describe this content. Multiple entries in a keywords list are typically delimited by commas."@en ;
                    rdfs:isDefinedBy        <http://www.w3.org/TR/vocab-dcat/> ;
                    dcterms:issued          "2014-01-16"^^xsd:date ;
                    owl:equivalentProperty   omv:keywords ,
                                             schema:keywords ,
                                             <http://www.isibang.ac.in/ns/mod/1.1/keyword> ;
                    pav:derivedFrom         <http://www.isibang.ac.in/ns/mod/1.0> ;
                    pav:importedOn          "2015-08-05"^^xsd:dateTime ;
                    
            #OPTIONAL STATEMENTS
                    prov:wasInfluencedBy    "MIRO guidelines: C.1" ,
                                            "FAIR principle: F2" .
            


### http://purl.org/dc/terms/type
dcterms:type        rdf:type                rdf:Property ;
                    rdfs:subPropertyOf      <http://purl.org/dc/elements/1.1/type> ;
                    rdfs:label              "type"@en ,
                                            "type"@fr ;
                    dcterms:description     "DCTERMS: The nature or genre of the resource. Recommended practice is to use a controlled vocabulary such as the DCMI Type Vocabulary [[DCMI-TYPE](http://dublincore.org/documents/dcmi-type-vocabulary/)]. To describe the file format, physical medium, or dimensions of the resource, use the property Format. OMV: The nature of the content of the ontology."@en ;
                    rdfs:isDefinedBy        <http://purl.org/dc/terms/> ;
                    dcterms:issued          "2008-01-14"^^xsd:date ;
                    owl:equivalentProperty  omv:isOfType ;
                    pav:derivedFrom         <http://www.isibang.ac.in/ns/mod/1.2> ;
                    pav:importedOn          "2017-07-06"^^xsd:dateTime ;
                    
            #OPTIONAL STATEMENTS
                    prov:wasInfluencedBy    "FAIR principle: F2" .




############################################################################################# HERE: moved properties as defined in MOD1.4 and updated to MOD2
############################################################################################# HERE: moved properties as defined in MOD1.4 and updated to MOD2
############################################################################################# HERE: moved properties as defined in MOD1.4 and updated to MOD2
############################################################################################# HERE: moved properties as defined in MOD1.4 and updated to MOD2
############################################################################################# HERE: moved properties as defined in MOD1.4 and updated to MOD2
############################################################################################# HERE: moved properties as defined in MOD1.4 and updated to MOD2
############################################################################################# HERE: moved properties as defined in MOD1.4 and updated to MOD2
############################################################################################# HERE: moved properties as defined in MOD1.4 and updated to MOD2


### http://purl.org/dc/terms/creator
dcterms:creator     rdf:type                rdf:Property ;
                    rdfs:subPropertyOf      <http://purl.org/dc/elements/1.1/creator>, dcterms:contributor ;
                    rdfs:label              "creator"@en ,
                                            "créateur"@fr ;
                    dcterms:description     "DCTERMS: An entity responsible for making the resource. Recommended practice is to identify the creator with a URI.  If this is not possible or feasible, a literal value that identifies the creator may be provided."@en ;
                    rdfs:isDefinedBy        <http://purl.org/dc/terms/> ;
                    dcterms:issued          "2008-01-14"^^xsd:date ;
                    owl:equivalentProperty  omv:creator ,
                                            pav:authoredBy ,
                                            pav:createdBy ,
                                            schema:author ,
                                            doap:maintainer ,
                                            prov:wasAttributedTo ,
                                            foaf:maker ;
                    pav:derivedFrom         <http://www.isibang.ac.in/ns/mod/1.0> ;
                    pav:importedOn          "2015-08-05"^^xsd:dateTime ;
                    
            #OPTIONAL STATEMENTS
                    prov:wasInfluencedBy    "MIRO guidelines: C.2" ;
            
            #OTHER ORIGINAL STATEMENTS IF ANY 
                    <http://purl.org/dc/dcam/rangeIncludes>     dcterms:Agent .


#################################################################
#   AnnotationProperty
#################################################################

###  http://www.w3.org/2004/02/skos/core#historyNote
skos:historyNote rdf:type owl:AnnotationProperty ;
                 rdfs:comment "A note about the past state/use/meaning of a concept."@en ;
                 rdfs:subPropertyOf skos:note .


###  http://www.w3.org/2004/02/skos/core#note
skos:note rdf:type owl:AnnotationProperty .


#################################################################
#    Datatypes
#################################################################

###  http://schema.org/Date
schema:Date rdf:type rdfs:Datatype .


###  http://schema.org/DateTime
schema:DateTime rdf:type rdfs:Datatype .


###  http://schema.org/Number
schema:Number rdf:type rdfs:Datatype .


###  http://schema.org/Text
schema:Text rdf:type rdfs:Datatype .


###  http://schema.org/URL
schema:URL rdf:type rdfs:Datatype .


#################################################################
#    Object Properties
#################################################################

###  http://creativecommons.org/ns#attributionURL
cc:attributionURL rdf:type owl:ObjectProperty ;
                  rdfs:range rdfs:Resource ;
                  rdfs:comment "The URL the creator of a Work would like used when attributing re-use."@en ;
                  rdfs:label "attribution URL"@en .


###  http://creativecommons.org/ns#license
cc:license rdf:type owl:ObjectProperty ;
           rdfs:subPropertyOf dcterms:license ;
           rdfs:comment """A Work has license a License.
(a subproperty of dc:license, the same as xhtml:license)."""@en ;
           rdfs:label "license"@en .



###  http://purl.org/dc/terms/Relation
dcterms:Relation rdf:type owl:ObjectProperty ;
             rdfs:range rdfs:Resource ;
             rdfs:comment "A related resource."@en ;
             rdfs:label "relation"@en .


###  http://purl.org/dc/terms/accessRights
dcterms:accessRights rdf:type owl:ObjectProperty ;
                 rdfs:domain [ rdf:type owl:Class ;
                               owl:unionOf ( dcat:Distribution
                                             dcat:Resource
                                           )
                             ] ;
                 rdfs:range dcterms:RightsStatement ;
                 rdfs:comment "Information about who access the resource or an indication of its security status."@en ;
                 rdfs:label "access rights"@en .


###  http://purl.org/dc/terms/accrualMethod
dcterms:accrualMethod rdf:type owl:ObjectProperty ;
                  rdfs:domain :SemanticArtefact ;
                  rdfs:range dcterms:MethodOfAccrual ;
                  rdfs:comment "The method by which items are added to a collection."@en ;
                  rdfs:label "accrual method"@en .


###  http://purl.org/dc/terms/accrualPeriodicity
dcterms:accrualPeriodicity rdf:type owl:ObjectProperty ;
                       rdfs:domain dcat:Dataset ;
                       rdfs:range dcterms:Frequency ;
                       rdfs:comment "The frequency at which dataset is published."@en ;
                       rdfs:label "accrual periodicity"@en .


###  http://purl.org/dc/terms/accrualPolicy
dcterms:accrualPolicy rdf:type owl:ObjectProperty ;
                  rdfs:domain :SemanticArtefact ;
                  rdfs:range dcterms:Policy ;
                  rdfs:comment "The policy governing the addition of items to a collection."@en ,
                               "accrual policy"@en .


###  http://purl.org/dc/terms/audience
dcterms:audience rdf:type owl:ObjectProperty ;
             rdfs:comment "A class of agents for whom the resource is intended or useful."@en ;
             rdfs:label "audience"@en .


###  http://purl.org/dc/terms/conformsTo
dcterms:conformsTo rdf:type owl:ObjectProperty ;
               rdfs:domain [ rdf:type owl:Class ;
                             owl:unionOf ( dcat:Distribution
                                           dcat:Resource
                                         )
                           ] ;
               rdfs:range dcterms:Standard ;
               rdfs:comment "An established standard to which the described resource conforms."@en ;
               rdfs:label "conforms to"@en .


###  http://purl.org/dc/terms/contributor
dcterms:contributor rdf:type owl:ObjectProperty ;
                rdfs:range dcterms:Agent ;
                rdfs:comment "An entity responsible for making contributions to the resource."@en ;
                rdfs:label "contributor"@en .


###  http://purl.org/dc/terms/coverage
dcterms:coverage rdf:type owl:ObjectProperty ;
             rdfs:range [ rdf:type owl:Class ;
                          owl:unionOf ( dcterms:Jurisdiction
                                        dcterms:Location
                                        dcterms:PeriodOfTime
                                      )
                        ] ;
             rdfs:comment "The spatial or temporal topic of the resource, spatial applicability of the resource, or jurisdiction under which the resource is relevant."@en ;
             rdfs:label "coverage"@en .


###  http://purl.org/dc/terms/creator
dcterms:creator rdf:type owl:ObjectProperty ;
            rdfs:comment "An entity responsible for making the resource."@en ;
            rdfs:label "creator"@en .


###  http://purl.org/dc/terms/format
dcterms:format rdf:type owl:ObjectProperty ;
           rdfs:range dcterms:MediaTypeOrExtent ;
           rdfs:comment "The file format, physical medium, or dimensions of the resource."@en ;
           rdfs:label "format"@en .


###  http://purl.org/dc/terms/hasFormat
dcterms:hasFormat rdf:type owl:ObjectProperty ;
              owl:inverseOf dcterms:isFormatOf ;
              rdfs:comment "a related resource that is substantially the same as the pre-existing described resource, but in another format."@en ;
              rdfs:label "has format"@en .


###  http://purl.org/dc/terms/hasPart
dcterms:hasPart rdf:type owl:ObjectProperty ;
            owl:inverseOf dcterms:isPartOf ;
            rdfs:comment "A related resource that is included either physically or logically in the described resource."@en ;
            rdfs:label "has part"@en .


###  http://purl.org/dc/terms/hasVersion
dcterms:hasVersion rdf:type owl:ObjectProperty ;
               rdfs:range rdfs:Resource ;
               rdfs:comment "a related resource that is a version, edition, or adaptation of the described resource."@en ;
               rdfs:label "has verison"@en .


###  http://purl.org/dc/terms/isFormatOf
dcterms:isFormatOf rdf:type owl:ObjectProperty ;
               rdfs:range rdfs:Resource ;
               rdfs:comment "a related resource that is substantially the same as the described resource, but in another format."@en ;
               rdfs:label "is format of"@en .


###  http://purl.org/dc/terms/isPartOf
dcterms:isPartOf rdf:type owl:ObjectProperty ;
             rdfs:range rdfs:Resource ;
             rdfs:comment "A related resource in which the described resource is physically or logically included."@en ;
             rdfs:label "is part of"@en .


###  http://purl.org/dc/terms/isReferencedBy
dcterms:isReferencedBy rdf:type owl:ObjectProperty ;
                   rdfs:range rdfs:Resource ;
                   rdfs:comment "A related resource that references, cites, or otherwise points to the described resource."@en ;
                   rdfs:label "is referenced by"@en .


###  http://purl.org/dc/terms/isVersionOf
dcterms:isVersionOf rdf:type owl:ObjectProperty ;
                rdfs:range rdfs:Resource ;
                rdfs:comment "A related resource of which the described resource is a version, edition, or adaptation."@en ;
                rdfs:label "is version of"@en .





###  http://purl.org/dc/terms/publisher
dcterms:publisher rdf:type owl:ObjectProperty ;
              rdfs:range dcterms:Agent ;
              rdfs:comment "An entity responsible for making the resource available."@en ;
              rdfs:label "publisher"@en .


###  http://purl.org/dc/terms/requires
dcterms:requires rdf:type owl:ObjectProperty ;
             rdfs:range rdfs:Resource ;
             rdfs:comment "A related resource that is required by the described resource to support its function, delivery, or coherence."@en ;
             rdfs:label "requires"@en .


###  http://purl.org/dc/terms/rights
dcterms:rights rdf:type owl:ObjectProperty ;
           rdfs:range dcterms:RightsStatement ;
           rdfs:comment "Information about rights held in and over the resource."@en ;
           rdfs:label "rights"@en .


###  http://purl.org/dc/terms/rightsHolder
dcterms:rightsHolder rdf:type owl:ObjectProperty ;
                 rdfs:range dcterms:Agent ;
                 rdfs:comment "A person or organization owning or managing rights over the resource."@en ;
                 rdfs:label "rights holder"@en .


###  http://purl.org/dc/terms/source
dcterms:source rdf:type owl:ObjectProperty ;
           rdfs:range rdfs:Resource ;
           rdfs:comment "A related resource from which the described resource is derived."@en ;
           rdfs:label "source"@en .


###  http://purl.org/dc/terms/spatial
dcterms:spatial rdf:type owl:ObjectProperty ;
            rdfs:subPropertyOf dcterms:coverage ;
            rdfs:range dcterms:Location ;
            rdfs:comment "Spatial characteristics of the resource."@en ;
            rdfs:label "spatial coverage"@en .


###  http://purl.org/dc/terms/temporal
dcterms:temporal rdf:type owl:ObjectProperty ;
             rdfs:subPropertyOf dcterms:coverage ;
             rdfs:range dcterms:PeriodOfTime ;
             rdfs:comment "Temporal characteristics of the resource."@en ;
             rdfs:label "temporal coverage"@en .


###  http://purl.org/dc/terms/type
dcterms:type rdf:type owl:ObjectProperty ;
         rdfs:range rdfs:Class ;
         rdfs:comment "The nature or genre of the resource."@en ;
         rdfs:label "type"@en .


###  http://purl.org/pav/authoredBy
pav:authoredBy rdf:type owl:ObjectProperty ;
               rdfs:subPropertyOf dcterms:creator ,
                                  pav:contributedBy ;
               rdfs:domain prov:Entity ;
               rdfs:range prov:Agent ;
               rdfs:comment "An agent that originated or gave existence to the work that is expressed by the digital resource."@en ;
               rdfs:label "authored by"@en .


###  http://purl.org/pav/contributedBy
pav:contributedBy rdf:type owl:ObjectProperty ;
                  rdfs:subPropertyOf dcterms:contributor ,
                                     prov:wasAttributedTo ;
                  rdfs:domain prov:Entity ;
                  rdfs:range prov:Agent ;
                  rdfs:comment "The resource was contributed to by the given agent."@en ;
                  rdfs:label "contributed by"@en .


###  http://purl.org/pav/createdBY
pav:createdBY rdf:type owl:ObjectProperty ;
              rdfs:subPropertyOf dcterms:creator ,
                                 prov:wasAttributedTo ;
              rdfs:domain prov:Entity ;
              rdfs:range prov:Agent ;
              rdfs:comment "An agent primary responsible for making the digital artifact or resource representation."@en ;
              rdfs:label "created bY"@en .


###  http://purl.org/pav/createdWith
pav:createdWith rdf:type owl:ObjectProperty ;
                rdfs:range rdfs:Resource ;
                rdfs:comment "The software/tool used by the creator (pav:createdBy) when making the digital resource, for instance a word processor or an annotation tool. A more independent software agent that creates the resource without direct interaction by a human creator should instead be indicated using pav:createdBy."@en ;
                rdfs:label "created with"@en .


###  http://purl.org/pav/curatedBy
pav:curatedBy rdf:type owl:ObjectProperty ;
              rdfs:subPropertyOf pav:contributedBy ;
              owl:inverseOf pav:curates ;
              rdfs:comment "Specifies an agent specialist responsible for shaping the expression in an appropriate format. Often the primary agent responsible for ensuring the quality of the representation."@en ;
              rdfs:label "curated by"@en .


###  http://purl.org/pav/curates
pav:curates rdf:type owl:ObjectProperty ;
            rdfs:comment "Provided for backwards compatibility. Use instead the inverse pav:curatedBy."@en ;
            rdfs:label "curates"@en .


###  http://purl.org/pav/derivedFrom
pav:derivedFrom rdf:type owl:ObjectProperty ;
                rdfs:range rdfs:Resource ;
                rdfs:comment "Derived from a different resource."@en ;
                rdfs:label "derived from"@en .


###  http://purl.org/pav/hasCurrentVersion
pav:hasCurrentVersion rdf:type owl:ObjectProperty ;
                      rdfs:subPropertyOf pav:hasVersion ;
                      rdfs:comment "This resource has a more specific, versioned resource with equivalent content."@en ;
                      rdfs:label "has current version"@en .


###  http://purl.org/pav/hasVersion
pav:hasVersion rdf:type owl:ObjectProperty ;
               rdfs:subPropertyOf dcterms:hasVersion ,
                                  prov:generalizationOf ;
               rdfs:comment "This resource has a more specific, versioned resource."@en ;
               rdfs:label "has version"@en .


###  http://rdfs.org/ns/void#classPartition
void:classPartition rdf:type owl:ObjectProperty ;
                    rdfs:subPropertyOf void:subset ;
                    rdfs:domain void:Dataset ;
                    rdfs:range void:Dataset ;
                    rdfs:comment "A subset of a void:Dataset that contains only the entities of a certain rdfs:Class."@en ;
                    rdfs:label "class partition"@en .


###  http://rdfs.org/ns/void#dataDump
void:dataDump rdf:type owl:ObjectProperty ;
              rdfs:domain void:Dataset ;
              rdfs:range rdfs:Resource ;
              rdfs:comment "An RDF dump, partial or complete, of a void:Dataset."@en ;
              rdfs:label "data dump"@en .


###  http://rdfs.org/ns/void#exampleResource
void:exampleResource rdf:type owl:ObjectProperty ;
                     rdfs:domain void:Dataset ;
                     rdfs:range rdfs:Resource ;
                     rdfs:comment "An example entity that is representative for the entities described in a void:Dataset."@en ;
                     rdfs:label "example resource"@en .


###  http://rdfs.org/ns/void#propertyPartition
void:propertyPartition rdf:type owl:ObjectProperty ;
                       rdfs:subPropertyOf void:subset ;
                       rdfs:domain void:Dataset ;
                       rdfs:range void:Dataset ;
                       rdfs:comment "A subset of a void:Dataset that contains only the triples of a certain rdf:Property."@en ;
                       rdfs:label "property partition"@en .


###  http://rdfs.org/ns/void#rootResource
void:rootResource rdf:type owl:ObjectProperty ;
                  rdfs:domain void:Dataset ;
                  rdfs:range rdfs:Resource ;
                  rdfs:comment "A top concept or entry point for a void:Dataset that is structured in a tree-like fashion. All resources in a dataset can be reached by following links from its root resources in a small number of steps."@en ;
                  rdfs:label "root resource"@en .


###  http://rdfs.org/ns/void#sparqlEndpoint
void:sparqlEndpoint rdf:type owl:ObjectProperty ;
                    rdfs:domain void:Dataset ;
                    rdfs:range rdfs:Resource ;
                    rdfs:comment "A SPARQL protocol endpoint that allows SPARQL query access to a void:Dataset."@en ;
                    rdfs:label "sparql endpoint"@en .


###  http://rdfs.org/ns/void#subset
void:subset rdf:type owl:ObjectProperty ;
            rdfs:domain void:Dataset ;
            rdfs:range void:Dataset ;
            rdfs:comment "A void:Dataset that is part of another void:Dataset."@en ;
            rdfs:label "subset"@en .


###  http://rdfs.org/ns/void#uriLookupEndpoint
void:uriLookupEndpoint rdf:type owl:ObjectProperty ;
                       rdfs:domain void:Dataset ;
                       rdfs:range rdfs:Resource ;
                       rdfs:comment "Defines a simple URI look-up protocol for accessing a dataset."@en ;
                       rdfs:label "uri lookup endpoint"@en .


###  http://rdfs.org/ns/void#vocabulary
void:vocabulary rdf:type owl:ObjectProperty ;
                rdfs:domain void:Dataset ;
                rdfs:range rdfs:Resource ;
                rdfs:comment "A vocabulary that is used in the dataset."@en ;
                rdfs:label "vocabulary"@en .


###  http://schema.org/about
schema:about rdf:type owl:ObjectProperty ;
                          rdfs:domain schema:CreativeWork ;
                          rdfs:comment "The subject matter of the content."@en ;
                          rdfs:label "about"@en .


###  http://schema.org/associatedMedia
schema:associatedMedia rdf:type owl:ObjectProperty ;
                                    rdfs:domain schema:CreativeWork ;
                                    rdfs:range schema:MediaObject ;
                                    rdfs:comment "A media object that encodes this CreativeWork. This property is a synonym for encoding."@en ;
                                    rdfs:label "associated media"@en .


###  http://schema.org/audience
schema:audience rdf:type owl:ObjectProperty ;
                             rdfs:domain schema:CreativeWork ;
                             rdfs:range schema:Audience ;
                             rdfs:comment "An intended audience, i.e. a group for whom something was created."@en ;
                             rdfs:label "audience"@en .


###  http://schema.org/author
schema:author rdf:type owl:ObjectProperty ;
                           rdfs:domain schema:CreativeWork ;
                           rdfs:range [ rdf:type owl:Class ;
                                        owl:unionOf ( schema:Organization
                                                      foaf:Person
                                                    )
                                      ] ;
                           rdfs:comment "The author of this content or rating. Please note that author is special in that HTML 5 provides a special mechanism for indicating authorship via the rel tag. That is equivalent to this and may be used interchangeably."@en ;
                           rdfs:label "author"@en .


###  http://schema.org/citation
schema:citation rdf:type owl:ObjectProperty ;
                             rdfs:domain schema:CreativeWork ;
                             rdfs:range schema:CreativeWork ;
                             rdfs:comment "A citation or reference to another creative work, such as another publication, web page, scholarly article, etc."@en ;
                             rdfs:label "citation"@en .


###  http://schema.org/comment
schema:comment rdf:type owl:ObjectProperty ;
                            rdfs:range schema:Comment ;
                            rdfs:comment "Comments, typically from users."@en ;
                            rdfs:label "comment"@en .


###  http://schema.org/contributor
schema:contributor rdf:type owl:ObjectProperty ;
                                rdfs:domain schema:CreativeWork ;
                                rdfs:range [ rdf:type owl:Class ;
                                             owl:unionOf ( schema:Organization
                                                           foaf:Person
                                                         )
                                           ] ;
                                rdfs:comment "A secondary contributor to the CreativeWork or Event."@en ;
                                rdfs:label "contributor"@en .


###  http://schema.org/copyrightHolder
schema:copyrightHolder rdf:type owl:ObjectProperty ;
                                    rdfs:domain schema:CreativeWork ;
                                    rdfs:range [ rdf:type owl:Class ;
                                                 owl:unionOf ( schema:Organization
                                                               foaf:Person
                                                             )
                                               ] ;
                                    rdfs:comment "The party holding the legal copyright to the CreativeWork."@en ;
                                    rdfs:label "copyright holder"@en .


###  http://schema.org/distribution
schema:distribution rdf:type owl:ObjectProperty ;
                                 rdfs:domain schema:Dataset ;
                                 rdfs:range schema:dataDownload ;
                                 rdfs:comment "A downloadable form of this dataset, at a specific location, in a specific format."@en ;
                                 rdfs:label "distribution"@en .


###  http://schema.org/hasPart
schema:hasPart rdf:type owl:ObjectProperty ;
                            owl:inverseOf schema:isPartOf ;
                            rdfs:comment "Indicates an item or CreativeWork that is part of this item, or CreativeWork (in some sense)."@en ;
                            rdfs:label "has part"@en .


###  http://schema.org/includedInDataCatalog
schema:includedInDataCatalog rdf:type owl:ObjectProperty ;
                                          rdfs:domain schema:Dataset ;
                                          rdfs:range schema:DataCatalog ;
                                          rdfs:comment "A data catalog which contains this dataset."@en ;
                                          rdfs:label "included in data catalog"@en .


###  http://schema.org/isBasedOn
schema:isBasedOn rdf:type owl:ObjectProperty ;
                              rdfs:domain schema:CreativeWork ;
                              rdfs:range schema:CreativeWork ;
                              rdfs:comment "A resource from which this work is derived or from which it is a modification or adaption."@en ;
                              rdfs:label "is based on"@en .


###  http://schema.org/isPartOf
schema:isPartOf rdf:type owl:ObjectProperty ;
                             rdfs:domain schema:CreativeWork ;
                             rdfs:range schema:CreativeWork ;
                             rdfs:comment "Indicates an item or CreativeWork that this item, or CreativeWork (in some sense), is part of."@en ;
                             rdfs:label "is Part of"@en .


###  http://schema.org/license
schema:license rdf:type owl:ObjectProperty ;
                            rdfs:domain schema:CreativeWork ;
                            rdfs:range schema:CreativeWork ;
                            rdfs:comment "A license document that applies to this content, typically indicated by URL."@en ;
                            rdfs:label "license"@en .


###  http://schema.org/mainEntity
schema:mainEntity rdf:type owl:ObjectProperty ;
                               rdfs:domain schema:CreativeWork ;
                               rdfs:comment "Indicates the primary entity described in some page or other CreativeWork."@en ;
                               rdfs:label "main entity"@en .


###  http://schema.org/publisher
schema:publisher rdf:type owl:ObjectProperty ;
                              rdfs:domain schema:CreativeWork ;
                              rdfs:range [ rdf:type owl:Class ;
                                           owl:unionOf ( schema:Organization
                                                         foaf:Person
                                                       )
                                         ] ;
                              rdfs:comment "The publisher of the creative work."@en ;
                              rdfs:label "publisher"@en .


###  http://schema.org/review
schema:review rdf:type owl:ObjectProperty ;
                           rdfs:range schema:Review ;
                           rdfs:comment "A review of the item."@en ;
                           rdfs:label "review"@en .


###  http://schema.org/sourceOrganization
schema:sourceOrganization rdf:type owl:ObjectProperty ;
                                       rdfs:domain schema:CreativeWork ;
                                       rdfs:range schema:Organization ;
                                       rdfs:comment "The Organization on whose behalf the creator was working."@en ;
                                       rdfs:label "source organization"@en .


###  http://schema.org/spatial
schema:spatial rdf:type owl:ObjectProperty ;
                            rdfs:domain schema:CreativeWork ;
                            rdfs:range schema:Place ;
                            rdfs:comment "The \"spatial\" property can be used in cases when more specific properties (e.g. locationCreated, spatialCoverage, contentLocation) are not known to be appropriate."@en ;
                            rdfs:label "spatial"@en .


###  http://schema.org/translationOfWork
schema:translationOfWork rdf:type owl:ObjectProperty ;
                                      owl:inverseOf schema:workTranslation ;
                                      rdfs:comment "The work that this work has been translated from. e.g. 物种起源 is a translationOf “On the Origin of Species”"@en ;
                                      rdfs:label "translation of work"@en .


###  http://schema.org/translator
schema:translator rdf:type owl:ObjectProperty ;
                               rdfs:domain schema:CreativeWork ;
                               rdfs:range [ rdf:type owl:Class ;
                                            owl:unionOf ( schema:Organization
                                                          foaf:Person
                                                        )
                                          ] ;
                               rdfs:comment "Organization or person who adapts a creative work to different languages, regional differences and technical requirements of a target market, or that translates during some event."@en ;
                               rdfs:label "translator"@en .


###  http://schema.org/workExample
schema:workExample rdf:type owl:ObjectProperty ;
                                rdfs:domain schema:CreativeWork ;
                                rdfs:range schema:CreativeWork ;
                                rdfs:comment "Example/instance/realization/derivation of the concept of this creative work. eg. The paperback edition, first edition, or eBook."@en ;
                                rdfs:label "work example"@en .


###  http://schema.org/workTranslation
schema:workTranslation rdf:type owl:ObjectProperty ;
                                    rdfs:domain schema:CreativeWork ;
                                    rdfs:range schema:CreativeWork ;
                                    rdfs:comment "A work that is a translation of the content of this work. e.g. 西遊記 has an English workTranslation “Journey to the West”,a German workTranslation “Monkeys Pilgerfahrt” and a Vietnamese translation Tây du ký bình khảo."@en ;
                                    rdfs:label "work translation"@en .


###  http://usefulinc.com/ns/doap#blog
doap:blog rdf:type owl:ObjectProperty ;
          rdfs:domain doap:Project ;
          rdfs:range [ rdf:type owl:Class ;
                       owl:unionOf ( sioc:Weblog
                                     rdfs:Resource
                                   )
                     ] ;
          rdfs:comment "URI of a blog related to a project."@en ;
          rdfs:label "blog"@en .


###  http://usefulinc.com/ns/doap#bug-database
doap:bug-database rdf:type owl:ObjectProperty ;
                  rdfs:domain doap:Project ;
                  rdfs:range rdfs:Resource ;
                  rdfs:comment "Bug tracker for a project."@en ;
                  rdfs:label "bug-database"@en .


###  http://usefulinc.com/ns/doap#developer
doap:developer rdf:type owl:ObjectProperty ;
               rdfs:domain doap:Project ;
               rdfs:range foaf:Person ;
               rdfs:comment "Developer of software for the project."@en ;
               rdfs:label "developer"@en .


###  http://usefulinc.com/ns/doap#download-mirror
doap:download-mirror rdf:type owl:ObjectProperty ;
                     rdfs:domain doap:Project ;
                     rdfs:range rdfs:Resource ;
                     rdfs:comment "Mirror of software download web page."@en ;
                     rdfs:label "download mirror"@en .


###  http://usefulinc.com/ns/doap#download-page
doap:download-page rdf:type owl:ObjectProperty ;
                   rdfs:domain doap:Project ;
                   rdfs:range rdfs:Resource ;
                   rdfs:comment "Web page from which the project software can be downloaded."@en ;
                   rdfs:label "download page"@en .


###  http://usefulinc.com/ns/doap#helper
doap:helper rdf:type owl:ObjectProperty ;
            rdfs:domain doap:Project ;
            rdfs:range foaf:Person ;
            rdfs:comment "Project contributor."@en ;
            rdfs:label "helper"@en .


###  http://usefulinc.com/ns/doap#mailing-list
doap:mailing-list rdf:type owl:ObjectProperty ;
                  rdfs:domain doap:Project ;
                  rdfs:range sioc:MailingList ;
                  rdfs:comment "Mailing list home page or email address."@en ;
                  rdfs:label "mailing-list"@en .


###  http://usefulinc.com/ns/doap#maintainer
doap:maintainer rdf:type owl:ObjectProperty ;
                rdfs:domain doap:Project ;
                rdfs:range foaf:Person ;
                rdfs:comment "Maintainer of a project, a project leader."@en ;
                rdfs:label "maintainer"@en .


###  http://usefulinc.com/ns/doap#release
doap:release rdf:type owl:ObjectProperty ;
             rdfs:domain doap:Project ;
             rdfs:range doap:Version ;
             rdfs:comment "A project release."@en ;
             rdfs:label "release"@en .


###  http://usefulinc.com/ns/doap#repository
doap:repository rdf:type owl:ObjectProperty ;
                rdfs:domain doap:Project ;
                rdfs:range doap:Repository ;
                rdfs:comment "Source code repository."@en ;
                rdfs:label "repository"@en .


###  http://usefulinc.com/ns/doap#screenshots
doap:screenshots rdf:type owl:ObjectProperty ;
                 rdfs:domain doap:Project ;
                 rdfs:range rdfs:Resource ;
                 rdfs:comment "Web page with screenshots of project."@en ;
                 rdfs:label "screenshots"@en .


###  http://usefulinc.com/ns/doap#wiki
doap:wiki rdf:type owl:ObjectProperty ;
          rdfs:domain doap:Project ;
          rdfs:range sioc:Wiki ;
          rdfs:comment "URL of Wiki for collaborative discussion of project."@en ;
          rdfs:label "wiki"@en .


###  http://w3id.org/nkos#alignedWith
nkos:alignedWith rdf:type owl:ObjectProperty ;
                 rdfs:domain frbr:Expression ;
                 rdfs:range frbr:Expression ;
                 rdfs:comment "A related resource with which the described resource is aligned."@en ;
                 rdfs:label "aligned with"@en .


###  http://w3id.org/nkos#basedOn
nkos:basedOn rdf:type owl:ObjectProperty ;
             rdfs:domain frbr:Work ;
             rdfs:range frbr:Work ;
             rdfs:comment "A resource used as the source for a derivative resource."@en ;
             rdfs:label "based on"@en .


###  http://w3id.org/nkos#usedBy
nkos:usedBy rdf:type owl:ObjectProperty ;
            rdfs:domain frbr:Expression ,
                        frbr:Work ;
            rdfs:range dcterms:AgentClass ;
            rdfs:comment "Agent using the described KOS."@en ;
            rdfs:label "used by"@en .


###  http://www.w3.org/2000/01/rdf-schema#seeAlso
rdfs:seeAlso rdf:type owl:ObjectProperty ;
             rdfs:domain rdfs:Resource ;
             rdfs:range rdfs:Resource ;
             rdfs:comment "rdfs:seeAlso is an instance of rdf:Property that is used to indicate a resource that might provide additional information about the subject resource."@en ;
             rdfs:label "see also"@en .


###  http://www.w3.org/ns/adms#identifier
adms:identifier rdf:type owl:ObjectProperty ;
                rdfs:domain adms:Asset ;
                rdfs:range adms:Identifier ;
                rdfs:comment "Links a resource to an adms:Identifier class."@en ;
                rdfs:label "identifier"@en .


###  http://www.w3.org/ns/adms#prev
adms:prev rdf:type owl:ObjectProperty ;
          rdfs:domain adms:Asset ;
          rdfs:range rdfs:Resource ;
          rdfs:comment "A link to the previous version of the Asset."@en ;
          rdfs:label "prev"@en .


###  http://www.w3.org/ns/adms#representationTechnique
adms:representationTechnique rdf:type owl:ObjectProperty ;
                             rdfs:domain adms:AssetDistribution ;
                             rdfs:range skos:Concept ;
                             rdfs:comment "More information about the format in which an Asset Distribution is released. This is different from the file format as, for example, a ZIP file (file format) could contain an XML schema (representation technique)."@en ;
                             rdfs:label "representation technique"@en .


###  http://www.w3.org/ns/adms#sample
adms:sample rdf:type owl:ObjectProperty ;
            rdfs:domain adms:Asset ;
            rdfs:range adms:Asset ;
            rdfs:comment "Links to a sample of an Asset (which is itself an Asset)."@en ;
            rdfs:label "sample"@en .


###  http://www.w3.org/ns/adms#status
adms:status rdf:type owl:ObjectProperty ;
            rdfs:domain [ rdf:type owl:Class ;
                          owl:unionOf ( adms:Asset
                                        adms:AssetDistribution
                                      )
                        ] ;
            rdfs:range skos:Concept ;
            rdfs:comment "The status of the Asset in the context of a particular workflow process."@en ;
            rdfs:label "status"@en .


###  http://www.w3.org/ns/adms#translation
adms:translation rdf:type owl:ObjectProperty ;
                 rdfs:domain adms:Asset ;
                 rdfs:range rdfs:Resource ;
                 rdfs:comment "Links Assets that are translations of each other."@en ;
                 rdfs:label "translation"@en .


###  http://www.w3.org/ns/dcat#accessSerive
dcat:accessSerive rdf:type owl:ObjectProperty ;
                                         rdfs:domain dcat:Distribution ;
                                         rdfs:range dcat:DataService ;
                                         rdfs:comment "A data service that gives access to the distribution of the dataset."@en ;
                                         rdfs:label "access service"@en .


###  http://www.w3.org/ns/dcat#accessService
dcat:accessService rdf:type owl:ObjectProperty ;
                                          rdfs:domain dcat:Distribution ;
                                          rdfs:range dcat:DataService ;
                                          rdfs:comment "A data service that gives access to the distribution of the dataset."@en ;
                                          rdfs:label "access service"@en .



###  http://www.w3.org/ns/dcat#compressFormat
dcat:compressFormat rdf:type owl:ObjectProperty ;
                                           rdfs:domain dcat:Distribution ;
                                           rdfs:range dcterms:MediaType ;
                                           rdfs:comment "The compression format of the distribution in which the data is contained in a compressed form, e.g. to reduce the size of the downloadable file."@en ,
                                                        "This property to be used when the files in the distribution are compressed, e.g. in a ZIP file. The format SHOULD be expressed using a media type as defined by IANA [IANA-MEDIA-TYPES], if available."@en ;
                                           rdfs:label "compression format"@en .


###  http://www.w3.org/ns/dcat#contactPoint
dcat:contactPoint rdf:type owl:ObjectProperty ;
                                         rdfs:domain dcat:Resource ;
                                         rdfs:range <http://www.w3.org/2006/vcard/ns#Kind> ;
                                         rdfs:comment "Relevant contact information for the cataloged resource. Use of vCard is recommended."@en ;
                                         rdfs:label "contact point"@en .


###  http://www.w3.org/ns/dcat#dataset
dcat:dataset rdf:type owl:ObjectProperty ;
                                    rdfs:domain dcat:Catalog ;
                                    rdfs:range dcat:Dataset ;
                                    rdfs:comment "A collection of data that is listed in the catalog."@en ;
                                    rdfs:label "dataset"@en .


###  http://www.w3.org/ns/dcat#distribution
dcat:distribution rdf:type owl:ObjectProperty ;
                                         rdfs:domain [ rdf:type owl:Class ;
                                                       owl:unionOf ( adms:Asset
                                                                     dcat:Dataset
                                                                   )
                                                     ] ;
                                         rdfs:range [ rdf:type owl:Class ;
                                                      owl:unionOf ( adms:AssetDistribution
                                                                    dcat:Distribution
                                                                  )
                                                    ] ;
                                         rdfs:comment "An available distribution of the dataset."@en ;
                                         rdfs:label "dataset distribution"@en .


###  http://www.w3.org/ns/dcat#downloadURL
dcat:downloadURL rdf:type owl:ObjectProperty ;
                                        rdfs:domain dcat:Distribution ;
                                        rdfs:range rdfs:Resource ;
                                        rdfs:comment "The URL of the downloadable file in a given format. E.g. CSV file or RDF file. The format is indicated by the distribution's dcterms:format and/or dcat:mediaType"@en ;
                                        rdfs:label "download URL"@en .




###  http://www.w3.org/ns/dcat#mediaType
dcat:mediaType rdf:type owl:ObjectProperty ;
                                      rdfs:subPropertyOf dcterms:format ;
                                      rdfs:domain dcat:Distribution ;
                                      rdfs:range dcterms:MediaType ;
                                      rdfs:comment "The media type of the distribution as defined by IANA [IANA-MEDIA-TYPES]."@en ;
                                      rdfs:label "media type"@en .


###  http://www.w3.org/ns/dcat#packageFormat
dcat:packageFormat rdf:type owl:ObjectProperty ;
                                          rdfs:domain dcat:Distribution ;
                                          rdfs:range dcterms:MediaType ;
                                          rdfs:comment "The package format of the distribution in which one or more data files are grouped together, e.g. to enable a set of related files to be downloaded together."@en ;
                                          rdfs:label "packaging format"@en .


###  http://www.w3.org/ns/dcat#record
dcat:record rdf:type owl:ObjectProperty ;
                                   rdfs:domain dcat:Catalog ;
                                   rdfs:range dcat:CatalogRecord ;
                                   rdfs:comment "A record describing the registration of a single resource (e.g., a dataset, a data service) that is part of the catalog."@en ;
                                   rdfs:label "catalog record"@en .


###  http://www.w3.org/ns/dcat#servesDataset
dcat:servesDataset rdf:type owl:ObjectProperty ;
                                          rdfs:range dcat:Dataset ;
                                          rdfs:comment "A collection of data that this data service can distribute."@en ;
                                          rdfs:label "serves dataset"@en .


###  http://www.w3.org/ns/dcat#service
dcat:service rdf:type owl:ObjectProperty ;
                                    rdfs:subPropertyOf dcterms:hasPart ;
                                    rdfs:domain dcat:Catalog ;
                                    rdfs:range dcat:DataService ;
                                    rdfs:comment "A site or end-point that is listed in the catalog."@en ;
                                    rdfs:label "service"@en .


###  http://www.w3.org/ns/dcat#theme
dcat:theme rdf:type owl:ObjectProperty ;
                                  rdfs:domain dcat:Resource ;
                                  rdfs:range skos:Concept ;
                                  rdfs:comment "A main category of the resource. A resource can have multiple themes."@en ;
                                  rdfs:label "theme"@en .


###  http://www.w3.org/ns/odrl/2/hasPolicy
odrl:hasPolicy rdf:type owl:ObjectProperty ;
               rdfs:domain [ rdf:type owl:Class ;
                             owl:unionOf ( dcat:Distribution
                                           dcat:Resource
                                         )
                           ] ;
               rdfs:range odrl:Policy ;
               rdfs:comment "Identifies an ODRL Policy for which the identified Asset is the target Asset to all the Rules."@en ;
               rdfs:label "has policy"@en .


###  http://www.w3.org/ns/prov#generalizationOf
prov:generalizationOf rdf:type owl:ObjectProperty ;
                      owl:inverseOf prov:specializationOf ;
                      rdfs:label "generalization of"@en .


###  http://www.w3.org/ns/prov#specializationOf
prov:specializationOf rdf:type owl:ObjectProperty ;
                      rdfs:domain prov:Entity ;
                      rdfs:range prov:Entity ;
                      rdfs:comment "An entity that is a specialization of another shares all aspects of the latter, and additionally presents more specific aspects of the same thing as the latter. In particular, the lifetime of the entity being specialized contains that of any specialization. Examples of aspects include a time period, an abstraction, and a context associated with the entity."@en ;
                      rdfs:label "specialization of"@en .


###  http://www.w3.org/ns/prov#wasAttributedTo
prov:wasAttributedTo rdf:type owl:ObjectProperty ;
                     rdfs:domain prov:Entity ;
                     rdfs:range prov:Agent ;
                     rdfs:comment "Attribution is the ascribing of an entity to an agent."@en ;
                     rdfs:label "was attributed to"@en .


###  http://www.w3.org/ns/prov#wasDerivedFrom
prov:wasDerivedFrom rdf:type owl:ObjectProperty ;
                    rdfs:domain prov:Entity ;
                    rdfs:range prov:Entity ;
                    rdfs:comment "A derivation is a transformation of an entity into another, an update of an entity resulting in a new one, or the construction of a new entity based on a pre-existing entity."@en ;
                    rdfs:label "was derived from"@en .


###  http://www.w3.org/ns/prov#wasGeneratedBy
prov:wasGeneratedBy rdf:type owl:ObjectProperty ;
                    rdfs:domain prov:Entity ;
                    rdfs:range prov:Activity ;
                    rdfs:comment "Generation is the completion of production of a new entity by an activity. This entity did not exist before generation and becomes available for usage after this generation."@en ;
                    rdfs:label "was generated by"@en .


###  http://www.w3.org/ns/prov#wasInfluencedBy
prov:wasInfluencedBy rdf:type owl:ObjectProperty ;
                     rdfs:domain prov:Entity ;
                     rdfs:range [ rdf:type owl:Class ;
                                  owl:unionOf ( prov:Activity
                                                prov:Entity
                                                foaf:Agent
                                              )
                                ] ;
                     rdfs:comment "Influence is the capacity of an entity, activity, or agent to have an effect on the character, development, or behavior of another by means of usage, start, end, generation, invalidation, communication, derivation, attribution, association, or delegation."@en ;
                     rdfs:label "was influenced by"@en .


###  http://www.w3.org/ns/prov#wasInvalidatedBy
prov:wasInvalidatedBy rdf:type owl:ObjectProperty ;
                      rdfs:domain prov:Entity ;
                      rdfs:range prov:Activity ;
                      rdfs:comment "Invalidation is the start of the destruction, cessation, or expiry of an existing entity by an activity. The entity is no longer available for use (or further invalidation) after invalidation. Any generation or usage of an entity precedes its invalidation."@en ;
                      rdfs:label "was invalidated by"@en .


###  http://www.w3.org/ns/prov#wasRevisionOf
prov:wasRevisionOf rdf:type owl:ObjectProperty ;
                   rdfs:domain prov:Entity ;
                   rdfs:range prov:Entity ;
                   rdfs:comment "A revision is a derivation for which the resulting entity is a revised version of some original. The implication here is that the resulting entity contains substantial content from the original. Revision is a particular case of derivation."@en ;
                   rdfs:label "was revision of"@en .


###  http://www.w3.org/ns/sparql-service-description#endpoint
sd:endpoint rdf:type owl:ObjectProperty ;
            rdfs:domain sd:Service ;
            rdfs:range rdfs:Resource ;
            rdfs:comment "Relates an instance of sd:Service to a SPARQL endpoint that implements the SPARQL Protocol service [SPROT] for the service. The object of the sd:endpoint property is an IRI."@en ;
            rdfs:label "endpoint"@en .


###  http://xmlns.com/foaf/0.1/fundedBy
foaf:fundedBy rdf:type owl:ObjectProperty ;
              rdfs:domain owl:Thing ;
              rdfs:range owl:Thing ;
              rdfs:comment "An organization funding a project or person."@en ;
              rdfs:label "funded by"@en .


###  http://xmlns.com/foaf/0.1/homepage
foaf:homepage rdf:type owl:ObjectProperty ;
              rdfs:subPropertyOf foaf:page ;
              rdfs:domain owl:Thing ;
              rdfs:range foaf:Document ;
              rdfs:comment "A homepage for some thing."@en ;
              rdfs:label "homepage"@en .


###  http://xmlns.com/foaf/0.1/isPrimaryTopicOf
foaf:isPrimaryTopicOf rdf:type owl:ObjectProperty ;
                      rdfs:subPropertyOf foaf:page ;
                      owl:inverseOf foaf:primaryTopic ;
                      rdf:type owl:InverseFunctionalProperty ;
                      rdfs:domain foaf:Document ;
                      rdfs:range foaf:Document ;
                      rdfs:comment "A document that this thing is the primary topic of."@en ;
                      rdfs:label "is primary topic of"@en .


###  http://xmlns.com/foaf/0.1/logo
foaf:logo rdf:type owl:ObjectProperty ;
          rdfs:domain owl:Thing ;
          rdfs:range owl:Thing ;
          rdfs:comment "A logo representing some thing."@en ;
          rdfs:label "logo"@en .


###  http://xmlns.com/foaf/0.1/maker
foaf:maker rdf:type owl:ObjectProperty ;
           rdfs:domain owl:Thing ;
           rdfs:range foaf:Agent ;
           rdfs:comment "An agent that made this thing."@en ;
           rdfs:label "maker"@en .





###  http://xmlns.com/foaf/0.1/primaryTopic
foaf:primaryTopic rdf:type owl:ObjectProperty ;
                  rdfs:subPropertyOf foaf:page ;
                  rdf:type owl:FunctionalProperty ;
                  rdfs:domain [ rdf:type owl:Class ;
                                owl:unionOf ( dcat:CatalogRecord
                                              foaf:Document
                                            )
                              ] ;
                  rdfs:range [ rdf:type owl:Class ;
                               owl:unionOf ( owl:Thing
                                             dcat:Resource
                                           )
                             ] ;
                  rdfs:comment "A page or document about this thing."@en ;
                  rdfs:label "primary topic"@en .


###  http://xmlns.com/foaf/0.1/topic
foaf:topic rdf:type owl:ObjectProperty ;
           rdfs:domain foaf:Document ;
           rdfs:range owl:Thing ;
           rdfs:comment "A topic of some page or document."@en ;
           rdfs:label "topic"@en .


###  https://w3id.org/mod#analytics
mod:analytics rdf:type owl:ObjectProperty ;
           rdfs:domain :SemanticArtefact ;
           rdfs:range :Analytics ;
           rdfs:comment "This property shall be used to store any analytics for an ontology. E.g., number of visits an ontology received in a portal, number of downloads, etc."@en ;
           rdfs:isDefinedBy "https://www.isibang.ac.in/ns/mod/1.4/"@en ;
           rdfs:label "analytics"@en .


###  https://w3id.org/mod#comesFromTheSameDomain
mod:comesFromTheSameDomain rdf:type owl:ObjectProperty ;
                        rdfs:subPropertyOf :semanticArtefactRelation ;
                        rdfs:domain :SemanticArtefact ;
                        rdfs:range :SemanticArtefact ;
                        rdfs:comment "If the two ontologies come from the same domain (without any other details)."@en ;
                        rdfs:label "comes from the same domain"@en .


###  https://w3id.org/mod#conformsToKnowledgeRepresentationParadigm
mod:conformsToKnowledgeRepresentationParadigm rdf:type owl:ObjectProperty ;
                                           rdfs:domain :SemanticArtefact ;
                                           rdfs:range :KnowledgeRepresentationParadigm ;
                                           rdfs:comment "A representation formalism that is followed to describe knowledge in an ontology. Example includes description logics, first order logic, etc. dcterms: An established standard to which the described resource conforms."@en ;
                                           rdfs:label "conforms to knowledge representation paradigm"@en ;
                                           skos:historyNote "This property has been adopted from OMV Ontology Metadata Vocabulary and redefined in the MOD namespace."@en .


###  https://w3id.org/mod#depiction
mod:depiction rdf:type owl:ObjectProperty ;
           rdfs:domain owl:Thing ;
           rdfs:range foaf:Image ;
           rdfs:comment "A depiction of some thing."@en ;
           rdfs:label "depiction"@en .


###  https://w3id.org/mod#describes
mod:describes rdf:type owl:ObjectProperty ;
           rdfs:domain :SemanticArtefact ;
           rdfs:range dcat:Dataset .


###  https://w3id.org/mod#designedForTask
mod:designedForTask rdf:type owl:ObjectProperty ;
                 rdfs:domain :SemanticArtefact ;
                 rdfs:range :SemanticArtefactTask ;
                 rdfs:label "designed for task"@en .


###  https://w3id.org/mod#endorsedBy
mod:endorsedBy rdf:type owl:ObjectProperty ;
            rdfs:domain :SemanticArtefact ;
            rdfs:range dcterms:Agent ;
            rdfs:comment "An ontology endorsed by an agent."@en ;
            rdfs:label "endorsed by"@en .


###  https://w3id.org/mod#generalizes
mod:generalizes rdf:type owl:ObjectProperty ;
             rdfs:subPropertyOf :semanticArtefactRelation ;
             owl:inverseOf :specializes ;
             rdfs:comment "Indicates that the subject vocabulary generalizes by some superclasses or superproperties the object vocabulary."@en ;
             rdfs:label "generalizes"@en .


###  https://w3id.org/mod#group
mod:group rdf:type owl:ObjectProperty ;
       rdfs:domain :SemanticArtefact ;
       rdfs:range :Group ;
       rdfs:comment "A group of ontologies that the ontology is usually considered into."@en ;
       rdfs:label "group"@en .


###  https://w3id.org/mod#hasDisjunctionsWith
mod:hasDisjunctionsWith rdf:type owl:ObjectProperty ;
                     rdfs:subPropertyOf :semanticArtefactRelation ;
                     rdfs:comment "Indicates that the subject vocabulary declares some disjunct classes with the object vocabulary."@en ;
                     rdfs:label "has disjunctions with"@en .


###  https://w3id.org/mod#hasDisparateModellingWith
mod:hasDisparateModellingWith rdf:type owl:ObjectProperty ;
                           rdfs:subPropertyOf :semanticArtefactRelation ;
                           rdfs:comment "Disagreements related  to  the  conceptualization  of  the  ontologies. Two ontologies are considered to have disparate modeling if they represent corresponding entities in different ways, e.g.  as an instance in one case and a class in the other."@en ;
                           rdfs:label "disparate modelling with"@en .


###  https://w3id.org/mod#hasEquivalencesWith
mod:hasEquivalencesWith rdf:type owl:ObjectProperty ;
                     rdfs:subPropertyOf :semanticArtefactRelation ;
                     rdfs:domain :SemanticArtefact ;
                     rdfs:range :SemanticArtefact ;
                     rdfs:comment "Indicates that the subject vocabulary declares some equivalent classes or properties with the object vocabulary."@en ;
                     rdfs:label "ontology aligned to"@en .


###  https://w3id.org/mod#hasEvaluation
mod:hasEvaluation rdf:type owl:ObjectProperty ;
               rdfs:domain :SemanticArtefact ;
               rdfs:range :Evaluation ;
               rdfs:comment "This property makes a relationship between an ontology and its evaluation result."@en ;
               rdfs:label "has evaluation"@en .


###  https://w3id.org/mod#metadataVoc
mod:metadataVoc rdf:type owl:ObjectProperty ;
             rdfs:subPropertyOf :semanticArtefactRelation ;
             rdfs:comment "Indicates that the subject vocabulary uses the object vocabulary in metadata at vocabulary or element level."@en ;
             rdfs:label "metadata vocubulary used"@en .


###  https://w3id.org/mod#qualifiedRelation
mod:qualifiedRelation rdf:type owl:ObjectProperty ;
                   rdfs:domain dcat:Resource ;
                   rdfs:range dcat:Relationship ;
                   rdfs:comment "Link to a description of a relationship with another resource."@en ;
                   rdfs:label "qualified relation"@en .


###  https://w3id.org/mod#semanticArtefactRelation
mod:semanticArtefactRelation rdf:type owl:ObjectProperty ;
                          rdfs:domain :SemanticArtefact ;
                          rdfs:range :SemanticArtefact .


###  https://w3id.org/mod#similar
mod:similar rdf:type owl:ObjectProperty ;
         rdfs:subPropertyOf :semanticArtefactRelation ;
         rdfs:domain :SemanticArtefact ;
         rdfs:range :SemanticArtefact ;
         rdfs:comment "Used to assert that two vocabularies are similar in scope and objectives, independently of the fact that they otherwise refer to each other."@en ;
         rdfs:label "similar to"@en .


###  https://w3id.org/mod#specializes
mod:specializes rdf:type owl:ObjectProperty ;
             rdfs:subPropertyOf :semanticArtefactRelation ;
             rdfs:comment "An entity that is a specialization of another shares all aspects of the latter, and additionally presents more specific aspects of the same thing as the latter. voaf:Indicates that the subject vocabulary defines some subclasses or subproperties of the object vocabulary, or local restrictions on those."@en ;
             rdfs:label "specializes"@en .


###  https://w3id.org/mod#usedBy
mod:usedBy rdf:type owl:ObjectProperty ;
        rdfs:subPropertyOf :semanticArtefactRelation ;
        rdfs:comment "Indicates that the subject vocabulary is used by the object vocabulary."@en ;
        rdfs:label "used by"@en .


###  https://w3id.org/mod#usedEngineeringMethodology
mod:usedEngineeringMethodology rdf:type owl:ObjectProperty ;
                            rdfs:domain :SemanticArtefact ;
                            rdfs:range :EngineeringMethodology ;
                            rdfs:label "used engineering methodology"@en ;
                            skos:historyNote "This property has been adopted from OMV Ontology Metadata Vocabulary, and renamed and redefined in the MOD namespace."@en .


###  https://w3id.org/mod#usedInProject
mod:usedInProject rdf:type owl:ObjectProperty ;
               rdfs:domain :SemanticArtefact ;
               rdfs:range foaf:Project ;
               rdfs:comment "An semantic artefact that is used in a project."@en ;
               rdfs:label "used in project"@en .


#################################################################
#    Data properties
#################################################################

###  http://creativecommons.org/ns#attributionName
cc:attributionName rdf:type owl:DatatypeProperty ;
                   rdfs:comment "The name the creator of a Work would like used when attributing re-use."@en ;
                   rdfs:label "attribution name"@en .


###  http://identifiers.org/idot/alternatePrefix
idot:alternatePrefix rdf:type owl:DatatypeProperty ;
                     rdfs:domain dcmi:Dataset ;
                     rdfs:range xsd:string ;
                     rdfs:label "alternate prefix"@en .


###  http://identifiers.org/idot/exampleIdentifier
idot:exampleIdentifier rdf:type owl:DatatypeProperty ;
                       rdfs:domain dcmi:Dataset ;
                       rdfs:range xsd:string ;
                       rdfs:label "example identifier"@en .


###  http://identifiers.org/idot/identifierPattern
idot:identifierPattern rdf:type owl:DatatypeProperty ;
                       rdfs:domain dcmi:Dataset ;
                       rdfs:range xsd:string ;
                       rdfs:label "identifier pattern"@en .


###  http://identifiers.org/idot/obsolete
idot:obsolete rdf:type owl:DatatypeProperty ;
              rdfs:domain dcmi:Dataset ;
              rdfs:range xsd:string ;
              rdfs:label "obsolete"@en .


###  http://identifiers.org/idot/preferredPrefix
idot:preferredPrefix rdf:type owl:DatatypeProperty ;
                     rdfs:domain dcmi:Dataset ;
                     rdfs:range xsd:string ;
                     rdfs:label "preferred prefix"@en .


###  http://identifiers.org/idot/state
idot:state rdf:type owl:DatatypeProperty ;
           rdfs:domain dcmi:Dataset ;
           rdfs:range xsd:string ;
           rdfs:label "state"@en .








###  http://purl.org/dc/terms/created
dcterms:created rdf:type owl:DatatypeProperty ;
            rdfs:subPropertyOf dcterms:date ;
            rdfs:range rdfs:Literal ;
            rdfs:comment "Date of creation of the resource."@en ;
            rdfs:label "created"@en ,
                       "date created"@en .


###  http://purl.org/dc/terms/date
dcterms:date rdf:type owl:DatatypeProperty ;
         rdfs:range rdfs:Literal ;
         rdfs:comment "A point or period of time associated with an event in the lifecycle of the resource."@en ;
         rdfs:label "date"@en .


###  http://purl.org/dc/terms/dateSubmitted
dcterms:dateSubmitted rdf:type owl:DatatypeProperty ;
                  rdfs:subPropertyOf dcterms:date ;
                  rdfs:range rdfs:Literal ;
                  rdfs:comment "Date of submission of the resource."@en ;
                  rdfs:label "date submitted"@en .




###  http://purl.org/dc/terms/identifier
dcterms:identifier rdf:type owl:DatatypeProperty ;
               rdfs:range rdfs:Literal ;
               rdfs:comment "An unambiguous reference to the resource within a given context."@en ;
               rdfs:label "identifier"@en .


###  http://purl.org/dc/terms/issued
dcterms:issued rdf:type owl:DatatypeProperty ;
           rdfs:subPropertyOf dcterms:date ;
           rdfs:range rdfs:Literal ;
           rdfs:comment "Date of formal issuance of the resource."@en ;
           rdfs:label "date issued"@en ,
                      "issued"@en .


###  http://purl.org/dc/terms/modified
dcterms:modified rdf:type owl:DatatypeProperty ;
             rdfs:subPropertyOf dcterms:date ;
             rdfs:range rdfs:Literal ;
             rdfs:comment "Date on which the resource was changed."@en ;
             rdfs:label "Date modified"@en .


###  http://purl.org/dc/terms/subject
dcterms:subject rdf:type owl:DatatypeProperty ;
            rdfs:comment "A topic of the resource."@en ;
            rdfs:label "subject"@en .


###  http://purl.org/dc/terms/title
dcterms:title rdf:type owl:DatatypeProperty ;
          rdfs:range rdfs:Literal ;
          rdfs:comment "A name given to the resource."@en ;
          rdfs:label "title"@en .


###  http://purl.org/dc/terms/valid
dcterms:valid rdf:type owl:DatatypeProperty ;
          rdfs:subPropertyOf dcterms:date ;
          rdfs:range rdfs:Literal ;
          rdfs:comment "Date (often a range) of validity of a resource."@en ;
          rdfs:label "valid"@en .


###  http://purl.org/pav/authoredOn
pav:authoredOn rdf:type owl:DatatypeProperty ;
               rdfs:subPropertyOf pav:contributedOn ;
               rdfs:range xsd:dateTime ;
               rdfs:comment "The date this resource was authored."@en ;
               rdfs:label "authored on"@en .


###  http://purl.org/pav/contributedOn
pav:contributedOn rdf:type owl:DatatypeProperty ;
                  rdfs:range xsd:dateTime ;
                  rdfs:comment "The date this resource was contributed to."@en ;
                  rdfs:label "contributed on"@en .


###  http://purl.org/pav/createdOn
pav:createdOn rdf:type owl:DatatypeProperty ;
              rdfs:range xsd:dateTime ;
              rdfs:comment "The date of creation of the resource representation."@en ;
              rdfs:label "created on"@en .


###  http://purl.org/pav/curatedOn
pav:curatedOn rdf:type owl:DatatypeProperty ;
              rdfs:subPropertyOf pav:contributedOn ;
              rdfs:range xsd:dateTime ;
              rdfs:comment "The date this resource was curated."@en ;
              rdfs:label "curated on"@en .


###  http://purl.org/pav/lastUpdateOn
pav:lastUpdateOn rdf:type owl:DatatypeProperty ;
                 rdfs:range xsd:dateTime ;
                 rdfs:comment "The date of the last update of the resource. An update is a change which did not warrant making a new resource related using pav:previousVersion, for instance correcting a spelling mistake."@en ;
                 rdfs:label "last update on"@en .


###  http://purl.org/pav/version
pav:version rdf:type owl:DatatypeProperty ;
            rdfs:domain prov:Entity ;
            rdfs:range xsd:string ;
            rdfs:comment "The version number of a resource. This is a freetext string, typical values are \"1.5\" or \"21\". The URI identifying the previous version can be provided using prov:previousVersion."@en ;
            rdfs:label "version"@en .


###  http://rdfs.org/ns/void#classes
void:classes rdf:type owl:DatatypeProperty ;
             rdfs:domain void:Dataset ;
             rdfs:range xsd:integer ;
             rdfs:comment "The total number of distinct classes in a void:Dataset. In other words, the number of distinct resources occuring as objects of rdf:type triples in the dataset."@en ;
             rdfs:label "classes"@en .


###  http://rdfs.org/ns/void#entities
void:entities rdf:type owl:DatatypeProperty ;
              rdfs:domain void:Dataset ;
              rdfs:range xsd:integer ;
              rdfs:comment "The total number of entities that are described in a void:Dataset."@en ;
              rdfs:label "entities"@en .


###  http://rdfs.org/ns/void#properties
void:properties rdf:type owl:DatatypeProperty ;
                rdfs:domain void:Dataset ;
                rdfs:range xsd:integer ;
                rdfs:comment "The total number of distinct properties in a void:Dataset. In other words, the number of distinct resources that occur in the predicate position of triples in the dataset."@en ;
                rdfs:label "properties"@en .


###  http://rdfs.org/ns/void#triples
void:triples rdf:type owl:DatatypeProperty ;
             rdfs:domain void:Dataset ;
             rdfs:range xsd:integer ;
             rdfs:comment "The total number of triples contained in a void:Dataset."@en ;
             rdfs:label "triples"@en .


###  http://rdfs.org/ns/void#uriRegexPattern
void:uriRegexPattern rdf:type owl:DatatypeProperty ;
                     rdfs:domain void:Dataset ;
                     rdfs:range xsd:string ;
                     rdfs:comment "A regular expression that matches the URIs of a void:Dataset's entities."@en ;
                     rdfs:label "uri regex pattern"@en .


###  http://rdfs.org/ns/void#uriSpace
void:uriSpace rdf:type owl:DatatypeProperty ;
              rdfs:domain void:Dataset ;
              rdfs:range xsd:string ;
              rdfs:comment "A URI that is a common string prefix of all the entity URIs in a void:Datset."@en ,
                           "The void:uriSpace property can be used to state that all entity URIs in a dataset start with a given string. In other words, they share a common “URI namespace”."@en ;
              rdfs:label "uri space"@en .


###  http://schema.org/award
schema:award rdf:type owl:DatatypeProperty ;
                          rdfs:range schema:Text ;
                          rdfs:comment "An award won by or for this item."@en ;
                          rdfs:label "award"@en .


###  http://schema.org/dateCreated
schema:dateCreated rdf:type owl:DatatypeProperty ;
                                rdfs:range schema:DateTime ;
                                rdfs:comment "The date on which the CreativeWork was created or the item was added to a DataFeed."@en ;
                                rdfs:label "date created"@en .


###  http://schema.org/dateModified
schema:dateModified rdf:type owl:DatatypeProperty ;
                                 rdfs:range schema:DateTime ;
                                 rdfs:comment "The date on which the CreativeWork was most recently modified or when the item's entry was modified within a DataFeed."@en ;
                                 rdfs:label "date modified"@en .


###  http://schema.org/datePublished
schema:datePublished rdf:type owl:DatatypeProperty ;
                                  rdfs:domain schema:CreativeWork ;
                                  rdfs:range [ rdf:type rdfs:Datatype ;
                                               owl:unionOf ( schema:Date
                                                             schema:DateTime
                                                           )
                                             ] ;
                                  rdfs:comment "Date of first broadcast/publication."@en ;
                                  rdfs:label "date published"@en .


###  http://schema.org/description
schema:description rdf:type owl:DatatypeProperty ;
                                rdfs:range schema:Text ;
                                rdfs:comment "A description of the item."@en ;
                                rdfs:label "description"@en .


###  http://schema.org/fileFormat
schema:fileFormat rdf:type owl:DatatypeProperty ;
                               rdfs:domain schema:CreativeWork ;
                               rdfs:range [ rdf:type rdfs:Datatype ;
                                            owl:unionOf ( schema:Text
                                                          schema:URL
                                                        )
                                          ] ;
                               rdfs:comment "Media type, typically MIME format (see IANA site) of the content e.g. application/zip of a SoftwareApplication binary. In cases where a CreativeWork has several media type representations, 'encoding' can be used to indicate each MediaObject alongside particular fileFormat information. Unregistered or niche file formats can be indicated instead via the most appropriate URL, e.g. defining Web page or a Wikipedia entry."@en ;
                               rdfs:label "file format"@en .


###  http://schema.org/image
schema:image rdf:type owl:DatatypeProperty ;
                          rdfs:range schema:URL ;
                          rdfs:comment "An image of the item. This can be a URL or a fully described ImageObject."@en ;
                          rdfs:label "image"@en .


###  http://schema.org/inLanguage
schema:inLanguage rdf:type owl:DatatypeProperty ;
                               rdfs:domain schema:CreativeWork ;
                               rdfs:range schema:Text ;
                               rdfs:comment "The language of the content or performance or used in an action. Please use one of the language codes from the IETF BCP 47 standard. See also availableLanguage."@en ;
                               rdfs:label "in language"@en .


###  http://schema.org/keywords
schema:keywords rdf:type owl:DatatypeProperty ;
                             rdfs:domain schema:CreativeWork ;
                             rdfs:range [ rdf:type rdfs:Datatype ;
                                          owl:unionOf ( schema:Text
                                                        schema:URL
                                                      )
                                        ] ;
                             rdfs:comment "Keywords or tags used to describe this content. Multiple entries in a keywords list are typically delimited by commas."@en ;
                             rdfs:label "keywords"@en .


###  http://schema.org/logo
schema:logo rdf:type owl:DatatypeProperty ;
                         rdfs:range schema:URL ;
                         rdfs:comment "An associated logo."@en ;
                         rdfs:label "logo"@en .


###  http://schema.org/mainEntityOfPage
schema:mainEntityOfPage rdf:type owl:DatatypeProperty ;
                                     rdfs:range schema:URL ;
                                     rdfs:comment "Indicates a page (or other CreativeWork) for which this thing is the main entity being described. See background notes for details."@en ;
                                     rdfs:label "main entity of page"@en .


###  http://schema.org/name
schema:name rdf:type owl:DatatypeProperty ;
                         rdfs:range schema:Text ;
                         rdfs:comment "The name of the item."@en ;
                         rdfs:label "name"@en .


###  http://schema.org/publishingPrinciples
schema:publishingPrinciples rdf:type owl:DatatypeProperty ;
                                         rdfs:domain schema:CreativeWork ;
                                         rdfs:comment """The publishingPrinciples property indicates (typically via URL) a document describing the editorial principles of an Organization (or individual e.g. a Person writing a blog) that relate to their activities as a publisher, e.g. ethics or diversity policies. When applied to a CreativeWork (e.g. NewsArticle) the principles are those of the party primarily responsible for the creation of the CreativeWork.

While such policies are most typically expressed in natural language, sometimes related information (e.g. indicating a funder) can be expressed using schema.org terminology."""@en ;
                                         rdfs:label "publishing principles"@en .


###  http://schema.org/schemaVersion
schema:schemaVersion rdf:type owl:DatatypeProperty ;
                                  rdfs:domain schema:CreativeWork ;
                                  rdfs:range [ rdf:type rdfs:Datatype ;
                                               owl:unionOf ( schema:Text
                                                             schema:URL
                                                           )
                                             ] ;
                                  rdfs:comment "Indicates (by URL or string) a particular version of a schema used in some CreativeWork. This property was created primarily to indicate the use of a specific schema.org release, e.g. 10.0 as a simple string, or more explicitly via URL, https://schema.org/docs/releases.html#v10.0. There may be situations in which other schemas might usefully be referenced this way, e.g. http://dublincore.org/specifications/dublin-core/dces/1999-07-02/ but this has not been carefully explored in the community."@en ;
                                  rdfs:label "schema version"@en .


###  http://schema.org/temporalCoverage
schema:temporalCoverage rdf:type owl:DatatypeProperty ;
                                     rdfs:domain schema:CreativeWork ;
                                     rdfs:range [ rdf:type rdfs:Datatype ;
                                                  owl:unionOf ( schema:DateTime
                                                                schema:Text
                                                                schema:URL
                                                              )
                                                ] ;
                                     rdfs:comment """The temporalCoverage of a CreativeWork indicates the period that the content applies to, i.e. that it describes, either as a DateTime or as a textual string indicating a time period in ISO 8601 time interval format. In the case of a Dataset it will typically indicate the relevant time period in a precise notation (e.g. for a 2011 census dataset, the year 2011 would be written \"2011/2012\"). Other forms of content e.g. ScholarlyArticle, Book, TVSeries or TVEpisode may indicate their temporalCoverage in broader terms - textually or via well-known URL. Written works such as books may sometimes have precise temporal coverage too, e.g. a work set in 1939 - 1945 can be indicated in ISO 8601 interval format format via \"1939/1945\".

Open-ended date ranges can be written with \"..\" in place of the end date. For example, \"2015-11/..\" indicates a range beginning in November 2015 and with no specified final date. This is tentative and might be updated in future when ISO 8601 is officially updated."""@en ;
                                     rdfs:label "temporal coverage"@en .


###  http://schema.org/version
schema:version rdf:type owl:DatatypeProperty ;
                            rdfs:domain schema:CreativeWork ;
                            rdfs:range [ rdf:type rdfs:Datatype ;
                                         owl:unionOf ( schema:Number
                                                       schema:Text
                                                     )
                                       ] ;
                            rdfs:comment "The version of the CreativeWork embodied by a specified resource."@en ;
                            rdfs:label "version"@en .


###  http://usefulinc.com/ns/doap#audience
doap:audience rdf:type owl:DatatypeProperty ;
              rdfs:domain doap:Project ;
              rdfs:range rdfs:Literal ;
              rdfs:comment "Description of target user base."@en ;
              rdfs:label "audience"@en .


###  http://usefulinc.com/ns/doap#created
doap:created rdf:type owl:DatatypeProperty ;
             rdfs:domain doap:Project ;
             rdfs:range rdfs:Literal ;
             rdfs:comment "Date when something was created, in YYYY-MM-DD form. e.g. 2004-04-05."@en ;
             rdfs:label "created"@en .


###  http://usefulinc.com/ns/doap#description
doap:description rdf:type owl:DatatypeProperty ;
                 rdfs:domain doap:Project ;
                 rdfs:range rdfs:Literal ;
                 rdfs:comment "Plain text description of a project, of 2-4 sentences in length."@en ;
                 rdfs:label "description"@en .


###  http://usefulinc.com/ns/doap#language
doap:language rdf:type owl:DatatypeProperty ;
              rdfs:domain doap:Project ;
              rdfs:range rdfs:Literal ;
              rdfs:comment "ISO language code a project has been translated into."@en ;
              rdfs:label "language"@en .


###  http://w3id.org/nkos#updateFrequency
nkos:updateFrequency rdf:type owl:DatatypeProperty ;
                     rdfs:domain frbr:Expression ;
                     rdfs:range rdfs:Literal ;
                     rdfs:comment "The period in which a KOS is typically updated."@en ;
                     rdfs:label "update frequency"@en .


###  http://www.geneontology.org/formats/oboInOwl#autoGeneratedBy
oboinowl:autoGeneratedBy rdf:type owl:DatatypeProperty ;
                         rdfs:label "auto-generated by"@en .


###  http://www.geneontology.org/formats/oboInOwl#hasDate
oboinowl:hasDate rdf:type owl:DatatypeProperty ;
                 rdfs:label "has date"@en .


###  http://www.geneontology.org/formats/oboInOwl#hasDefaultNamespace
oboinowl:hasDefaultNamespace rdf:type owl:DatatypeProperty ;
                             rdfs:label "has default namespace"@en .


###  http://www.geneontology.org/formats/oboInOwl#hasSubset
oboinowl:hasSubset rdf:type owl:DatatypeProperty ;
                   rdfs:label "has subset"@en .


###  http://www.geneontology.org/formats/oboInOwl#hasSynonymType
oboinowl:hasSynonymType rdf:type owl:DatatypeProperty ;
                        rdfs:label "has synonym type"@en .


###  http://www.geneontology.org/formats/oboInOwl#hasVersion
oboinowl:hasVersion rdf:type owl:DatatypeProperty ;
                    rdfs:label "has version"@en .


###  http://www.geneontology.org/formats/oboInOwl#savedBy
oboinowl:savedBy rdf:type owl:DatatypeProperty ;
                 rdfs:label "saved by"@en .




###  http://www.w3.org/2004/02/skos/core#altLabel
skos:altLabel rdf:type owl:DatatypeProperty ;
              rdfs:domain :SemanticArtefact ;
              rdfs:range rdfs:Literal ;
              rdfs:comment "An alternative lexical label for a resource."@en ;
              rdfs:label "alternative label"@en .




###  http://www.w3.org/2004/02/skos/core#prefLabel
skos:prefLabel rdf:type owl:DatatypeProperty ;
               rdfs:domain :SemanticArtefact ;
               rdfs:range rdfs:Literal ;
               rdfs:comment "The preferred lexical label for a resource, in a given language."@en ;
               rdfs:label "pref label"@en ,
                          "preferred label"@en .


###  http://www.w3.org/ns/adms#versionNotes
adms:versionNotes rdf:type owl:DatatypeProperty ;
                  rdfs:domain adms:Asset ;
                  rdfs:range rdfs:Literal ;
                  rdfs:comment "A description of changes between this version and the previous version of the Asset."@en ;
                  rdfs:label "version notes"@en .


###  http://www.w3.org/ns/dcat#byteSize
dcat:byteSize rdf:type owl:DatatypeProperty ;
                                     rdfs:domain dcat:Distribution ;
                                     rdfs:range xsd:nonNegativeInteger ;
                                     rdfs:comment "The size in bytes can be approximated (as a decimal) when the precise size is not known."@en ,
                                                  "The size of a distribution in bytes."@en ;
                                     rdfs:label "byte size"@en .



###  http://www.w3.org/ns/dcat#spatialResolutionInMeters
dcat:spatialResolutionInMeters rdf:type owl:DatatypeProperty ;
                                                      rdfs:domain [ rdf:type owl:Class ;
                                                                    owl:unionOf ( dcat:Dataset
                                                                                  dcat:Distribution
                                                                                )
                                                                  ] ;
                                                      rdfs:range xsd:decimal ;
                                                      rdfs:comment "Minimum spatial separation resolvable in a dataset, measured in meters."@en ;
                                                      rdfs:label "spatial resolution in meters"@en .


###  http://www.w3.org/ns/dcat#temporalResolution
dcat:temporalResolution rdf:type owl:DatatypeProperty ;
                                               rdfs:domain [ rdf:type owl:Class ;
                                                             owl:unionOf ( dcat:Dataset
                                                                           dcat:Distribution
                                                                         )
                                                           ] ;
                                               rdfs:comment "Minimum time period resolvable in the dataset."@en ;
                                               rdfs:label "temporal resolution"@en .


###  http://www.w3.org/ns/prov#generatedAtTime
prov:generatedAtTime rdf:type owl:DatatypeProperty ;
                     rdfs:domain prov:Entity ;
                     rdfs:range schema:DateTime ;
                     rdfs:comment "Generation is the completion of production of a new entity by an activity. This entity did not exist before generation and becomes available for usage after this generation."@en ;
                     rdfs:label "generated at time"@en .


###  http://www.w3.org/ns/prov#invalidatedAtTime
prov:invalidatedAtTime rdf:type owl:DatatypeProperty ;
                       rdfs:domain prov:Entity ;
                       rdfs:range schema:DateTime ;
                       rdfs:comment "Invalidation is the start of the destruction, cessation, or expiry of an existing entity by an activity. The entity is no longer available for use (or further invalidation) after invalidation. Any generation or usage of an entity precedes its invalidation."@en ;
                       rdfs:label "invalidated at time"@en .


###  http://xmlns.com/foaf/0.1/name
foaf:name rdf:type owl:DatatypeProperty ;
          rdfs:domain foaf:Document ;
          rdfs:range xsd:string ;
          rdfs:comment "A name for some thing."@en ;
          rdfs:label "name"@en .


###  https://schema.org/alternateName
schema:alternateName rdf:type owl:DatatypeProperty ;
                     rdfs:range schema:Text ;
                     rdfs:comment "An alias for the item."@en ;
                     rdfs:label "alternate name"@en .


###  https://vocab.org/vann/changes
vann:changes rdf:type owl:DatatypeProperty ;
             rdfs:comment "A reference to a resource that describes changes between this version of a vocabulary and the previous."@en ;
             rdfs:label "changes"@en .


###  https://vocab.org/vann/example
vann:example rdf:type owl:DatatypeProperty ;
             rdfs:comment "A reference to a resource that provides an example of how this resource can be used."@en ;
             rdfs:label "example"@en .


###  https://vocab.org/vann/preferredNamespacePrefix
vann:preferredNamespacePrefix rdf:type owl:DatatypeProperty ;
                              rdfs:comment "The preferred namespace prefix to use when using terms from this vocabulary in an XML document."@en ;
                              rdfs:label "preferred namespace prefix"@en .


###  https://vocab.org/vann/preferredNamespaceUri
vann:preferredNamespaceUri rdf:type owl:DatatypeProperty ;
                           rdfs:comment "The preferred namespace URI to use when using terms from this vocabulary in an XML document."@en ;
                           rdfs:label "preferred namespace uri"@en .


###  https://vocab.org/vann/usageNote
vann:usageNote rdf:type owl:DatatypeProperty ;
               rdfs:comment "A reference to a resource that provides information on how this resource is to be used."@en ;
               rdfs:label "usage note"@en .




###  https://w3id.org/mod#authorProperty
mod:authorProperty rdf:type owl:DatatypeProperty ;
                rdfs:range xsd:anyURI ;
                rdfs:comment "property used to specify the author of a class (BioPortal definition)."@en ;
                rdfs:label "object author property"@en .


###  https://w3id.org/mod#averageChildCount
mod:averageChildCount rdf:type owl:DatatypeProperty ;
                   rdfs:subPropertyOf :metrics ;
                   rdfs:range xsd:nonNegativeInteger ;
                   rdfs:comment "Average number of children per class (BioPortal definition) ."@en ;
                   rdfs:label "average number of children per class"@en .


###  https://w3id.org/mod#browsingUI
mod:browsingUI rdf:type owl:DatatypeProperty ;
            rdfs:domain :SemanticArtefact ;
            rdfs:range xsd:anyURI ;
            rdfs:comment "The user interface (URL) where the ontology may be browsed or searched."@en ;
            rdfs:label "Browsing user interface"@en ,
                       "browsing UI"@en .


###  https://w3id.org/mod#classesWithMoreThan25Children
mod:classesWithMoreThan25Children rdf:type owl:DatatypeProperty ;
                               rdfs:subPropertyOf :metrics ;
                               rdfs:range xsd:nonNegativeInteger ;
                               rdfs:comment "Number of classes that have more than 25 direct subclasses (BioPortal definition)."@en ;
                               rdfs:label "number of classes with more than 25 children"@en .


###  https://w3id.org/mod#classesWithNoDefinition
mod:classesWithNoDefinition rdf:type owl:DatatypeProperty ;
                         rdfs:subPropertyOf :metrics ;
                         rdfs:range xsd:nonNegativeInteger ;
                         rdfs:comment "List of classes that have no value for the definition property (BioPortal definition). For ontologies in OBO and RRF formats, the property for definition is part of the language. For OWL ontologies, the authors specify this property as part of the ontology metadata (the default is skos:definition)."@en ;
                         rdfs:label "number of classes with no definition"@en .


###  https://w3id.org/mod#classesWithOneChild
mod:classesWithOneChild rdf:type owl:DatatypeProperty ;
                     rdfs:subPropertyOf :metrics ;
                     rdfs:range xsd:nonNegativeInteger ;
                     rdfs:comment "Number of classes that have only one subclass in the is-a hierarchy (BioPortal definition)."@en ;
                     rdfs:label "number of classes with a single child"@en .


###  https://w3id.org/mod#competencyQuestion
mod:competencyQuestion rdf:type owl:DatatypeProperty ;
                    rdfs:domain :SemanticArtefact ;
                    rdfs:range xsd:string ;
                    rdfs:comment "A set of questions made to build an ontology at the design time."@en ;
                    rdfs:label "competency question"@en .


###  https://w3id.org/mod#definitionProperty
mod:definitionProperty rdf:type owl:DatatypeProperty ;
                    rdfs:domain :SemanticArtefactDistribution ;
                    rdfs:range xsd:anyURI ;
                    rdfs:comment "Property used to specify the definition of a class (BioPortal definition)."@en ;
                    rdfs:label "object definition property"@en .








###  https://w3id.org/mod#hierarchyProperty
mod:hierarchyProperty rdf:type owl:DatatypeProperty ;
                   rdfs:domain :SemanticArtefactDistribution ;
                   rdfs:range xsd:anyURI ;
                   rdfs:comment "property used to specify the hierarchy  (e.g. rdfs:subClassOf or skos:broader)."@en ;
                   rdfs:label "transitive hierarchy property"@en .


###  https://w3id.org/mod#knownUsage
mod:knownUsage rdf:type owl:DatatypeProperty ;
            rdfs:domain :SemanticArtefact ;
            rdfs:range xsd:string ;
            rdfs:comment "The applications where the ontology is being used."@en ;
            rdfs:label "known usage"@en ;
            skos:historyNote "This property has been adopted from OMV Ontology Metadata Vocabulary and redefined in the MOD namespace."@en .


###  https://w3id.org/mod#maxChildCount
mod:maxChildCount rdf:type owl:DatatypeProperty ;
               rdfs:subPropertyOf :metrics ;
               rdfs:range xsd:nonNegativeInteger ;
               rdfs:comment """Maximum number of children per class (BioPortal definition)
Screen reader support enabled."""@en ;
               rdfs:label "maximum number of children per class"@en .


###  https://w3id.org/mod#maxDepth
mod:maxDepth rdf:type owl:DatatypeProperty ;
          rdfs:subPropertyOf :metrics ;
          rdfs:range xsd:nonNegativeInteger ;
          rdfs:comment "Maximum depth of the hierarchy tree (BioPortal definition)."@en ;
          rdfs:label "maximum depth of the hierarchy"@en .


###  https://w3id.org/mod#metrics
mod:metrics rdf:type owl:DatatypeProperty ;
         rdfs:domain :SemanticArtefactDistribution ;
         rdfs:comment "A generic property to store any metrics related to the ontology."@en ;
         rdfs:label "metrics"@en .


###  https://w3id.org/mod#numberOfAxioms
mod:numberOfAxioms rdf:type owl:DatatypeProperty ;
                rdfs:subPropertyOf :metrics ;
                rdfs:range xsd:nonNegativeInteger ;
                rdfs:comment "The total number of axioms in an ontology."@en ;
                rdfs:label "number of axioms or triples"@en .


###  https://w3id.org/mod#numberOfClasses
mod:numberOfClasses rdf:type owl:DatatypeProperty ;
                 rdfs:subPropertyOf :metrics ;
                 rdfs:range xsd:nonNegativeInteger ;
                 rdfs:comment "The total number of classes in an ontology."@en ;
                 rdfs:label "number of classes"@en .


###  https://w3id.org/mod#numberOfDataProperties
mod:numberOfDataProperties rdf:type owl:DatatypeProperty ;
                        rdfs:subPropertyOf :numberOfProperties ;
                        rdfs:range xsd:nonNegativeInteger ;
                        rdfs:comment "The total number of data properties in an ontology."@en ;
                        rdfs:label "number of data properties"@en .


###  https://w3id.org/mod#numberOfIndividuals
mod:numberOfIndividuals rdf:type owl:DatatypeProperty ;
                     rdfs:subPropertyOf :metrics ;
                     rdfs:range xsd:nonNegativeInteger ;
                     rdfs:comment "The total number of individuals in an ontology."@en ;
                     rdfs:label "number of individuals"@en .


###  https://w3id.org/mod#numberOfLabels
mod:numberOfLabels rdf:type owl:DatatypeProperty ;
                rdfs:subPropertyOf :metrics ;
                rdfs:range xsd:nonNegativeInteger ;
                rdfs:comment "Number of defined labels for any resources in an ontology (classes, properties, etc)."@en ;
                rdfs:label "number of labels"@en .


###  https://w3id.org/mod#numberOfObjectProperties
mod:numberOfObjectProperties rdf:type owl:DatatypeProperty ;
                          rdfs:subPropertyOf :numberOfProperties ;
                          rdfs:range xsd:nonNegativeInteger ;
                          rdfs:comment "The total number of object properties in an ontology."@en ;
                          rdfs:label "number of object properties"@en .


###  https://w3id.org/mod#numberOfProperties
mod:numberOfProperties rdf:type owl:DatatypeProperty ;
                    rdfs:subPropertyOf :metrics ;
                    rdfs:range xsd:nonNegativeInteger ;
                    rdfs:comment "The total number of properties in an ontology."@en ;
                    rdfs:label "number of properties"@en .


###  https://w3id.org/mod#obsoleteParent
mod:obsoleteParent rdf:type owl:DatatypeProperty ;
                rdfs:domain :SemanticArtefactDistribution ;
                rdfs:range xsd:anyURI ;
                rdfs:comment "property used to specify the root of an obsolete branch in the ontology."@en ;
                rdfs:label "root of obsolete branch"@en .


###  https://w3id.org/mod#obsoleteProperty
mod:obsoleteProperty rdf:type owl:DatatypeProperty ;
                  rdfs:domain :SemanticArtefactDistribution ;
                  rdfs:range xsd:anyURI ;
                  rdfs:comment "property used to specify an obsolete class."@en ;
                  rdfs:label "object obsolete property"@en .


###  https://w3id.org/mod#prefLabelPropert
mod:prefLabelPropert rdf:type owl:DatatypeProperty ;
                  rdfs:domain :SemanticArtefactDistribution ;
                  rdfs:range xsd:anyURI ;
                  rdfs:comment "Property used to specify preferred name (BioPortal definition)."@en ;
                  rdfs:label "object preferred label property"@en .


###  https://w3id.org/mod#sampleQueries
mod:sampleQueries rdf:type owl:DatatypeProperty ;
               rdfs:domain :SemanticArtefactDistribution ;
               rdfs:range xsd:string ;
               rdfs:comment "A set of queries (may be SPARQL, DL Queries) that are provided along with an ontology."@en ;
               rdfs:label "sample queries"@en .



###  https://w3id.org/mod#synonymProperty
mod:synonymProperty rdf:type owl:DatatypeProperty ;
                 rdfs:domain :SemanticArtefactDistribution ;
                 rdfs:range xsd:anyURI ;
                 rdfs:comment "Property used to specify preferred name (BioPortal definition)."@en ;
                 rdfs:label "object synonym property"@en .


###  https://w3id.org/mod#toDoList
mod:toDoList rdf:type owl:DatatypeProperty ;
          rdfs:domain :SemanticArtefact ;
          rdfs:range xsd:string ;
          rdfs:comment "Describes future tasks planned by a resource curator. This property is primarily intended to be used for vocabularies or datasets, but the domain is left open, it can be used for any resource. Use iCalendar Vtodo class and its properties to further describe the task calendar, priorities etc."@en ;
          rdfs:label "to do list"@en ;
          skos:historyNote """This property had been originally defined by VOAF metadata vocabulary. 
Now, it has been adopted and redefined in the MOD namespace."""@en .


#################################################################
#    Classes
#################################################################

###  http://creativecommons.org/ns#License
cc:License rdf:type owl:Class ;
           rdfs:comment "A set of requests/permissions to users of a Work, e.g. a copyright license, the public domain, information for distributors."@en ;
           rdfs:label "License"@en .


###  http://creativecommons.org/ns#work
cc:work rdf:type owl:Class ;
        rdfs:comment """A potentially copyrightable work.
(source: https://creativecommons.org/ns)"""@en ;
        rdfs:label "Work"@en .


###  http://iflastandards.info/ns/fr/frbr/frbrer/Expression
frbr:Expression rdf:type owl:Class ;
                  rdfs:comment "The intellectual or artistic realization of a work in the form of alpha-numeric, musical, or choreographic notation, sound, image, object, movement, etc., or any combination of such forms."@en ;
                  rdfs:label "Expression"@en .


###  http://iflastandards.info/ns/fr/frbr/frbrer/Work
frbr:Work rdf:type owl:Class ;
            rdfs:comment "A distinct intellectual or artistic creation."@en ;
            rdfs:label "Work"@en .


###  http://purl.org/dc/dcmitype/Collection
dcmi:Collection rdf:type owl:Class ;
                rdfs:comment "An aggregation of resources."@en ;
                rdfs:label "Collection"@en .


###  http://purl.org/dc/dcmitype/Dataset
dcmi:Dataset rdf:type owl:Class ;
             rdfs:comment "Data encoded in a defined structure. Examples include lists, tables, and databases. A dataset may be useful for direct machine processing."@en ;
             rdfs:label "Dataset"@en .


###  http://purl.org/dc/terms/Agent
dcterms:Agent rdf:type owl:Class ;
          rdfs:comment "A resource that acts or has the power to act."@en ;
          rdfs:label "Agent"@en .


###  http://purl.org/dc/terms/AgentClass
dcterms:AgentClass rdf:type owl:Class ;
               rdfs:comment "A group of agents."@en ;
               rdfs:label "Agent Class"@en .


###  http://purl.org/dc/terms/Frequency
dcterms:Frequency rdf:type owl:Class ;
              rdfs:comment "A rate at which something recurs."@en ;
              rdfs:label "Frequency"@en .


###  http://purl.org/dc/terms/Jurisdiction
dcterms:Jurisdiction rdf:type owl:Class ;
                 rdfs:comment "The extent or range of judicial, law enforcement, or other authority."@en ;
                 rdfs:label "Jurisdiction"@en .


###  http://purl.org/dc/terms/LicenseDocument
dcterms:LicenseDocument rdf:type owl:Class ;
                    rdfs:comment "A legal document giving official permission to do something with a resource."@en ;
                    rdfs:label "License Document"@en .


###  http://purl.org/dc/terms/LinguisticSystem
dcterms:LinguisticSystem rdf:type owl:Class ;
                     rdfs:comment "A system of signs, symbols, sounds, gestures, or rules used in communication."@en ;
                     rdfs:label "Linguistic System"@en .


###  http://purl.org/dc/terms/Location
dcterms:Location rdf:type owl:Class ;
             rdfs:comment "A spatial region or named place."@en ;
             rdfs:label "Location"@en .


###  http://purl.org/dc/terms/MediaType
dcterms:MediaType rdf:type owl:Class ;
              rdfs:subClassOf dcterms:MediaTypeOrExtent ;
              rdfs:comment "A file format or physical medium."@en ;
              rdfs:label "Media Type"@en .


###  http://purl.org/dc/terms/MediaTypeOrExtent
dcterms:MediaTypeOrExtent rdf:type owl:Class ;
                      rdfs:comment "A media type or extent."@en ;
                      rdfs:label "Media Type or Extent"@en .


###  http://purl.org/dc/terms/MethodOfAccrual
dcterms:MethodOfAccrual rdf:type owl:Class ;
                    rdfs:comment "A method by which resources are added to a collection."@en ;
                    rdfs:label "Method of Accrual"@en .


###  http://purl.org/dc/terms/PeriodOfTime
dcterms:PeriodOfTime rdf:type owl:Class ;
                 rdfs:comment "An interval of time that is named or defined by its start and end dates."@en ;
                 rdfs:label "Period Of Time"@en .


###  http://purl.org/dc/terms/Policy
dcterms:Policy rdf:type owl:Class ;
           rdfs:comment "A plan or course of action by an authority, intended to influence and determine decisions, actions, and other matters."@en ;
           rdfs:label "Policy"@en .


###  http://purl.org/dc/terms/RightsStatement
dcterms:RightsStatement rdf:type owl:Class ;
                    rdfs:comment "A statement about the intellectual property rights (IPR) held in or over a resource, a legal document giving official permission to do something with a resource, or a statement about access rights."@en ;
                    rdfs:label "Rights statement"@en .


###  http://purl.org/dc/terms/Standard
dcterms:Standard rdf:type owl:Class ;
             rdfs:comment "A reference point against which other things can be evaluated or compared."@en ;
             rdfs:label "Standard"@en .


###  http://rdfs.org/ns/void#Dataset
void:Dataset rdf:type owl:Class ;
             rdfs:comment "A dataset is a set of RDF triples that are published, maintained or aggregated by a single provider."@en ;
             rdfs:label "Dataset"@en .


###  http://rdfs.org/sioc/ns#MailingList
sioc:MailingList rdf:type owl:Class ;
                                      rdfs:comment "Describes an electronic mailing list."@en ;
                                      rdfs:label "MailingList"@en .


###  http://rdfs.org/sioc/ns#Weblog
sioc:Weblog rdf:type owl:Class ;
                                 rdfs:comment "Describes a weblog (blog), i.e. an online journal."@en ;
                                 rdfs:label "Weblog"@en .


###  http://rdfs.org/sioc/ns#Wiki
sioc:Wiki rdf:type owl:Class ;
                               rdfs:comment "Describes a wiki space."@en ;
                               rdfs:isDefinedBy "http://rdfs.org/sioc/types#"@en ;
                               rdfs:label "Wiki"@en .


###  http://schema.org/Audience
schema:Audience rdf:type owl:Class ;
                             rdfs:comment "Intended audience for an item, i.e. the group for whom the item was created."@en ;
                             rdfs:label "Audience"@en .


###  http://schema.org/Comment
schema:Comment rdf:type owl:Class ;
                            rdfs:subClassOf schema:CreativeWork ;
                            rdfs:comment "A comment on an item - for example, a comment on a blog post. The comment's content is expressed via the text property, and its topic via about, properties shared with all CreativeWorks."@en ;
                            rdfs:label "Comment"@en .


###  http://schema.org/CreativeWork
schema:CreativeWork rdf:type owl:Class ;
                                 rdfs:comment "The most generic kind of creative work, including books, movies, photographs, software programs, etc."@en ;
                                 rdfs:label "Creative Work"@en .


###  http://schema.org/DataCatalog
schema:DataCatalog rdf:type owl:Class ;
                                rdfs:subClassOf schema:CreativeWork ;
                                rdfs:comment "A collection of datasets."@en ;
                                rdfs:label "Data Catalog"@en .


###  http://schema.org/Dataset
schema:Dataset rdf:type owl:Class ;
                            rdfs:subClassOf schema:CreativeWork ;
                            rdfs:comment "A body of structured information describing some topic(s) of interest."@en ;
                            rdfs:label "Dataset"@en .


###  http://schema.org/MediaObject
schema:MediaObject rdf:type owl:Class ;
                                rdfs:subClassOf schema:CreativeWork ;
                                rdfs:comment "A media object, such as an image, video, or audio object embedded in a web page or a downloadable dataset i.e. DataDownload. Note that a creative work may have many media objects associated with it on the same web page. For example, a page about a single song (MusicRecording) may have a music video (VideoObject), and a high and low bandwidth audio stream (2 AudioObject's)."@en ;
                                rdfs:label "Media Object"@en .


###  http://schema.org/Organization
schema:Organization rdf:type owl:Class ;
                                 rdfs:comment "An organization such as a school, NGO, corporation, club, etc."@en ;
                                 rdfs:label "Organization"@en .


###  http://schema.org/Person
schema:Person rdf:type owl:Class ;
                           rdfs:comment "A person (alive, dead, undead, or fictional)."@en ;
                           rdfs:label "Person"@en .


###  http://schema.org/Place
schema:Place rdf:type owl:Class ;
                          rdfs:comment "Entities that have a somewhat fixed, physical extension."@en ;
                          rdfs:label "Place"@en .


###  http://schema.org/Review
schema:Review rdf:type owl:Class ;
                           rdfs:subClassOf schema:CreativeWork ;
                           rdfs:comment "A review of an item - for example, of a restaurant, movie, or store."@en ;
                           rdfs:label "Review"@en .


###  http://schema.org/dataDownload
schema:dataDownload rdf:type owl:Class ;
                                 rdfs:subClassOf schema:MediaObject ;
                                 rdfs:comment "A dataset in downloadable form."@en ;
                                 rdfs:label "data download"@en .


###  http://usefulinc.com/ns/doap#Project
doap:Project rdf:type owl:Class ;
             rdfs:subClassOf void:Dataset ;
             rdfs:comment "A project."@en ;
             rdfs:label "Project"@en .


###  http://usefulinc.com/ns/doap#Repository
doap:Repository rdf:type owl:Class ;
                rdfs:comment "Source code repository."@en ;
                rdfs:label "Repository"@en .


###  http://usefulinc.com/ns/doap#Version
doap:Version rdf:type owl:Class ;
             rdfs:comment "Version information of a project release."@en ;
             rdfs:label "Version"@en .


###  http://www.w3.org/2000/01/rdf-schema#Class
rdfs:Class rdf:type owl:Class ;
           rdfs:comment "The class resource, everything."@en ;
           rdfs:label "Class"@en .


###  http://www.w3.org/2000/01/rdf-schema#Resource
rdfs:Resource rdf:type owl:Class ;
              rdfs:subClassOf rdfs:Class ;
              rdfs:comment "All things described by RDF are called resources."@en ;
              rdfs:label "Resource"@en .


###  http://www.w3.org/2004/02/skos/core#Concept
skos:Concept rdf:type owl:Class ;
             rdfs:comment "An idea or notion; a unit of thought."@en ;
             rdfs:label "Concept"@en .


###  http://www.w3.org/2004/02/skos/core#ConceptScheme
skos:ConceptScheme rdf:type owl:Class ;
                   rdfs:subClassOf :SemanticArtefactDistribution ;
                   rdfs:comment "A SKOS concept scheme can be viewed as an aggregation of one or more SKOS concepts. Semantic relationships (links) between those concepts may also be viewed as part of a concept scheme."@en ;
                   rdfs:label "Concept Scheme"@en .


###  http://www.w3.org/2006/vcard/ns#Kind
<http://www.w3.org/2006/vcard/ns#Kind> rdf:type owl:Class ;
                                       rdfs:comment """\"Kinds\" to represent the types of objects to be represented by vCard:	 
Individual - To represent people
Organization - To represent organisations
Group - To represent groups of vCard objects
Location - To represent location objects"""@en ;
                                       rdfs:label "Kind"@en .


###  http://www.w3.org/ns/adms#Asset
adms:Asset rdf:type owl:Class ;
           rdfs:subClassOf dcat:Dataset ;
           rdfs:comment "An abstract entity that reflects the intellectual content of the asset and represents those characteristics of the asset that are independent of its physical embodiment. This abstract entity combines the FRBR entities work (a distinct intellectual or artistic creation) and expression (the intellectual or artistic realization of a work)."@en ;
           rdfs:label "Asset"@en .


###  http://www.w3.org/ns/adms#AssetDistribution
adms:AssetDistribution rdf:type owl:Class ;
                       rdfs:subClassOf dcat:Distribution ;
                       rdfs:comment "A particular physical embodiment of an Asset, which is an example of the FRBR entity manifestation (the physical embodiment of an expression of a work)."@en ;
                       rdfs:label "Asset Distribution"@en .


###  http://www.w3.org/ns/adms#Identifier
adms:Identifier rdf:type owl:Class ;
                rdfs:comment """This is based on the UN/CEFACT Identifier class which consists of:

    a content string which is the identifier;
    an optional identifier for the identifier scheme;
    an optional identifier for the version of the identifier scheme;
    an optional identifier for the agency that manages the identifier scheme."""@en ;
                rdfs:label "Identifier"@en .


###  http://www.w3.org/ns/dcat#Catalog
dcat:Catalog rdf:type owl:Class ;
                                    rdfs:subClassOf dcat:Dataset .


###  http://www.w3.org/ns/dcat#CatalogRecord
dcat:CatalogRecord rdf:type owl:Class ;
                                          rdfs:comment "A record in a catalog, describing the registration of a single dcat:Resource."@en ;
                                          rdfs:label "Catalog Record"@en .


###  http://www.w3.org/ns/dcat#DataService
dcat:DataService rdf:type owl:Class ;
                                        rdfs:subClassOf dcat:Resource .


###  http://www.w3.org/ns/dcat#Dataset
dcat:Dataset rdf:type owl:Class ;
                                    rdfs:subClassOf dcat:Resource ;
                                    rdfs:label "Dataset"@en .


###  http://www.w3.org/ns/dcat#Distribution
dcat:Distribution rdf:type owl:Class ;
                                         rdfs:comment "A specific representation of a dataset. A dataset might be available in multiple serializations that may differ in various ways, including natural language, media-type or format, schematic organization, temporal and spatial resolution, level of detail or profiles (which might specify any or all of the above)."@en ;
                                         rdfs:label "Distribution"@en .


###  http://www.w3.org/ns/dcat#Relationship
dcat:Relationship rdf:type owl:Class ;
                                         rdfs:comment "An association class for attaching additional information to a relationship between DCAT Resources."@en ;
                                         rdfs:label "Relationship"@en .


###  http://www.w3.org/ns/dcat#Resource
dcat:Resource rdf:type owl:Class ;
                                     rdfs:subClassOf rdfs:Resource ;
                                     rdfs:comment "Resource published or curated by a single agent."@en ;
                                     rdfs:label "Cataloged Resource"@en ,
                                                "Resource"@en .


###  http://www.w3.org/ns/odrl/2/Policy
odrl:Policy rdf:type owl:Class ;
            rdfs:label "Policy"@en .


###  http://www.w3.org/ns/prov#Activity
prov:Activity rdf:type owl:Class ;
              rdfs:comment "An activity is something that occurs over a period of time and acts upon or with entities; it may include consuming, processing, transforming, modifying, relocating, using, or generating entities."@en ;
              rdfs:label "Activity"@en .


###  http://www.w3.org/ns/prov#Agent
prov:Agent rdf:type owl:Class ;
           rdfs:comment "An agent is something that bears some form of responsibility for an activity taking place, for the existence of an entity, or for another agent's activity."@en ;
           rdfs:label "Agent"@en .


###  http://www.w3.org/ns/prov#Entity
prov:Entity rdf:type owl:Class ;
            rdfs:comment "An entity is a physical, digital, conceptual, or other kind of thing with some fixed aspects; entities may be real or imaginary."@en ;
            rdfs:label "Entity"@en .


###  http://www.w3.org/ns/sparql-service-description#Service
sd:Service rdf:type owl:Class ;
           rdfs:comment "An instance of sd:Service represents a SPARQL service made available via the SPARQL Protocol."@en ;
           rdfs:label "Service"@en .


###  http://xmlns.com/foaf/0.1/Agent
foaf:Agent rdf:type owl:Class ;
           rdfs:comment "An agent (eg. person, group, software or physical artifact)."@en ;
           rdfs:label "Agent"@en .


###  http://xmlns.com/foaf/0.1/Document
foaf:Document rdf:type owl:Class ;
              rdfs:comment "A document."@en ;
              rdfs:label "Document"@en .


###  http://xmlns.com/foaf/0.1/Image
foaf:Image rdf:type owl:Class ;
           rdfs:subClassOf foaf:Document ;
           rdfs:comment "An image."@en ;
           rdfs:label "Image"@en .


###  http://xmlns.com/foaf/0.1/Person
foaf:Person rdf:type owl:Class ;
            rdfs:subClassOf foaf:Agent ;
            rdfs:comment "A person."@en ;
            rdfs:label "Person"@en .


###  http://xmlns.com/foaf/0.1/Project
foaf:Project rdf:type owl:Class ;
             rdfs:comment "A project (a collective endeavour of some kind)."@en ;
             rdfs:label "Project"@en .


###  https://w3id.org/mod#Analytics
mod:Analytics rdf:type owl:Class ;
           rdfs:comment "Number of visits an ontology received."@en ;
           rdfs:isDefinedBy "https://www.isibang.ac.in/ns/mod/1.4/"@en ;
           rdfs:label "Analytics"@en .


###  https://w3id.org/mod#EngineeringMethodology
mod:EngineeringMethodology rdf:type owl:Class ;
                        rdfs:comment "Information about the engineering methodology."@en ;
                        rdfs:label "Engineering Methodology"@en ;
                        skos:historyNote "This class has been adopted from OMV Ontology Metadata Vocabulary, and renamed and redefined in the MOD namespace."@en .


###  https://w3id.org/mod#Evaluation
mod:Evaluation rdf:type owl:Class ;
            rdfs:comment "The results of evaluating an ontology. An ontology can have more than one evaluations."@en ;
            rdfs:label "Evaluation"@en .


###  https://w3id.org/mod#Group
mod:Group rdf:type owl:Class ;
       rdfs:comment "A group of ontologies that the ontology is usually considered into."@en ;
       rdfs:label "Group"@en .


###  https://w3id.org/mod#KnowledgeRepresentationParadigm
mod:KnowledgeRepresentationParadigm rdf:type owl:Class ;
                                 rdfs:label "Knowledge representation paradigm"@en .


###  https://w3id.org/mod#SemanticArtefact
mod:SemanticArtefact rdf:type owl:Class ;
                  rdfs:subClassOf cc:work ,
                                  frbr:Expression ,
                                  frbr:Work ,
                                  dcmi:Collection ,
                                  dcmi:Dataset ,
                                  schema:Dataset ,
                                  doap:Project ,
                                  adms:Asset ,
                                  dcat:Dataset ,
                                  dcat:Resource ,
                                  prov:Entity ,
                                  sd:Service ,
                                  foaf:Document ;
                  rdfs:label "Semantic Artefact"@en .


###  https://w3id.org/mod#SemanticArtefactCatalogRecord
mod:SemanticArtefactCatalogRecord rdf:type owl:Class ;
                               rdfs:subClassOf dcat:CatalogRecord .


###  https://w3id.org/mod#SemanticArtefactDistribution
mod:SemanticArtefactDistribution rdf:type owl:Class ;
                              rdfs:subClassOf adms:AssetDistribution ,
                                              dcat:Distribution .


###  https://w3id.org/mod#SemanticArtefactEvaluation
mod:SemanticArtefactEvaluation rdf:type owl:Class ;
                            rdfs:label "Semantic Artefact Evaluation"@en .


###  https://w3id.org/mod#SemanticArtefactService
mod:SemanticArtefactService rdf:type owl:Class ;
                         rdfs:subClassOf dcat:DataService .


###  https://w3id.org/mod#SemanticArtefactTask
mod:SemanticArtefactTask rdf:type owl:Class ;
                      rdfs:label "Semantic Artefact Task"@en .


###  https://w3id.org/mod#SemanticArtfeactCatalog
mod:SemanticArtfeactCatalog rdf:type owl:Class ;
                         rdfs:subClassOf dcat:Catalog .


###  https://w3id.org/mod#Taxonomy
mod:Taxonomy rdf:type owl:Class ;
          rdfs:subClassOf :SemanticArtefact .


###  https://w3id.org/mod#Terminology
mod:Terminology rdf:type owl:Class ;
             rdfs:subClassOf :SemanticArtefact .


###  https://w3id.org/mod#Thesaurus
mod:Thesaurus rdf:type owl:Class ;
           rdfs:subClassOf :SemanticArtefact .


###  Generated by the OWL API (version 4.5.9.2019-02-01T07:24:44Z) https://github.com/owlcs/owlapi
