@prefix mod: <https://w3id.org/mod#> .
@prefix cc: <http://creativecommons.org/ns#> .
@prefix sd: <http://www.w3.org/ns/sparql-service-description#> .
@prefix dc: <http://purl.org/dc/elements/1.1/> .
@prefix dcterms: <http://purl.org/dc/terms/> .
@prefix door: <http://kannel.open.ac.uk/ontology#> .
@prefix omv: <http://omv.ontoware.org/2005/05/ontology#> .
@prefix owl: <http://www.w3.org/2002/07/owl#> .
@prefix pav: <http://purl.org/pav/> .
@prefix rdf: <http://www.w3.org/1999/02/22-rdf-syntax-ns#> .
@prefix xml: <http://www.w3.org/XML/1998/namespace/> .
@prefix xsd: <http://www.w3.org/2001/XMLSchema#> .
@prefix adms: <http://www.w3.org/ns/adms#> .
@prefix dcat: <http://www.w3.org/ns/dca#> .
@prefix dcmi: <http://purl.org/dc/dcmitype/> .
@prefix doap: <http://usefulinc.com/ns/doap#> .
@prefix foaf: <http://xmlns.com/foaf/0.1/> .
@prefix idot: <http://identifiers.org/idot/> .
@prefix nkos: <http://w3id.org/nkos#> .
@prefix odrl: <http://www.w3.org/ns/odrl/2/> .
@prefix prov: <http://www.w3.org/ns/prov#> .
@prefix rdfs: <http://www.w3.org/2000/01/rdf-schema#> .
@prefix sioc: <http://rdfs.org/sioc/> .
@prefix skos: <http://www.w3.org/2004/02/skos/core#> .
@prefix vann: <https://vocab.org/vann/> .
@prefix void: <http://rdfs.org/ns/void#> .
@prefix voaf: <http://purl.org/vocommons/voaf#> .
@prefix frbr: <http://purl.org/vocab/frbr/core#> .
@prefix schema: <https://schema.org/> .
@prefix oboinowl: <http://www.geneontology.org/formats/oboInOwl#> .
@base <https://w3id.org/mod> .

<https://w3id.org/modp> rdf:type owl:Ontology ;       

#################################################################
#    MOD2.0 profile description with MOD2 profile properties
#################################################################

# This section is a description of MOD2 profile with a subset of properties of the profile itself. 
# Properties are sorted and grouped as in GSheet working document.
# Texttual descriptions are available in English and French. 
# Properties from MOD2 that are not used to described MOD2 profile are commented.

  ########## Intrinsic properties ##########
    mod:acronym                     "MODP" ;
    dcterms:title                   "MODP: Metadata for Ontology Description and publication Profile"@en,
                                    "MODP: Profil de Metadonnées pour la Description et la publication d'Ontologies"@fr ;
    dcterms:alternative             "MOD metadata profile"@en ,
                                    "Profil de métadonnées MOD"@fr ;
    owl:ontologyIRI                 <https://w3id.org/modp> ;
    owl:versionIRI                  <https://w3id.org/modp/2.0> ;
    owl:versionInfo                 "2.0.1" ;
    mod:status                      "alpha" ;
    owl:deprecated                  false ;
    dcterms:license                 <https://creativecommons.org/licenses/by/4.0> ; 
    mod:hasRepresentationLanguage   omv:OWL ;
    mod:hasFormalityLevel           omv:Vocabulary ;
    mod:hasSyntax                   <http://www.w3.org/ns/formats/Turtle> ;
    dcterms:language                <http://lexvo.org/id/iso639-3/eng> ,
                                    <http://lexvo.org/id/iso639-3/fra> ;

  ########## Description properties ##########
    dcterms:description        
                                    "MODP (Metadata for Ontology Description and publication Profile) is a metadata profile to describe metadata descriptions for ontologies or semantic resources/artefacts in general (thesaurus, terminologies, vocabularies, etc.). The MODP OWL file is a formal specifications of the metadata profile in RDF. It is based on the work done to build the MOD ontology. MODP is maximal (i.e., contains as much property as possible) and can be used to define sub-profiles for recommended metadata properties (e.g., H2020 project FAIRsFAIR semantic artefact minimum metadata profile). Users can go through MODP and pickup the required properties to describe their ontology."@en, 
                                    "MODP (Profil de Metadonnées pour la Description et la publication d'Ontologie) est un profil de métadonnées pour décire des descriptions de métadonnées pour les ontologies ou les ressources/artefacts sémantiques en général (thésaurus, terminologies, vocabulaires, etc.). Le fichier MODP OWL est une description formelle du profil en RDF basée sur le travail fait pur construire l'ontologie MOD. MODP est maximal (i.e., contient autant de propriété que possible) et peut donc être utilisé pour définir des sous-profils de métadonnées (e.g., le profil de métadonnées minimale pour les artefacts sémanttique du projet H2020 FAIRsFAIR). Les utilisateurs peuvent consulter la spécification de MODP et récupérer les propriétés requises pour décrire leur ontologie."@fr ;
    dcterms:abstract
                                    "MODP provides a set of properties which can be used by ontology developers, ontology libraries (e.g., ontology registry, ontology repository, ontology portal), to describe and publish ontologies or semantic resources/artefacts. The enriched description of ontologies, in turn, will help users to search, discover, identify and select ontologies."@en ,
                                    "MODP fournit un ensemble de propriétés pouvant être utilisées par les développeurs d’ontologies ou les portails d’ontologies (registre, bibliothèques), pour décrire et publier des ontologies ou des ressources/artefacts sémantiques. La description enrichie des ontologies aidera les utilisateurs à rechercher, découvrir, identifier et sélectionner des ontologies."@fr ;
    cc:morePermissions              "https://github.com/sifrproject/MOD-Ontology/blob/master/LICENSE" ;
    cc:useGuidelines                "MODP is free of use; feedback is welcome."@en ,
                                    "MODP peut être utilisée de manière libre; les retours sont appréciés."@fr ;
    rdfs:comment            
                                    "This project is connected to the work done within AgroPortal (with MOD1.4). MODP and MOD 2.0 are work in progress."@en ,
                                    "Ce projet est lié au travail mis en œuvre dans AgroPortal (avec MOD1.4). MODP et MOD2.0 sont en cours de développement."@fr ;
    omv:keywords                    "metadata description, metadata vocabularies, ontology description, metadata profile"@en ,
                                    "description de métadonnées, vocabulaires de métadonnées, description d'ontologie, profil de métadonnées"@fr ;
    pav:createdWith                 "Text editor" ;
    dcterms:coverage    
                                    "Ontologies or semantic resources/artefacts in general (thesaurus, terminologies, vocabularies, etc.)"@en ,
                                    "Les ontologies ou les ressources/artefacts sémantiques en général (thésaurus, terminologies, vocabulaires, etc.)"@fr ;
    mod:competencyQuestion
                                    "How to standardly and semantically capture the description of an ontology while relying on other existing metadata vocabularies?"@en ,
                                    "Comment capturer de manière standard et sémantique la description d'une ontologie en s'appuyant sur d'autres vocabulaires de métadonnées existants?"@fr ;
    foaf:homepage                   <https://github.com/sifrproject/MOD-Ontology> ;
    dcterms:accessRights        
                                    "MOD and MODP are licensed under the Creative Commons Attribution 4.0 ; For details, see here: https://github.com/sifrproject/MOD-Ontology/blob/master/LICENSE"@en ,
                                    "MOD and MODP sont disponibles sous Licence Creative Commons Attribution 4.0 ; pour plus de details voir https://github.com/sifrproject/MOD-Ontology/blob/master/LICENSE"@fr ;
    vann:changes                    
                                    "See changes in MOD2."@en ,
                                    "Voir changements dans MOD2"@fr ;
    vann:example                    
                                    "An adaptation of MOD1.4 is used within AgroPortal, since 2017. MOD2 is the baseline for H2020 project FAIRsFAIR semantic artefact minimum metadata profile."@en ,
                                    "Une adaptation de MOD est utilisée dans AgroPortal, depuis 2017. MOD2 est réutilisée par le profil de métadonnées minimale pour les artefacts sémanttique du projet H2020 FAIRsFAIR."@fr ;
    mod:prefLabelProperty           rdfs:label ;
    mod:synonymProperty             skos:altLabel ;
    mod:definitionProperty          dcterms:description ;
    mod:authorProperty              pav:importedBy ;
    mod:obsoleteProperty            owl:deprecated ;
    mod:hierarchyProperty           rdfs:subClassOf ;
    mod:toDoList                   "https://github.com/sifrproject/MOD-Ontology/raw/master/mod-v2.0_todos.txt" ;

  ########## People properties ##########
  
    dcterms:creator                 "Biswanath Dutta (https://orcid.org/0000-0003-3059-8202)" ,
                                    "Clement Jonquet (https://orcid.org/0000-0002-2404-1582)" ; 
    dcterms:contributor             "Anne Toulet (https://orcid.org/0000-0003-0463-0854)" ; 
    dcterms:publisher               "Indian Statistical Institute, Bangalore Centre, India (https://www.isibang.ac.in)" ,
                                    "LIRMM, University of Montpellier, France (http://www.lirmm.fr)" ;
    schema:translator               "Clement Jonquet" ;
    dcterms:rightsHolder            "Indian Statistical Institute and University of Montpellier"@en ,
                                    "Institut Indien de la Statistique et Université de Montpellier"@fr;

  ########## Grouping properties ##########

    dcterms:subject                 "Metadata descriptions"@en ;
    mod:group                       "Metadata vocabularies"@en ;

  ########## Relation properties ##########

##  owl:imports                     ;  
    owl:priorVersion                <https://www.isibang.ac.in/ns/mod/1.4/> ,
                                    <https://www.isibang.ac.in/ns/mod/1.2/> ,
                                    <https://www.isibang.ac.in/ns/mod/1.1/> ,
                                    <https://www.isibang.ac.in/ns/mod/1.0/> ;
    owl:backwardCompatibleWith      <http://omv.ontoware.org/2005/05/ontology> ;
    owl:incompatibleWith            <http://kannel.open.ac.uk/ontology> ;
##  dcterms:isPartOf                ;
##  dcterms:hasPart                 ;  
##  dcterms:hasVersion              ;
##  dcterms:isFormatOf              ;
##  dcterms:hasFormat               ;
    dcterms:relation              
                                    "MOD uses or relates to each of these vocabularies: ADMS,CC,DCAT,DC,DCT,DOAP,DOOR,FOAF,IDOT,OBOINOWL,OMV,OWL,NKOS,PAV,PROV,RDFS,SCHEMA,SD,SKOS,VANN,VOAF,VOID."@en ,
                                    "MOD utilise ou se repose sur chacun des vocabulaires suivants : ADMS,CC,DCAT,DC,DCT,DOAP,DOOR,FOAF,IDOT,OBOINOWL,OMV,OWL,NKOS,PAV,PROV,RDFS,SCHEMA,SD,SKOS,VANN,VOAF,VOID."@fr ;
    mod:specializes                 <http://omv.ontoware.org/2005/05/ontology>;
##  schema:workTranslation          ;
##  schema:translationOfWork        ;
    mod:comesFromTheSameDomain      "OBOINOWL,OMV,OWL,NKOS,RDFS,SKOS,VANN,VOAF,VOID" ;
    mod:similar                     "OMV,VANN,VOAF,VOID" ;
    mod:hasEquivalencesWith      
                                    "MOD properties are 'reused' from properties in each these vocabularies: ADMS,CC,DCAT,DC,DCT,DOAP,FOAF,IDOT,OBOINOWL,OWL,NKOS,PAV,PROV,RDFS,SCHEMA,SD,SKOS,VANN,VOID. Reuses are formalized by a dcterms:relation. MOD2 redefines properties from DOOR, OMV, VOAF."@en ,  
                                    "Les propriétés de MOD sont 'importées' à partir des vocabulaires suivants : ADMS,CC,DCAT,DC,DCT,DOAP,FOAF,IDOT,OBOINOWL,OWL,NKOS,PAV,PROV,RDFS,SCHEMA,SD,SKOS,VANN,VOID. Les réutilisations soont formalisées par une propriété dcterms:relation. MOD2 re-définie les propriétés dans DOOR, OMV, VOAF."@fr ;
    mod:hasDisparateModelling  
                                    "DOAP (MOD reuses properties from both objects doap:Project and foaf:Document that are disjoincts.)"@en ,
                                    "DOAP (MOD réutilise des propriétés de des objets doap:Project et foaf:Document qui sont disjointes.)"@fr ;
##  mod:usedBy                      ;
    mod:generalizes                 "DOOR,OMV,VOAF"  ;
##  mod:hasDisjunctionsWith    ;

  ########## Content properties ##########

    foaf:primaryTopic       mod:Ontology ;
    void:rootResource       mod:Ontology ;
    mod:browsingUI          "https://www.isibang.ac.in/ns/mod/index.html" ;
##  sd:endpoint             ;
    mod:vocabularyUsed      <http://creativecommons.org/ns#> ,
                            <http://www.w3.org/ns/sparql-service-description#> ,
                            <http://purl.org/dc/terms/> ,
                            <http://omv.ontoware.org/2005/05/ontology#> ,
                            <http://www.w3.org/2002/07/owl#> ,
                            <http://purl.org/pav/> ,
                            <http://www.w3.org/1999/02/22-rdf-syntax-ns#> ,
                            <http://www.w3.org/XML/1998/namespace> ,
                            <http://www.w3.org/2001/XMLSchema#> ,
                            <http://usefulinc.com/ns/doap/> ,
                            <http://xmlns.com/foaf/0.1/> ,
                            <http://identifiers.org/idot/> ,
                            <http://www.w3.org/ns/prov#> ,
                            <http://www.w3.org/2000/01/rdf-schema#> ,
                            <http://www.w3.org/2004/02/skos/core#> ,
                            <http://purl.org/vocab/vann/> ,
                            <http://rdfs.org/ns/void#> ,
                            <https://schema.org/> ;
    mod:sampleQueries       
                            "For sample SPARQL queries to query MOD OWL knowledge base, see here: https://github.com/sifrproject/MOD-Ontology/blob/master/SPARQL_Queries_on_MOD_1.2.3-with-instances.txt"@en ,
                            "Pour des examples de requêtes SPARQL sur la base de connaissances MOD, voir ici : https://github.com/sifrproject/MOD-Ontology/blob/master/SPARQL_Queries_on_MOD_1.2.3-with-instances.txt"@fr ;
##  void:propertyPartition  ;
##  void:classPartition     ;
    void:dataDump           "https://www.isibang.ac.in/ns/mod/ontology.ttl" ,
                            "https://www.isibang.ac.in/ns/mod/ontology.json" ,
                            "https://www.isibang.ac.in/ns/mod/ontology.xml" ,
                            "https://www.isibang.ac.in/ns/mod/ontology.nt" ,
                            "https://www.isibang.ac.in/ns/mod/ontology.ttl" ;
##  void:openSearchDescription    ;
##  void:uriLookupEndpoint        ;

  ########## Community properties ##########

    mod:knownUsage          
                            "MOD is used for instance in AgroPortal (http://agroportal.lirmm.fr) to provide equivalences in AgroPortal's ontology metadata model. Other uses will be documented here in the future."@en ,
                            "MOD est utilisée par exemple dans AgroPortal (http://agroportal.lirmm.fr) pour fournir des equivalences au sein du modèle de métadonnées d'ontologies. D'autres usages seront documentés ici dans le futur."@fr ;
    mod:endorsedBy          "No organization is currenlty officially endorsing MOD."@en ,
                            "MOD n'est encore officiellement recommandée par aucune organization."@fr ;
    mod:usedInProject       "AgroPortal (http://agroportal.lirmm.fr)" ;
    dcterms:audience            
                            "MOD primary targets ontology (or semantic resource/artefact) developers and ontology library, repository or service providers."@en ,
                            "MOD s'adresse en priorité aux dévelopeurs d'ontologies (ou de ressource/artefact sémantiques) ainsi qu'au dévelopeurs de bibliothèque, de portail ou de service pour des ontologies."@fr ;
    foaf:fundedBy           
                            "Indian Statistical Institute, University of Montpellier, European French National Research Agency (under grant ANR-10-LABX-20, ANR-11-BINF-0002, ANR-19-DATA-0019), European Union’s Horizon 2020 research and innovation programme under the Marie Sklodowska-Curie grant agreement No 701771 and H2020 FAIRsFAIR project No 831558."@en ;
    doap:repository         <https://github.com/sifrproject/MOD-Ontology> ;
    doap:bugDatabase        <https://github.com/sifrproject/MOD-Ontology/issues> ;
##  doap:mailingList        ;
##  mod:hasEvaluation       ;
##  schema:comment          ;
##  mod:analytics           ;

  ########## Date properties ##########

    dcterms:created         "2021-12-01" ;
    dcterms:modified        "2022-02-14" ;
##  dcterms:valid           ;
##  pav:curatedOn           ;

  ########## Metrics properties ##########

##  mod:metrics                       ;
    mod:numberOfClasses               79 ;
    mod:numberOfIndividuals           7 ;
    mod:numberOfProperties            260 ;
    mod:numberOfObjectProperties      149 ;
    mod:numberOfDataProperties        111 ;
    mod:numberOfAxioms                1507 ;   
##  mod:numberOfLabels                ;
##  mod:byteSize                      ;
##  mod:maxDepth                      ;
##  mod:maxChildCount                 ;
##  mod:averageChildCount             ;
##  mod:classesWithOneChild           ;
##  mod:classesWithMoreThan25Children ; 
##  mod:classesWithNoDefinition       ;

  ########## Provenance properties ##########

    dcterms:source            
                            "MOD source is described in https://dx.doi.org/10.1007/978-3-319-70863-8_17 and https://doi.org/10.1007/s13740-018-0091-5"@en ,
                            "L'origine de MOD est décrite dans https://dx.doi.org/10.1007/978-3-319-70863-8_17 et https://doi.org/10.1007/s13740-018-0091-5"@fr ;
    prov:wasGeneratedBy     
                            "MOD is the result of a manual process of identifying, reviewing, and selecting candidate properties from standards metadata vocabularies if relevant to describe an ontology or any kind of semantic resource. When a property cannot be identified, it could be created in the MOD namespace. Since MCD2, it has been created as an extension of DCAT2."@en ,
                            "MOD est le résultat d'un processus manuel d'identification, de révision et de sélection des propriétés candidates à partir de vocabulaires de métadonnées standards, pour décrire une ontologie ou tout type de ressource sémantique. Lorsqu'une propriété ne peut pas être identifiée, elle peut être créée dans l'espace de noms MOD. Depuis MOD2, MOD est construote comme une extension de DCAT2"@fr ;
##  prov:wasInvalidatedBy   ;
    dcterms:accrualMethod       
                            "When a need of a new property is identified by the developer team, we review classic/standards metadata vocabularies to identifiy if the desire property already exists. If it exists in several metadata vocabularies we give priorities to consitency with previous MOD choices, then W3C Recommendations, then community standards."@en ,
                            "Lorsqu'un besoin d'une nouvelle propriété est identifié par l'équipe de développeurs, nous passons en revue les vocabulaires de métadonnées classiques / standards pour identifier si la propriété désirée existe déjà. Si elle existe dans plusieurs vocabulaires de métadonnées, nous donnons la priorité à la cohérence avec les choix précédents dans MOD, puis aux recommandations du W3C, puis aux normes de la communauté."@fr ;
    dcterms:accrualPeriodicity  
                            "New properties are added on demand with no specific periodicity."@en ,
                            "Les nouvelles propriétés sont ajoutées à la demande sans périodicité particulière."@fr ;
    dcterms:accrualPolicy       
                            "Editorial choice of the developer team."@en ,
                            "Choix éditorial de l'équipe de développeurs."@fr .


#################################################################
# Pattern to respect for each MOD properties
#################################################################
#
#### PropertyURI
#originalns:xx      rdf:type                rdf:Property ;
#                   rdfs:subPropertyOf      SUPER PROPERTY IF ANY
#                   rdfs:label              ""@en ,
#                                           ""@fr ;
#                   rdfs:domain             DOMAIN INFO IF ANY
#                   rdfs:range              RANGE INFO IF ANY
#                   dcterms:description     DESCCRIPTION FROM ORIGINAL SOURCE ;
#                   rdfs:isDefinedBy        URI OF ORIGINAL SOURCE ;
#                   dcterms:issued          "DATE OF THE FIRST CREATION OF THE PROPERTY BY ORIGINAL RESOURCE"^^xsd:date ;
#                   dcterms:relation        RELATED PROPERTY IN ANOTHER METADATA (not owl:equivalentProperty); 
#                   pav:derivedFrom         URI OF FIRST MOD VERSION INCLUDING" ;
#                   pav:importedOn          "DATE OF FIRST MOD VERSION INCLUDING"^^xsd:dateTime ;
#                    
#            #OPTIONAL STATEMENTS
#                   prov:wasInfluencedBy    "MIRO guidelines: ...." ;
#            
#            #OTHER ORIGINAL STATEMENTS IF ANY 
#            
#################################################################


#################################################################
#  Properties (sorted as in GSheet working document)
#################################################################

##########################################
########## Intrinsic properties ##########
##########################################


### https://w3id.org/mod#acronym
mod:acronym         rdf:type                owl:DatatypeProperty ;
                    rdfs:subPropertyOf      rdfs:label ;
                    rdfs:label              "acronym"@en ,
                                            "acronyme"@fr ;
                    rdfs:domain             mod:SemanticArtefact ;
                    rdfs:range              xsd:string ;
                    dcterms:description     "MOD: Short acronym label, often used as an identifier within some ontology platforms such as BioPortal or OBO Foundry. OMV: A short name by which an ontology is formally known."@en ;
                    rdfs:isDefinedBy        <http://omv.ontoware.org/2005/05/ontology> ;
                    dcterms:issued          "2009-12-24"^^xsd:date ;
                    dcterms:relation        <http://www.isibang.ac.in/ns/mod/1.0/acronym> ;
                    pav:derivedFrom         <http://www.isibang.ac.in/ns/mod/1.0> ;
                    pav:importedOn          "2015-08-05"^^xsd:dateTime ;
            
            #OPTIONAL STATEMENTS
                    skos:historyNote        "This property has been adopted from OMV Ontology Metadata Vocabulary and redefined in the MOD namespace."@en ;
                    prov:wasInfluencedBy    "MIRO guidelines: A.1" ,
                                            "FAIR principle: F2" .
            


### http://purl.org/dc/terms/title
dcterms:title       rdf:type                rdf:Property ;
                    rdfs:subPropertyOf      dc:title ;
                    rdfs:label              "title"@en ,
                                            "titre"@fr ;
                    rdfs:range              rdfs:Literal ;
                    dcterms:description     "DCTERMS: A name given to the resource. OMV: The name by which an ontology is formally known. RDFS: A human-readable name for the subject. FOAF:  A name for some thing. SKOS: The preferred and alternative labels are useful when generating or creating human-readable representations of a knowledge organization system. SCHEMA: The name of the item."@en ;
                    rdfs:isDefinedBy        <http://purl.org/dc/terms/> ;
                    dcterms:issued          "2008-01-14"^^xsd:date ;
                    dcterms:relation        cc:attributionName ,
                                            omv:name ,
                                            schema:name ,
                                            skos:prefLabel ,
                                            foaf:name ;
                    pav:derivedFrom         <http://www.isibang.ac.in/ns/mod/1.2> ;
                    pav:importedOn          "2017-07-06"^^xsd:dateTime ;
                    
            #OPTIONAL STATEMENTS
                    prov:wasInfluencedBy    "MIRO guidelines: A.1" ,
                                            "FAIR principle: F2" .
     


### http://purl.org/dc/terms/alternative
dcterms:alternative rdf:type                rdf:Property ;
                    rdfs:subPropertyOf      dc:title , dcterms:title ;
                    rdfs:label              "alternative name"@en ,
                                            "nom alternatif"@fr ;
                    rdfs:range              rdfs:Literal ;
                    dcterms:description     "DCTERMS: An alternative name for the resource. The distinction between titles and alternative titles is application-specific. SKOS: The preferred and alternative labels are useful when generating or creating human-readable representations of a knowledge organization system. SCHEMA: An alias for the item. A short label that is used by some communities to refer to a dataset (see 'preferredPrefix')."@en ;
                    rdfs:isDefinedBy        <http://purl.org/dc/terms/> ;
                    dcterms:issued          "2000-07-11"^^xsd:date ;
                    dcterms:relation        idot:alternatePrefix ,
                                            schema:alternateName ,
                                            skos:altLabel ;
                    pav:derivedFrom         <http://www.isibang.ac.in/ns/mod/1.2> ;
                    pav:importedOn          "2017-07-06"^^xsd:dateTime ;
                    
            #OPTIONAL STATEMENTS
                    prov:wasInfluencedBy    "MIRO guidelines: A.1" ,
                                            "FAIR principle: F2" .
            


### http://www.w3.org/2004/02/skos/core#hiddenLabel
skos:hiddenLabel    rdf:type                rdf:Property ,
                                            owl:AnnotationProperty ;
                    rdfs:subPropertyOf      rdfs:label ;
                    rdfs:label              "hidden label"@en ,
                                            "nom caché"@fr ;

                    rdfs:range              rdfs:Literal ;
                    dcterms:description     "MOD: Hidden or past name. SKOS: A lexical label for a resource that should be hidden when generating visual displays of the resource, but should still be accessible to free text search operations."@en;
                    rdfs:isDefinedBy        <http://www.w3.org/2004/02/skos/core> ;
                    dcterms:issued          "2009-08-18"^^xsd:date ;
                    pav:derivedFrom         <http://www.isibang.ac.in/ns/mod/1.4> ;
                    pav:importedOn          "2018-08-02"^^xsd:dateTime ;
                    
            #OPTIONAL STATEMENTS
                    prov:wasInfluencedBy    "MIRO guidelines: A.1" ,
                                            "FAIR principle: F2" ;
            
            #OTHER ORIGINAL STATEMENTS IF ANY 
                    rdfs:comment            "S12 (not formally stated): The range of skos:hiddenLabel is the class of RDF plain literals. S13 (not formally stated): skos:prefLabel, skos:altLabel and skos:hiddenLabel are pairwise disjoint properties."@en .


    
### https://w3id.org/mod#URI
mod:URI             rdf:type                owl:DatatypeProperty ;
                    rdfs:label              "URI"@en ,
                                            "URI"@fr ;
                    rdfs:domain             mod:SemanticArtefact ;
                    rdfs:range              xsd:anyURI ;
                    dcterms:description     "OMV: The URI of the ontology which is described by this metadata."@en ;
                    rdfs:isDefinedBy        <http://omv.ontoware.org/2005/05/ontology> ;
                    dcterms:issued          "2009-12-24"^^xsd:date ;
                    dcterms:relation        omv:URI ;
                    pav:derivedFrom         <http://www.isibang.ac.in/ns/mod/1.2> ;
                    pav:importedOn          "2017-07-06"^^xsd:dateTime ;
            
            #OPTIONAL STATEMENTS
                    skos:historyNote        "This property has been adopted from OMV Ontology Metadata Vocabulary and redefined in the MOD namespace."@en ;
                    prov:wasInfluencedBy    "MIRO guidelines: A.4" ,
                                            "FAIR principle: F1" .   
  


### http://www.w3.org/2002/07/owl#versionIRI
owl:versionIRI      rdf:type                owl:OntologyProperty ;
                    rdfs:label              "version IRI"@en ,
                                            "IRI de la version"@fr ;
                    rdfs:domain             owl:Ontology ;
                    rdfs:range              owl:Ontology ;
                    dcterms:description     "OWL: The property that identifies the version IRI of an ontology."@en ;  
                    rdfs:isDefinedBy        <http://www.w3.org/2002/07/owl#> ;
                    dcterms:issued          "2004-02-10"^^xsd:date ;
                    pav:derivedFrom         <http://www.isibang.ac.in/ns/mod/1.2> ;
                    pav:importedOn          "2017-07-06"^^xsd:dateTime ;
                    
            #OPTIONAL STATEMENTS
                    prov:wasInfluencedBy    "MIRO guidelines: A.4" ,
                                            "FAIR principle: F1" .
            


### http://purl.org/dc/terms/identifier
dcterms:identifier  rdf:type                rdf:Property ;
                    rdfs:subPropertyOf      dc:identifier  ;
                    rdfs:label              "Other identifier"@en ,
                                            "Autre identifiant"@fr ;
                    rdfs:range              rdfs:Literal ;
                    dcterms:description     "DCTERMS: An unambiguous reference to the resource within a given context. Recommended practice is to identify the resource by means of a string conforming to an identification system. Examples include International Standard Book Number (ISBN), Digital Object Identifier (DOI), and Uniform Resource Name (URN).  Persistent identifiers should be provided as HTTP URIs. SKOS: A notation is a string of characters such as 'T58.5 or '303.4833' used to uniquely identify a concept within the scope of a given concept scheme. ADMS: adms:identifier is used to link any resource to an instance of adms:Identifier which is its range. N.B. it is not appropriate to use dcterms:identifer to link to the Identifier class as its range is rdfs:Literal. ADMS uses this to provide any identifier for the Asset."@en ;
                    rdfs:isDefinedBy        <http://purl.org/dc/terms/> ;
                    dcterms:issued          "2008-01-14"^^xsd:date ;
                    dcterms:relation        skos:notation ,
                                            adms:identifier ,
                                            schema:identifier ;
                    pav:derivedFrom         <http://www.isibang.ac.in/ns/mod/1.0> ;
                    pav:importedOn          "2015-08-05"^^xsd:dateTime ;
                    
            #OPTIONAL STATEMENTS
                    prov:wasInfluencedBy    "FAIR principle: F1,A1" .
            


### http://www.w3.org/2002/07/owl#versionInfo
owl:versionInfo     rdf:type                owl:AnnotationProperty  ;
                    rdfs:label              "version information"@en ,
                                            "information de version"@fr ;
                    rdfs:domain             rdfs:Resource ;
                    rdfs:range              rdfs:Resource ;
                    dcterms:description     "MOD: The version of the released ontology. OMV: The version information of the ontology. OWL: The annotation property that provides version information for an ontology or another OWL construct. PAV: The version number of a resource. This is a freetext string, typical values are '1.5' or '21'. DOAP: A project release."@en ;  
                    rdfs:isDefinedBy        <http://www.w3.org/2002/07/owl#> ;
                    dcterms:issued          "2004-02-10"^^xsd:date ;
                    dcterms:relation        omv:version ,
                                            pav:version ,
                                            doap:release ,
                                            oboinowl:data-version ,
                                            oboinowl:hasVersion ,
                                            schema:version ,
                                            <http://www.isibang.ac.in/ns/mod/1.0/version> ;
                    pav:derivedFrom         <http://www.isibang.ac.in/ns/mod/1.0> ;
                    pav:importedOn          "2015-08-05"^^xsd:dateTime ;
        
            #OPTIONAL STATEMENTS
                    prov:wasInfluencedBy    "MIRO guidelines: A.1" ,
                                            "FAIR principle: R1.2" .
            


### https://w3id.org/mod#status
mod:status          rdf:type                owl:DatatypeProperty ;
                    rdfs:label              "status"@en ,
                                            "statut"@fr ;
                    rdfs:domain             mod:SemanticArtefact ;
                    rdfs:range              xsd:string ;
                    dcterms:description     "OMV: It specifies the tracking information for the contents of the ontology. Pre-defined values. IDOT: State of a resource (physical location providing access to data or information about the identified entity). This is should be based on a recent manual or automatic check of the resource. Possible values are: 'up', 'down', 'probably up', 'obsolete resource', 'restricted access' and 'unknown'."@en ;
                    rdfs:isDefinedBy        <http://omv.ontoware.org/2005/05/ontology> ;
                    dcterms:issued          "2009-12-24"^^xsd:date ;
                    dcterms:relation        idot:state ,
                                            adms:adms-status ;
                    pav:derivedFrom         <http://www.isibang.ac.in/ns/mod/1.0> ;
                    pav:importedOn          "2015-08-05"^^xsd:dateTime ;
            
            #OPTIONAL STATEMENTS
                    skos:historyNote        "This property has been adopted from OMV Ontology Metadata Vocabulary and redefined in the MOD namespace."@en ;
                    prov:wasInfluencedBy    "FAIR principle: A2" .



### http://www.w3.org/2002/07/owl#deprecated
owl:deprecated     rdf:type                owl:AnnotationProperty ; 
                   rdfs:label              "deprecated"@en ,
                                           "obsolète"@fr ;
                   rdfs:domain             rdfs:Resource ;
                   rdfs:range              rdfs:Resource ;
                   dcterms:description     "OWL: The annotation property that indicates that a given entity has been deprecated. IDOT: Indicates if the current dataset is obsolete (not provided any more to the public community). Value can either be 'true' or 'false' (xsd:boolean). The statement is usually omitted if 'false'."@en ;
                   rdfs:isDefinedBy        <http://www.w3.org/2002/07/owl#> ;
                   dcterms:issued          "2004-02-10"^^xsd:date ;
                   dcterms:relation        idot:obsolete ,
                                           <http://www.isibang.ac.in/ns/mod/1.1/deprecated> ;                                         
                   pav:derivedFrom         <http://www.isibang.ac.in/ns/mod/1.1> ;
                   pav:importedOn          "2016-09-02"^^xsd:dateTime ; 
                                       
            #OPTIONAL STATEMENTS
                    prov:wasInfluencedBy   "FAIR principle: A2" .
            
     

### http://purl.org/dc/terms/license
dcterms:license     rdf:type                rdf:Property ;
                    rdfs:subPropertyOf      dc:rights , dcterms:rights ;
                    rdfs:label              "license"@en ,
                                            "licence"@fr ;
                    dcterms:description     "DCTERMS: A legal document giving official permission to do something with the resource. Recommended practice is to identify the license document with a URI. If this is not possible or feasible, a literal value that identifies the license may be provided. DCTERMS:rights Information about rights held in and over the resource. OMV: Underlying license model. SCHEMA: A license document that applies to this content, typically indicated by URL."@en ;
                    rdfs:isDefinedBy        <http://purl.org/dc/terms/> ;
                    dcterms:issued          "2004-06-14"^^xsd:date ;
                    dcterms:relation        cc:license ,
                                            omv:license ,
                                            schema:license ;
                    pav:derivedFrom         <http://www.isibang.ac.in/ns/mod/1.0> ;
                    pav:importedOn          "2015-08-05"^^xsd:dateTime ;
                    
            #OPTIONAL STATEMENTS
                    prov:wasInfluencedBy    "MIRO guidelines: A.3" ,
                                            "FAIR principle: A2" ;
            
            #OTHER ORIGINAL STATEMENTS IF ANY 
                    <http://purl.org/dc/dcam/rangeIncludes>     dcterms:LicenseDocument .



### https://w3id.org/mod#hasRepresentationLanguage
mod:hasRepresentationLanguage   
                    rdf:type                owl:DatatypeProperty ;
                    rdfs:label              "representation language"@en ,
                                            "language de représentation"@fr ;
                    rdfs:domain             mod:SemanticArtefactDistribution ;
                    rdfs:range              xsd:anyURI ;
                    dcterms:description     "MOD: A language that is used to create an ontology. OMV: The ontology language."@en ;
                    rdfs:isDefinedBy        <http://omv.ontoware.org/2005/05/ontology> ;
                    dcterms:issued          "2009-12-24"^^xsd:date ;
                    dcterms:relation        omv:hasOntologyLanguage ,
                                            schema:fileFormat ,
                                            <http://www.isibang.ac.in/ns/mod/1.0/ontologyDesignLanguage> ;
                    pav:derivedFrom         <http://www.isibang.ac.in/ns/mod/1.0> ;
                    pav:importedOn          "2015-08-05"^^xsd:dateTime ;
                    
            #OPTIONAL STATEMENTS
                    skos:historyNote        "This property has been adopted from OMV Ontology Metadata Vocabulary and redefined in the MOD namespace."@en ;
                    prov:wasInfluencedBy    "MIRO guidelines: E.1" ,
                                            "FAIR principle: I1" .
                


### https://w3id.org/mod#hasFormalityLevel
mod:hasFormalityLevel   
                    rdf:type                owl:DatatypeProperty ;
                    rdfs:label              "formality level"@en ,
                                            "niveau de formalisme"@fr ;
                    rdfs:domain             mod:SemanticArtefact ;
                    rdfs:range              xsd:string ;
                    dcterms:description     "MOD: The level of formality of an ontology. OMV: Level of formality of the ontology."@en ;
                    rdfs:isDefinedBy        <http://omv.ontoware.org/2005/05/ontology> ;
                    dcterms:issued          "2009-12-24"^^xsd:date ;
                    dcterms:relation        omv:hasFormalityLevel ,
                                            schema:fileFormat ,
                                            <http://www.isibang.ac.in/ns/mod/1.0/formalityLevel> ;
                    pav:derivedFrom         <http://www.isibang.ac.in/ns/mod/1.0> ;
                    pav:importedOn          "2015-08-05"^^xsd:dateTime ;
                    
            #OPTIONAL STATEMENTS
                    skos:historyNote        "This property has been adopted from OMV Ontology Metadata Vocabulary and redefined in the MOD namespace."@en ;
                    prov:wasInfluencedBy    "MIRO guidelines: E.1" ,
                                            "FAIR principle: I1" .
              


### https://w3id.org/mod#hasSyntax
mod:hasSyntax       rdf:type                owl:DatatypeProperty ;
                    rdfs:label              "syntax"@en ,
                                            "syntaxe"@fr ;
                    rdfs:domain             mod:SemanticArtefactDistribution ;
                    rdfs:range              xsd:anyURI ;
                    dcterms:description     "MOD: The syntax followed in the creation of an ontology. OMV: The presentation syntax for the ontology langage."@en ;
                    rdfs:isDefinedBy        <http://omv.ontoware.org/2005/05/ontology> ;
                    dcterms:issued          "2009-12-24"^^xsd:date ;
                    dcterms:relation        omv:hasOntologySyntax ,
                                            dcterms:format ,
                                            <http://www.isibang.ac.in/ns/mod/1.0/syntax> ;
                    pav:derivedFrom         <http://www.isibang.ac.in/ns/mod/1.0> ;
                    pav:importedOn          "2015-08-05"^^xsd:dateTime ;
            
            #OPTIONAL STATEMENTS
                    skos:historyNote        "This property has been adopted from OMV Ontology Metadata Vocabulary and redefined in the MOD namespace."@en ;
                    prov:wasInfluencedBy    "MIRO guidelines: E.1" ,
                                            "FAIR principle: I1" .
    


### http://purl.org/dc/terms/language
dcterms:language    rdf:type                rdf:Property ;
                    rdfs:subPropertyOf      dc:language ;
                    rdfs:label              "natural language"@en ,
                                            "langage naturel"@fr ;
                    dcterms:description     "DCTERMS: A language of the resource. Recommended practice is to use either a non-literal value representing a language from a controlled vocabulary such as ISO 639-2 or ISO 639-3, or a literal value consisting of an IETF Best Current Practice 47 [[IETF-BCP47](https://tools.ietf.org/html/bcp47)] language tag. OMV: The language of the content of the ontology, i.e. English, French, etc. DOAP: ISO language code a project has been translated into."@en ;
                    rdfs:isDefinedBy        <http://purl.org/dc/terms/> ;
                    dcterms:issued          "2008-01-14"^^xsd:date ;
                    dcterms:relation        omv:naturalLanguage ,
                                            schema:inLanguage ,
                                            doap:language ;
                    pav:derivedFrom         <http://www.isibang.ac.in/ns/mod/1.0> ;
                    pav:importedOn          "2015-08-05"^^xsd:dateTime ;
                    
            #OPTIONAL STATEMENTS
                    prov:wasInfluencedBy    "FAIR principle: F2" ;
            
            #OTHER ORIGINAL STATEMENTS IF ANY 
                    <http://purl.org/dc/dcam/rangeIncludes>     dcterms:LinguisticSystem .

    
##########################################
######## Description properties ##########
##########################################
      

### http://purl.org/dc/terms/description
dcterms:description rdf:type                rdf:Property ;
                    rdfs:subPropertyOf      dc:description ;
                    rdfs:label              "description"@en ,
                                            "description"@fr ;
                    dcterms:description     "DCTERMS: An account of the resource. Description may include but is not limited to: an abstract, a table of contents, a graphical representation, or a free-text account of the resource. OMV: Free text description of an ontology. SCHEMA: A description of the item. DOAP: Plain text description of a project, of 2-4 sentences in length."@en ;
                    rdfs:isDefinedBy        <http://purl.org/dc/terms/> ;
                    dcterms:issued          "2008-01-14"^^xsd:date ;
                    dcterms:relation        omv:description ,
                                            schema:description ,
                                            doap:description ;
                    pav:derivedFrom         <http://www.isibang.ac.in/ns/mod/1.0> ;
                    pav:importedOn          "2015-08-05"^^xsd:dateTime ;
                    
            #OPTIONAL STATEMENTS
                    prov:wasInfluencedBy    "MIRO guidelines: C.3" ,
                                            "FAIR principle: F2" .
            


### http://purl.org/dc/terms/abstract
dcterms:abstract    rdf:type                rdf:Property ;
                    rdfs:subPropertyOf      dc:description , dcterms:description ;
                    rdfs:label              "abstract"@en ,
                                            "résumé"@fr ;
                    dcterms:description     "DCTERMS: A summary of the resource."@en ;
                    rdfs:isDefinedBy        <http://purl.org/dc/terms/> ;
                    dcterms:issued          "2000-07-11"^^xsd:date ;
                    pav:derivedFrom         <http://www.isibang.ac.in/ns/mod/1.2> ;
                    pav:importedOn          "2017-07-06"^^xsd:dateTime ;
                    
            #OPTIONAL STATEMENTS
                    prov:wasInfluencedBy    "FAIR principle: F2" .
            


### http://creativecommons.org/ns#morePermissions
cc:morePermissions  rdf:type                rdf:Property ;
                    rdfs:subPropertyOf      dcterms:relation ; 
                    rdfs:label              "more permissions"@en ,
                                            "droits d'accès détaillés"@fr ;
                    rdfs:domain             cc:Work ;
                    rdfs:range              rdfs:Resource ;
                    dcterms:description     "CC: A related resource which describes additional permissions or alternative licenses for a Work which may be available."@en ;     
                    rdfs:isDefinedBy        <http://creativecommons.org/ns#> ;
                    dcterms:issued          "2008-03-03"^^xsd:date ;
                    pav:derivedFrom         <http://www.isibang.ac.in/ns/mod/1.4> ;
                    pav:importedOn          "2018-08-02"^^xsd:dateTime ;
                    
            #OPTIONAL STATEMENTS
                    prov:wasInfluencedBy    "FAIR principle: R1.1" .
  


### http://creativecommons.org/ns#useGuidelines
cc:useGuidelines    rdf:type                rdf:Property ;
                    rdfs:subPropertyOf      dcterms:relation ; 
                    rdfs:label              "use guidelines"@en ,
                                            "guide d'utilisation"@fr ;
                    rdfs:domain             cc:Work ;
                    rdfs:range              rdfs:Resource ;
                    dcterms:description     "CC: A related resource which defines non-binding use guidelines for the work."@en ;     
                    rdfs:isDefinedBy        <http://creativecommons.org/ns#> ;
                    dcterms:issued          "2008-03-03"^^xsd:date ;
                    pav:derivedFrom         <http://www.isibang.ac.in/ns/mod/1.4> ;
                    pav:importedOn          "2018-08-02"^^xsd:dateTime ;
                    
            #OPTIONAL STATEMENTS
                    prov:wasInfluencedBy    "FAIR principle: R1.1" .
  

### http://purl.org/dc/terms/bibliographicCitation
dcterms:bibliographicCitation
                    rdf:type                rdf:Property ;
                    rdfs:subPropertyOf      dc:identifier , dcterms:identifier;
                    rdfs:label              "bibliographic reference"@en ,
                                            "référence bibliographique";
                    rdfs:range              rdfs:Literal ;
                    dcterms:description     "DCTERMS: A bibliographic reference for the resource. Recommended practice is to include sufficient bibliographic detail to identify the resource as unambiguously as possible. OMV: List of bibliographic references describing the ontology and its applications. FOAF: A document that this thing is the primary topic of"@en ;
                    rdfs:isDefinedBy        <http://purl.org/dc/terms/> ;
                    dcterms:issued          "2003-02-15"^^xsd:date ;
                    dcterms:relation        omv:reference ,
                                            foaf:isPrimaryTopicOf ,
                                            schema:citation ;
                    pav:derivedFrom         <http://www.isibang.ac.in/ns/mod/1.2> ;
                    pav:importedOn          "2017-07-06"^^xsd:dateTime ;
                    
            #OPTIONAL STATEMENTS
                    prov:wasInfluencedBy    "FAIR principle: F2" .



### http://www.w3.org/ns/dcat#landingPage
dcat:landingPage    rdf:type                rdf:Property , owl:ObjectProperty ;
                    rdfs:subPropertyOf      foaf:page ; 
                    rdfs:label              "landing page"@en ,
                                            "page d'atterrissage"@fr ;
                    rdfs:range              foaf:Document ;
                    dcterms:description     "DCAT: A Web page that can be navigated to in a Web browser to gain access to the dataset, its distributions and/or additional information. MOD: A link to the documentation page on a thing. OMV: URL for further documentation. RDFS: Further information about the subject resource. DOAP: URL of Wiki for collaborative discussion of project. VANN: A reference to a resource that provides information on how this resource is to be used."@en ;
                    rdfs:isDefinedBy        <http://www.w3.org/TR/vocab-dcat/> ;
                    dcterms:issued          "2014-01-16"^^xsd:date ;
                    dcterms:relation        omv:documentation ,
                                            vann:usageNote ,
                                            doap:wiki ,
                                            rdfs:seeAlso ,
                                            <http://www.isibang.ac.in/ns/mod/1.0/document> ;
                    pav:derivedFrom         <http://www.isibang.ac.in/ns/mod/1.0> ;
                    pav:importedOn          "2015-08-05"^^xsd:dateTime ;
                    
            #OPTIONAL STATEMENTS
                    prov:wasInfluencedBy    "MIRO guidelines: C.3, F.1" ,
                                            "FAIR principle: F2" ;
            
            #OTHER ORIGINAL STATEMENTS IF ANY 
                    skos:scopeNote          "If the distribution(s) are accessible only through a landing page (i.e. direct download URLs are not known), then the landing page link should be duplicated as accessURL on a distribution."@en .


### http://www.w3.org/ns/dcat#accessURL
dcat:accessURL      rdf:type                rdf:Property , owl:ObjectProperty ;
                    rdfs:label              "access URL"@en ,
                                            "URL d'accès"@fr ;
                    rdfs:domain             dcat:Distribution ;
                    rdfs:range              rdfs:Resource ;
                    dcterms:description     "DCAT: A URL of a resource that gives access to a distribution of the dataset. E.g. landing page, feed, SPARQL endpoint. Use for all cases except a simple download link, in which case downloadURL is preferred. OMV: The location where the ontology can be found. It should be accessible via a URL. It can be the same as the value for URI property. DOAP:  Web page from which the project software can be downloaded."@en ;
                    rdfs:isDefinedBy        <http://www.w3.org/TR/vocab-dcat/> ;
                    dcterms:issued          "2014-01-16"^^xsd:date ;
                    dcterms:relation        omv:resourceLocator ,
                                            doap:download-page ;
                    pav:derivedFrom         <http://www.isibang.ac.in/ns/mod/1.2> ;
                    pav:importedOn          "2017-07-06"^^xsd:dateTime ;
                    
            #OPTIONAL STATEMENTS
                    prov:wasInfluencedBy    "MIRO guidelines: A.4" ,
                                            "FAIR principle: F2" ;
            
            #OTHER ORIGINAL STATEMENTS IF ANY 
                     skos:scopeNote         "If the distribution(s) are accessible only through a landing page (i.e. direct download URLs are not known), then the landing page link should be duplicated as accessURL on a distribution."@en .
 
 

### http://www.w3.org/2000/01/rdf-schema#Comment
rdfs:comment        rdf:type                rdf:Property ;
                    rdfs:label              "notes or comments"@en ,
                                            "notes ou commentaires"@fr ;
                    rdfs:domain             rdfs:Resource ;
                    rdfs:range              rdfs:Literal ;           
                    dcterms:description     "RDFS: A description of the subject resource. OMV: Additional information about the ontology that is not included somewhere else (e.g. information that you do not want to include in the documentation)."@en ;
                    rdfs:isDefinedBy        <http://www.w3.org/2000/01/rdf-schema#> ;
                    dcterms:issued          "2002-04-30"^^xsd:date ;
                    dcterms:relation        omv:notes ,
                                            dcterms:description ,
                                            adms:versionNotes ;
                    pav:derivedFrom         <http://www.isibang.ac.in/ns/mod/1.2> ;
                    pav:importedOn          "2017-07-06"^^xsd:dateTime ;
                    
            #OPTIONAL STATEMENTS
                    prov:wasInfluencedBy    "FAIR principle: F2" .
        


### http://www.w3.org/ns/dcat#keyword
dcat:keyword        rdf:type                rdf:Property , owl:DatatypeProperty ;
                    rdfs:subPropertyOf      dcterms:subject ; 
                    rdfs:label              "keyword"@en ,
                                            "motclé"@fr ;
                    rdfs:range              rdfs:Literal ;
                    dcterms:description     "DCAT: A keyword or tag describing a resource. MOD: A keyword(s) is used to describe the content of an ontology. OMV: List of keywords related to an ontology. SCHEMA: Keywords or tags used to describe this content. Multiple entries in a keywords list are typically delimited by commas."@en ;
                    rdfs:isDefinedBy        <http://www.w3.org/TR/vocab-dcat/> ;
                    dcterms:issued          "2014-01-16"^^xsd:date ;
                    dcterms:relation         omv:keywords ,
                                             schema:keywords ,
                                             <http://www.isibang.ac.in/ns/mod/1.1/keyword> ;
                    pav:derivedFrom         <http://www.isibang.ac.in/ns/mod/1.0> ;
                    pav:importedOn          "2015-08-05"^^xsd:dateTime ;
                    
            #OPTIONAL STATEMENTS
                    prov:wasInfluencedBy    "MIRO guidelines: C.1" ,
                                            "FAIR principle: F2" .
            


### http://purl.org/dc/terms/type
dcterms:type        rdf:type                rdf:Property ;
                    rdfs:subPropertyOf      dc:type ;
                    rdfs:label              "type"@en ,
                                            "type"@fr ;
                    dcterms:description     "DCTERMS: The nature or genre of the resource. Recommended practice is to use a controlled vocabulary such as the DCMI Type Vocabulary [[DCMI-TYPE](http://dublincore.org/documents/dcmi-type-vocabulary/)]. To describe the file format, physical medium, or dimensions of the resource, use the property Format. OMV: The nature of the content of the ontology."@en ;
                    rdfs:isDefinedBy        <http://purl.org/dc/terms/> ;
                    dcterms:issued          "2008-01-14"^^xsd:date ;
                    dcterms:relation        omv:isOfType ;
                    pav:derivedFrom         <http://www.isibang.ac.in/ns/mod/1.2> ;
                    pav:importedOn          "2017-07-06"^^xsd:dateTime ;
                    
            #OPTIONAL STATEMENTS
                    prov:wasInfluencedBy    "FAIR principle: F2" .



### https://w3id.org/mod#designedForTask
mod:designedForTask rdf:type                owl:ObjectProperty ;
                    rdfs:label              "designed for task"@en ,
                                            "concou pour la tâche"@fr ;
                    rdfs:domain             mod:SemanticArtefact ;
                    rdfs:range              mod:SemanticArtefactTask ;
                    dcterms:description     "OMV: The purpose for which the ontology was originally designed."@en ;
                    rdfs:isDefinedBy        <http://omv.ontoware.org/2005/05/ontology> ;
                    dcterms:issued          "2009-12-24"^^xsd:date ;
                    pav:derivedFrom         <http://www.isibang.ac.in/ns/mod/1.2> ;
                    pav:importedOn          "2017-07-06"^^xsd:dateTime ;
                    
            #OPTIONAL STATEMENTS
                    prov:wasInfluencedBy    "MIRO guidelines: B.1" ,
                                            "FAIR principle: R1.2" .



### http://purl.org/pav/createdWith
mod:createdWith     rdf:type                owl:ObjectProperty ;
                    rdfs:subPropertyOf      prov:wasAttributedTo ;
                    rdfs:label              "created with"@en ,
                                            "crée avec"@fr ;
                    dcterms:description     "PAV: The software/tool used by the creator (pav:createdBy) when making the digital resource, for instance a word processor or an annotation tool. MOD: The tool used for the creation of an ontology. OMV: Information about the tool used to create the ontology."@en ;
                    rdfs:isDefinedBy        <http://purl.org/pav/> ;
                    dcterms:issued          "2014-08-28"^^xsd:date ;
                    dcterms:relation        omv:usedOntologyEngineeringTool ,
                                            oboinowl:auto-generated-by , 
                                            <http://www.isibang.ac.in/ns/mod/1.0/toolUsed> ;
                    pav:derivedFrom         <http://www.isibang.ac.in/ns/mod/1.0> ;
                    pav:importedOn          "2015-08-05"^^xsd:dateTime ;
            
            #OPTIONAL STATEMENTS
                    prov:wasInfluencedBy    "MIRO guidelines: E.2" ,
                                            "FAIR principle: R1.2" .
        


### https://w3id.org/mod#usedEngineeringMethodology
mod:usedEngineeringMethodology
                    rdf:type                owl:ObjectProperty ;
                    rdfs:label              "engineering methodology"@en ,
                                            "méthodologie de développement"@fr ;
                    rdfs:domain             mod:SemanticArtefact ;
                    rdfs:range              mod:EngineeringMethodology ;
                    dcterms:description     "MOD: A methodolgy follwoing which an ontology is created. OMV: Information about the method model used to create the ontology."@en ;
                    rdfs:isDefinedBy        <http://omv.ontoware.org/2005/05/ontology> ;
                    dcterms:issued          "2009-12-24"^^xsd:date ;
                    dcterms:relation        adms:representationTechnique ,
                                            schema:publishingPrinciples ,
                                            <http://www.isibang.ac.in/ns/mod/1.0/methodologyUsed> ;
                    pav:derivedFrom         <http://www.isibang.ac.in/ns/mod/1.0> ;
                    pav:importedOn          "2015-08-05"^^xsd:dateTime ;
            
            #OPTIONAL STATEMENTS
                    skos:historyNote        "This property has been adopted from OMV Ontology Metadata Vocabulary and redefined in the MOD namespace."@en ;
                    prov:wasInfluencedBy    "MIRO guidelines: A.6" ,
                                            "FAIR principle: R1.2" .
        


### https://w3id.org/mod#conformsToKnowledgeRepresentationParadigm
mod:conformsToKnowledgeRepresentationParadigm
                    rdf:type                owl:ObjectProperty ;
                    rdfs:label              "knowledge representation paradigm"@en ,
                                            "paradigme de représentation des connaissances"@fr ;
                    rdfs:domain             mod:SemanticArtefact ;
                    rdfs:range              mod:KnowledgeRepresentationParadigm ;
                    dcterms:description     "MOD: A representation formalism that is followed to describe knowledge in an ontology. Example includes description logics, first order logic, etc. dcterms: An established standard to which the described resource conforms. OMV: Information about the paradigm model used to create the ontology. DCTERMS: An established standard to which the described resource conforms."@en ;
                    rdfs:isDefinedBy        <http://omv.ontoware.org/2005/05/ontology> ;
                    dcterms:issued          "2009-12-24"^^xsd:date ;
                    dcterms:relation        omv:conformsToKnowledgeRepresentationParadigm , 
                                            dcterms:conformsTo ,
                                            <http://www.isibang.ac.in/ns/mod/1.0/knowledgeRepresentationFormalism> ;
                    pav:derivedFrom         <http://www.isibang.ac.in/ns/mod/1.0> ;
                    pav:importedOn          "2015-08-05"^^xsd:dateTime ;
            
            #OPTIONAL STATEMENTS
                    skos:historyNote        "This property has been adopted from OMV Ontology Metadata Vocabulary and redefined in the MOD namespace."@en ;
                    prov:wasInfluencedBy    "MIRO guidelines: E.1" ,
                                            "FAIR principle: R1.2" .
        


### http://purl.org/dc/terms/coverage
dcterms:coverage    rdf:type                rdf:Property ;
                    rdfs:subPropertyOf      dc:coverage ;
                    rdfs:label              "coverage"@en ,
                                            "couverture"@fr ;
                    dcterms:description     "DCTERMS: The spatial or temporal topic of the resource, the spatial applicability of the resource, or the jurisdiction under which the resource is relevant. Spatial topic and spatial applicability may be a named place or a location specified by its geographic coordinates. Temporal topic may be a named period, date, or date range. A jurisdiction may be a named administrative entity or a geographic place to which the resource applies. Recommended practice is to use a controlled vocabulary such as the Getty Thesaurus of Geographic Names [[TGN](https://www.getty.edu/research/tools/vocabulary/tgn/index.html)]. Where appropriate, named places or time periods may be used in preference to numeric identifiers such as sets of coordinates or date ranges.  Because coverage is so broadly defined, it is preferable to use the more specific subproperties Temporal Coverage and Spatial Coverage."@en ;
                    rdfs:isDefinedBy        <http://purl.org/dc/terms/> ;
                    dcterms:issued          "2008-01-14"^^xsd:date ;
                    pav:derivedFrom         <http://www.isibang.ac.in/ns/mod/1.2> ;
                    pav:importedOn          "2017-07-06"^^xsd:dateTime ;
                    
            #OPTIONAL STATEMENTS
                    prov:wasInfluencedBy    "MIRO guidelines: C.1" ,
                                            "FAIR principle: F2" ;
            
            #OTHER ORIGINAL STATEMENTS IF ANY 
                    <http://purl.org/dc/dcam/rangeIncludes>     dcterms:Jurisdiction, dcterms:Location, dcterms:Period  .



### https://w3id.org/mod#competencyQuestion
mod:competencyQuestion 
                    rdf:type                owl:DatatypeProperty ;
                    rdfs:label              "competency question"@en ,
                                            "question de compétence"@fr ;
                    rdfs:domain             mod:SemanticArtefact ;
                    rdfs:range              xsd:string ;
                    dcterms:description     "A set of questions made to build an ontology at the design time."@en ;
                    rdfs:isDefinedBy        <https://w3id.org/mod> ;
                    dcterms:issued          "2015-08-05"^^xsd:dateTime ;
                    pav:derivedFrom         <http://www.isibang.ac.in/ns/mod/1.0> ;
                    pav:importedOn          "2015-08-05"^^xsd:dateTime ;
                    
            #OPTIONAL STATEMENTS
                    prov:wasInfluencedBy    "MIRO guidelines: A.6, D.3" ,
                                            "FAIR principle: R1.2" .
            
            
                     
### http://xmlns.com/foaf/0.1/depiction
foaf:depiction      rdf:type                rdf:Property , owl:ObjectProperty ;
                    rdfs:label              "depiction"@en ,
                                            "représentation"@fr ;
                    rdfs:domain             owl:Thing ;
                    rdfs:range              foaf:Image ;
                    dcterms:description     "FOAF: A depiction of some thing. DOAP: Web page with screenshots of project. An image of the item. This can be a URL or a fully described ImageObject."@en ;
                    rdfs:isDefinedBy        <http://xmlns.com/foaf/0.1/> ;
                    dcterms:issued          "2014-01-14"^^xsd:date ;
                    dcterms:relation        schema:image ,
                                            doap:screenshots ;
                    pav:derivedFrom          <http://www.isibang.ac.in/ns/mod/1.2> ;
                    pav:importedOn          "2017-07-06"^^xsd:dateTime ;
                    
            #OPTIONAL STATEMENTS
                    prov:wasInfluencedBy    "FAIR principle: F2" ;
            
            #OTHER ORIGINAL STATEMENTS IF ANY 
                    owl:inverseOf           foaf:depicts .
                    


### http://xmlns.com/foaf/0.1/logo
foaf:logo           rdf:type                rdf:Property , owl:InverseFunctionalProperty , owl:ObjectProperty  ;
                    rdfs:label              "logo"@en ,
                                            "logo"@fr ;
                    rdfs:domain             owl:Thing ;
                    rdfs:range              owl:Thing ;
                    dcterms:description     "FOAF: A logo representing some thing. SCHEMA: An associated logo."@en ;
                    rdfs:isDefinedBy        <http://xmlns.com/foaf/0.1/> ;
                    dcterms:issued          "2014-01-14"^^xsd:date ;
                    dcterms:relation        schema:logo ;
                    pav:derivedFrom          <http://www.isibang.ac.in/ns/mod/1.2> ;
                    pav:importedOn          "2017-07-06"^^xsd:dateTime ;
                    
            #OPTIONAL STATEMENTS
                    prov:wasInfluencedBy    "FAIR principle: F2" ;
            
            #OTHER ORIGINAL STATEMENTS IF ANY 
                    owl:inverseOf           foaf:depicts .
                    



### http://xmlns.com/foaf/0.1/homepage
foaf:homepage       rdf:type                rdf:Property , owl:InverseFunctionalProperty , owl:ObjectProperty  ;
                    rdfs:subPropertyOf      foaf:page , foaf:isPrimaryTopicOf ;
                    rdfs:label              "homepage"@en ,
                                            "page web"@fr ;
                    rdfs:domain             owl:Thing ;
                    rdfs:range              owl:Document ;
                    dcterms:description     "FOAF: A homepage for some thing. MOD: An unambiguous reference to the resource within a given context. DOAP: URI of a blog related to a project. CC: The URL the creator of a Work would like used when attributing re-use. SCHEMA: Indicates a page (or other CreativeWork) for which this thing is the main entity being described."@en ;
                    rdfs:isDefinedBy        <http://xmlns.com/foaf/0.1/> ;
                    dcterms:issued          "2014-01-14"^^xsd:date ;
                    dcterms:relation        schema:mainEntityOfPage ,
                                            cc:attributionURL ,
                                            doap:blog ,
                                            <http://www.isibang.ac.in/ns/mod/1.0/homepage> ;
                    pav:derivedFrom          <http://www.isibang.ac.in/ns/mod/1.0> ;
                    pav:importedOn          "2015-08-05"^^xsd:dateTime ;
                    
            #OPTIONAL STATEMENTS
                    prov:wasInfluencedBy    "MIRO guidelines: C.3" ,
                                            "FAIR principle: F2" .
            


### http://purl.org/dc/terms/accessRights
dcterms:accessRights
                    rdf:type                rdf:Property ;
                    rdfs:subPropertyOf      dc:rights , dcterms:rights ;
                    rdfs:label              "access rights"@en ,
                                            "droits d'accès"@fr ;
                    dcterms:description     "DCTERMS: Information about who access the resource or an indication of its security status. Access Rights may include information regarding access or restrictions based on privacy, security, or other policies. MOD: Information on access (i.e., read, download) to an ontology."@en ;
                    rdfs:isDefinedBy        <http://purl.org/dc/terms/> ;
                    dcterms:issued          "2003-02-15"^^xsd:date ;
                    dcterms:relation        <http://www.isibang.ac.in/ns/mod/1.0/accessibility> ;
                    pav:derivedFrom         <http://www.isibang.ac.in/ns/mod/1.0> ;
                    pav:importedOn          "2015-08-05"^^xsd:dateTime ;
                    
            #OPTIONAL STATEMENTS
                    prov:wasInfluencedBy    "FAIR principle: R1.1" ;
            
            #OTHER ORIGINAL STATEMENTS IF ANY 
                    <http://purl.org/dc/dcam/rangeIncludes>     dcterms:RightsStatement .


    
### https://vocab.org/vann/changes
vann:changes        rdf:type                owl:AnnotationProperty ;
                    rdfs:subPropertyOf      rdfs:seeAlso ;
                    rdfs:label              "changes"@en ,
                                            "changements"@fr ;
                    dcterms:description     "VANN: A reference to a resource that describes changes between this version of a vocabulary and the previous."@en ;
                    rdfs:isDefinedBy        <http://purl.org/vocab/vann/> ;
                    dcterms:issued          "2005-04-01"^^xsd:date ;
                    pav:derivedFrom         <http://www.isibang.ac.in/ns/mod/1.2> ;
                    pav:importedOn          "2017-07-06"^^xsd:dateTime ;
                    
            #OPTIONAL STATEMENTS
                    prov:wasInfluencedBy    "FAIR principle: R1.2" .



### https://vocab.org/vann/example
vann:example        rdf:type                owl:AnnotationProperty ;
                    rdfs:subPropertyOf      rdfs:seeAlso ;
                    rdfs:label              "example"@en ,
                                            "exemple"@fr ;
                    dcterms:description     "VANN: A reference to a resource that provides an example of how this resource can be used. SCHEMA: Example/instance/realization/derivation of the concept of this creative work. eg. The paperback edition, first edition, or eBook."@en ;
                    rdfs:isDefinedBy        <http://purl.org/vocab/vann/> ;
                    dcterms:issued          "2005-04-01"^^xsd:date ;
                    dcterms:relation        schema:workExample ;
         
                    pav:derivedFrom         <http://www.isibang.ac.in/ns/mod/1.2> ;
                    pav:importedOn          "2017-07-06"^^xsd:dateTime ;
                    
            #OPTIONAL STATEMENTS
                    prov:wasInfluencedBy    "MIRO guidelines: G.3" ,
                                            "FAIR principle: F2" .



### http://purl.org/vocab/vann/preferredNamespaceUri
vann:preferredNamespaceUri 
                    rdf:type                owl:AnnotationProperty ;
                    rdfs:label              "preferred namespace URI"@en ,
                                            "URI préféré d'espace de nom"@fr ;
                    dcterms:description     "VANN: The preferred namespace URI to use when using terms from this vocabulary in an XML document. VOID: A URI that is a common string prefix of all the entity URIs in a void:Dataset."@en ;
                    rdfs:isDefinedBy        <http://purl.org/vocab/vann/> ;
                    dcterms:issued          "2005-04-01"^^xsd:date ;
                    dcterms:relation        void:uriSpace ;
                    pav:derivedFrom         <http://www.isibang.ac.in/ns/mod/1.2> ;
                    pav:importedOn          "2017-07-06"^^xsd:dateTime ;
                    
            #OPTIONAL STATEMENTS
                    prov:wasInfluencedBy    "MIRO guidelines: E.5" ,
                                            "FAIR principle: F2" .
            


### http://purl.org/vocab/vann/preferredNamespacePrefix
vann:preferredNamespacePrefix
                    rdf:type                owl:AnnotationProperty ;
                    rdfs:label              "preferred namespace prefix"@en ,
                                            "préfixe d'espace de nom préféré"@fr  ;
                    dcterms:description     "VANN: The preferred namespace prefix to use when using terms from this vocabulary in an XML document. IDOT: Short label that is commonly used to refer to the dataset. Often utilised to identify the dataset in IRIs for specific items (or records). This may also stand in place of the base IRI of the dataset (e.g. see http://prefix.cc)."@en ; 
                    rdfs:isDefinedBy        <http://purl.org/vocab/vann/> ;
                    dcterms:issued          "2005-04-01"^^xsd:date ;
                    dcterms:relation        idot:preferredPrefix ,
                                            oboinowl:default-namespace ,
                                            oboinowl:hasDefaultNamespace ;
                    pav:derivedFrom         <http://www.isibang.ac.in/ns/mod/1.2> ;
                    pav:importedOn          "2017-07-06"^^xsd:dateTime ;
                    
            #OPTIONAL STATEMENTS
                    prov:wasInfluencedBy    "MIRO guidelines: E.11" ,
                                            "FAIR principle: F2" .
            


### https://w3id.org/mod#prefLabelProperty
mod:prefLabelProperty
                    rdf:type                owl:DatatypeProperty ;
                    rdfs:label              "object preferred label property"@en ,
                                            "propriété de nom préféré des objets"@fr ;
                    rdfs:domain             mod:SemanticArtefactDistribution ;
                    rdfs:range              xsd:anyURI ;
                    dcterms:description     "MOD: Property used to specify objects' preferred label."@en ;
                    rdfs:isDefinedBy        <https://w3id.org/mod> ;
                    dcterms:issued          "2018-08-02"^^xsd:date ;
                    pav:derivedFrom         <http://www.isibang.ac.in/ns/mod/1.4> ;
                    pav:importedOn          "2018-08-02"^^xsd:dateTime ;

            #OPTIONAL STATEMENTS
                    prov:wasInfluencedBy    "MIRO guidelines: E.7" ,
                                            "FAIR principle: R1" .
                        


### https://w3id.org/mod#synonymProperty
mod:synonymProperty rdf:type                owl:DatatypeProperty ;
                    rdfs:label              "object synonym property"@en ,
                                            "propriété de synonyme des objets"@fr ;
                    rdfs:domain             mod:SemanticArtefactDistribution ;
                    rdfs:range              xsd:anyURI ;
                    dcterms:description     "MOD: Property used to specify objects' synonyms."@en ;
                    rdfs:isDefinedBy        <https://w3id.org/mod> ;
                    dcterms:issued          "2018-08-02"^^xsd:date ;
                    dcterms:relation        oboinowl:hasSynonymType ,
                                            oboinowl:synonymtypedef ;
                    pav:derivedFrom         <http://www.isibang.ac.in/ns/mod/1.4> ;
                    pav:importedOn          "2018-08-02"^^xsd:dateTime ;
                    
            #OPTIONAL STATEMENTS
                    prov:wasInfluencedBy    "MIRO guidelines: E.7" ,
                                            "FAIR principle: R1" .



                        

### https://w3id.org/mod#definitionProperty
mod:definitionProperty 
                    rdf:type                owl:DatatypeProperty ;
                    rdfs:label              "object definition property"@en ,
                                            "propriété de définition des objets"@fr ;
                    rdfs:domain             mod:SemanticArtefactDistribution ;
                    rdfs:range              xsd:anyURI ;
                    dcterms:description     "MOD: Property used to specify objects' definition."@en ;
                    rdfs:isDefinedBy        <https://w3id.org/mod> ;
                    dcterms:issued          "2018-08-02"^^xsd:date ;
                    pav:derivedFrom         <http://www.isibang.ac.in/ns/mod/1.4> ;
                    pav:importedOn          "2018-08-02"^^xsd:dateTime ;
                    
            #OPTIONAL STATEMENTS
                    prov:wasInfluencedBy    "MIRO guidelines: E.7" ,
                                            "FAIR principle: R1" .
                    


### https://w3id.org/mod#authorProperty
mod:authorProperty  rdf:type                owl:DatatypeProperty ;
                    rdfs:label              "object author property"@en ,
                                            "propriété d'auteur des objets"@fr ;
                    rdfs:domain             mod:SemanticArtefactDistribution ;
                    rdfs:range              xsd:anyURI ;
                    dcterms:description     "MOD: Property used to specify objects's author."@en ;
                    rdfs:isDefinedBy        <https://w3id.org/mod> ;
                    dcterms:issued          "2018-08-02"^^xsd:date ;
                    pav:derivedFrom         <http://www.isibang.ac.in/ns/mod/1.4> ;
                    pav:importedOn          "2018-08-02"^^xsd:dateTime ;
                   
            #OPTIONAL STATEMENTS
                    prov:wasInfluencedBy    "MIRO guidelines: E.7" ,
                                            "FAIR principle: R1" .



### https://w3id.org/mod#obsoleteProperty
mod:obsoleteProperty
                    rdf:type               owl:DatatypeProperty ;
                    rdfs:label              "object obsolete property"@en ,
                                            "propriété d'obsolescence des objets"@fr ;
                    rdfs:domain             mod:SemanticArtefactDistribution ;
                    rdfs:range              xsd:anyURI ;
                    dcterms:description     "MOD: Property used to specify obsolete objects."@en ;
                    rdfs:isDefinedBy        <https://w3id.org/mod> ;
                    dcterms:issued          "2018-08-02"^^xsd:date ;
                    pav:derivedFrom         <http://www.isibang.ac.in/ns/mod/1.4> ;
                    pav:importedOn          "2018-08-02"^^xsd:dateTime ;
                    
            #OPTIONAL STATEMENTS
                    prov:wasInfluencedBy    "MIRO guidelines: E.7" ,
                                            "FAIR principle: R1" .



### https://w3id.org/mod#hierarchyProperty
mod:hierarchyProperty
                    rdf:type                owl:DatatypeProperty ;
                    rdfs:label              "transitive hierarchy property"@en ,
                                            "propriété de hiérarchie transitive"@fr ;
                    rdfs:domain             mod:SemanticArtefactDistribution ;
                    rdfs:range              xsd:anyURI ;
                    dcterms:description     "MOD: Property used to specify the hierarchy (e.g. rdfs:subClassOf or skos:broader)."@en ;
                    rdfs:isDefinedBy        <https://w3id.org/mod> ;
                    dcterms:issued          "2018-08-02"^^xsd:date ;
                    pav:derivedFrom         <http://www.isibang.ac.in/ns/mod/1.4> ;
                    pav:importedOn          "2018-08-02"^^xsd:dateTime ;

            #OPTIONAL STATEMENTS
                    prov:wasInfluencedBy    "MIRO guidelines: E.9" ,
                                            "FAIR principle: R1" .



### https://w3id.org/mod#obsoleteParent
mod:obsoleteParent
                    rdf:type                owl:DatatypeProperty ;
                    rdfs:label              "transitive hierarchy property"@en ,
                                            "propriété de hiérarchie transitive"@fr ;
                    rdfs:domain             mod:SemanticArtefactDistribution ;
                    rdfs:range              xsd:anyURI ;
                    dcterms:description     "MOD: Property used to specify the root of an obsolete branch in the ontology."@en ;
                    rdfs:isDefinedBy        <https://w3id.org/mod> ;
                    dcterms:issued          "2018-08-02"^^xsd:date ;
                    pav:derivedFrom         <http://www.isibang.ac.in/ns/mod/1.4> ;
                    pav:importedOn          "2018-08-02"^^xsd:dateTime ;

            #OPTIONAL STATEMENTS
                    prov:wasInfluencedBy    "FAIR principle: R1" .




### http://rdfs.org/ns/void#uriRegexPattern
void:uriRegexPattern
                    rdf:type                rdf:Property ;
                    rdfs:label              "identifier pattern"@en ,
                                            "patron d'identifiant"@fr ;
                    rdfs:domain             void:Dataset ;
                    dcterms:description     "VOID: A regular expression that matches the URIs of a void:Dataset's entities. IDOT: Regular expression describing alphanumeric strings used to identify items (or records) in a dataset."@en ;
                    rdfs:isDefinedBy        <http://vocab.deri.ie/void> ;
                    dcterms:issued          "2010-01-26"^^xsd:date ;
                    dcterms:relation        idot:identifierPattern ;
                    pav:derivedFrom         <http://www.isibang.ac.in/ns/mod/1.4> ;
                    pav:importedOn          "2018-08-02"^^xsd:dateTime ;
                    
            #OPTIONAL STATEMENTS
                    prov:wasInfluencedBy    "MIRO guidelines: E.6" ,
                                            "FAIR principle: F2" .



### https://w3id.org/mod#toDoList
mod:toDoList        rdf:type                owl:ObjectProperty ;
                    rdfs:label              "to-do list"@en ,
                                            "liste des choses à faire"@fr;
                    rdfs:range              <http://www.w3.org/2002/12/cal/ical#Vtodo> ;
                    dcterms:description     "VOID: Describes future tasks planned by a resource curator. This property is primarily intended to be used for vocabularies or datasets, but the domain is left open, it can be used for any resource. Use iCalendar Vtodo class and its properties to further describe the task calendar, priorities etc."@en ;    
                    rdfs:isDefinedBy        <http://purl.org/vocommons/voaf> ;
                    dcterms:issued          "2013-05-23"^^xsd:date ;
                    dcterms:relation        voaf:toDoList ;
                    pav:derivedFrom         <http://www.isibang.ac.in/ns/mod/1.4> ;
                    pav:importedOn          "2018-08-02"^^xsd:dateTime ;
                    
            #OPTIONAL STATEMENTS
                    skos:historyNote        "This property had been originally defined by VOAF metadata vocabulary. Now, it has been adopted and redefined in the MOD namespace."@en ;
                    prov:wasInfluencedBy    "FAIR principle: F2" .
            


### http://rdfs.org/ns/void#exampleResource
void:exampleResource
                    rdf:type                rdf:Property ;
                    rdfs:label              "example de resource"@en ,
                                            "exemple de resource"@fr;
                    rdfs:domain             void:Dataset ;
                    rdfs:range              rdfs:Resource ;
                    dcterms:description     "VOID: Example resource of dataset. IDOT: An example identifier used by one item (or record) from a dataset."@en ;
                    rdfs:isDefinedBy        <http://vocab.deri.ie/void> ;
                    dcterms:issued          "2010-01-26"^^xsd:date ;
                    dcterms:relation        idot:exampleIdentifier ;
                    pav:derivedFrom         <http://www.isibang.ac.in/ns/mod/1.4> ;
                    pav:importedOn          "2018-08-02"^^xsd:dateTime ;
                    
            #OPTIONAL STATEMENTS
                    prov:wasInfluencedBy    "MIRO guidelines: E.6" ,
                                            "FAIR principle: F2" .
            

### http://schema.org/award
schema:award        rdf:type                rdf:Property ;
                    rdfs:label              "award"@en ,
                                            "prix"@fr ;
                    dcterms:description     "SCHEMA: An award won by or for this item."@en ;
                    rdfs:isDefinedBy        <http://schema.org/> ;
                    dcterms:issued          "2012-04-21"^^xsd:date ;
                    pav:derivedFrom         <http://www.isibang.ac.in/ns/mod/1.4> ;
                    pav:importedOn          "2018-08-02"^^xsd:dateTime ;
                    
            #OPTIONAL STATEMENTS
                    prov:wasInfluencedBy    "FAIR principle: F2" ;
            
            #OTHER ORIGINAL STATEMENTS IF ANY 
                    schema:domainIncludes   schema:CreativeWork, schema:Organization, schema:Person, schema:Product, schema:Service ;
                    schema:rangeIncludes    schema:Text .



### http://schema.org/associatedMedia
schema:associatedMedia
                    rdf:type                rdf:Property ;
                    rdfs:label              "associated media"@en ,
                                            "média associé"@fr  ;
                    dcterms:description     "SCHEMA: A media object that encodes this CreativeWork. This property is a synonym for encoding."@en ;
                    rdfs:isDefinedBy        <http://schema.org/> ;
                    dcterms:issued          "2012-04-21"^^xsd:date ;
                    pav:derivedFrom         <http://www.isibang.ac.in/ns/mod/1.4> ;
                    pav:importedOn          "2014-07-28"^^xsd:dateTime ;
                    
            #OPTIONAL STATEMENTS
                    prov:wasInfluencedBy    "FAIR principle: F2" ;
            
            #OTHER ORIGINAL STATEMENTS IF ANY 
                    schema:domainIncludes   schema:CreativeWork, schema:HyperToc, schema:HyperTocEntry ;
                    schema:rangeIncludes    schema:MediaObject .



### http://schema.org/includedInDataCatalog
schema:includedInDataCatalog
                    rdf:type                rdf:Property ;
                    rdfs:label              "Indexed or included in catalog or repository"@en ,
                                            "indexé ou inclus dans un catalogue ou un entrepôt"@fr ;
                    dcterms:description     "SCHEMA: A data catalog which contains this dataset."@en ;
                    rdfs:isDefinedBy        <http://schema.org/> ;
                    dcterms:issued          "2016-05-04"^^xsd:date ;
                    pav:derivedFrom         <http://www.isibang.ac.in/ns/mod/1.4> ;
                    pav:importedOn          "2014-07-28"^^xsd:dateTime ;
                    
            #OPTIONAL STATEMENTS
                    prov:wasInfluencedBy    "FAIR principle: F4, A1.1, A1.2" ;
            
            #OTHER ORIGINAL STATEMENTS IF ANY 
                    schema:domainIncludes   schema:Dataset ;
                    schema:inverseOf        schema:dataset ;
                    schema:rangeIncludes    schema:DataCatalog .



########################################################
########## People and organization properties ##########
########################################################
    
### http://purl.org/dc/terms/creator
dcterms:creator     rdf:type                rdf:Property ;
                    rdfs:subPropertyOf      dc:creator , dcterms:contributor ;
                    rdfs:label              "creator"@en ,
                                            "créateur"@fr ;
                    dcterms:description     "DCTERMS: An entity responsible for making the resource. Recommended practice is to identify the creator with a URI.  If this is not possible or feasible, a literal value that identifies the creator may be provided."@en ;
                    rdfs:isDefinedBy        <http://purl.org/dc/terms/> ;
                    dcterms:issued          "2008-01-14"^^xsd:date ;
                    dcterms:relation        omv:creator ,
                                            pav:authoredBy ,
                                            pav:createdBy ,
                                            schema:author ,
                                            doap:maintainer ,
                                            prov:wasAttributedTo ,
                                            foaf:maker ;
                    pav:derivedFrom         <http://www.isibang.ac.in/ns/mod/1.0> ;
                    pav:importedOn          "2015-08-05"^^xsd:dateTime ;
                    
            #OPTIONAL STATEMENTS
                    prov:wasInfluencedBy    "MIRO guidelines: C.2" , 
                                            "FAIR principle: F2" ;
            
            #OTHER ORIGINAL STATEMENTS IF ANY 
                    <http://purl.org/dc/dcam/rangeIncludes>     dcterms:Agent .



### http://purl.org/dc/terms/contributor
dcterms:contributor rdf:type                rdf:Property ;
                    rdfs:subPropertyOf      dc:contributor ;
                    rdfs:label              "contributor"@en ,
                                            "contributeur"@fr ;
                    dcterms:description     "DCTERMS: An entity responsible for making contributions to the resource. OMV: Contributors to the creation of the ontology. PAV: The resource was contributed to by the given agent. SCHEMA: A secondary contributor to the CreativeWork or Event. DOAP: Project contributor."@en ;
                    rdfs:isDefinedBy        <http://purl.org/dc/terms/> ;
                    dcterms:issued          "2008-01-14"^^xsd:date ;
                    dcterms:relation        omv:hasContributor ,
                                            pav:contributedBy ,
                                            schema:contributor ,
                                            doap:developer ,
                                            doap:helper ,
                                            oboinowl:saved-by ,
                                            oboinowl:savedBy  ;
                    pav:derivedFrom         <http://www.isibang.ac.in/ns/mod/1.0> ;
                    pav:importedOn          "2015-08-05"^^xsd:dateTime ;
                    
            #OPTIONAL STATEMENTS
                    prov:wasInfluencedBy    "MIRO guidelines: C.2" , 
                                            "FAIR principle: F2" ;
            
            #OTHER ORIGINAL STATEMENTS IF ANY 
                    <http://purl.org/dc/dcam/rangeIncludes>     dcterms:Agent .



### http://purl.org/dc/terms/publisher
dcterms:publisher   rdf:type                rdf:Property ;
                    rdfs:subPropertyOf      dc:publisher ;
                    rdfs:label              "publisher"@en ,
                                            "éditeur"@fr ;
                    dcterms:description     "DDCTERMS: An entity responsible for making the resource available."@en ;
                    rdfs:isDefinedBy        <http://purl.org/dc/terms/> ;
                    dcterms:issued          "2008-01-14"^^xsd:date ;
                    dcterms:relation        schema:publisher ,
                                            adms:schemaAgency ;
                    pav:derivedFrom         <http://www.isibang.ac.in/ns/mod/1.0> ;
                    pav:importedOn          "2015-08-05"^^xsd:dateTime ;
                    
            #OPTIONAL STATEMENTS
                    prov:wasInfluencedBy    "MIRO guidelines: A.2" , 
                                            "FAIR principle: F2" ;
            
            #OTHER ORIGINAL STATEMENTS IF ANY 
                    <http://purl.org/dc/dcam/rangeIncludes>     dcterms:Agent .



### http://purl.org/pav/curatedBy
mod:curatedBy       rdf:type                owl:ObjectProperty ;
                    rdfs:subPropertyOf      pav:contributedBy ;
                    rdfs:label              "curated by"@en ,
                                            "contrôlé par"@fr ;
                    dcterms:description     "PAV: Specifies an agent specialist responsible for shaping the expression in an appropriate format. Often the primary agent responsible for ensuring the quality of the representation. MOD: A curator who restructure the previously authored content and shape it to be appropriate for the intended representation (e.g. by normalizing the fields for being represented in a spreadsheet). "@en ;
                    rdfs:isDefinedBy        <http://purl.org/pav/> ;
                    dcterms:issued          "2014-08-28"^^xsd:date ;
                    pav:derivedFrom         <http://www.isibang.ac.in/ns/mod/1.2> ;
                    pav:importedOn          "2017-07-06"^^xsd:dateTime ;
            
            #OPTIONAL STATEMENTS
                    prov:wasInfluencedBy    "MIRO guidelines: C.2" ,
                                            "FAIR principle: F2" ;
        
            #OTHER ORIGINAL STATEMENTS IF ANY 
                    owl:inverseOf           pav:curates ;
                    rdfs:seeAlso            pav:createdBy , 
                                            pav:curatedOn .



### http://schema.org/translator
schema:translator   rdf:type                rdf:Property ;
                    rdfs:label              "translator"@en ,
                                            "traducteur"@fr ;
                    dcterms:description     "SCHEMA: Organization or person who adapts a creative work to different languages, regional differences and technical requirements of a target market, or that translates during some event."@en ;
                    rdfs:isDefinedBy        <http://schema.org/> ;
                    dcterms:issued          "2012-04-21"^^xsd:date ;
                    pav:derivedFrom         <http://www.isibang.ac.in/ns/mod/1.4> ;
                    pav:importedOn          "2018-08-02"^^xsd:dateTime ;
                    
            #OPTIONAL STATEMENTS
                    prov:wasInfluencedBy    "FAIR principle: F2" ;
            
            #OTHER ORIGINAL STATEMENTS IF ANY 
                    schema:domainIncludes   schema:CreativeWork, schema:Event ;
                    schema:rangeIncludes    schema:Organization, schema:Person .



### http://purl.org/dc/terms/rightsHolder
dcterms:rightsHolder
                    rdf:type                rdf:Property ;
                    rdfs:label              "rights holder"@en ,
                                            "détenteur des droits"@fr ;
                    rdfs:range              dcterms:Agent ;
                    dcterms:description     "DCTERMS: A person or organization owning or managing rights over the resource. MOD: The person who can be contacted to enquire about an ontology. SCHEMA: The party holding the legal copyright to the CreativeWork. DCAT: Relevant contact information for the cataloged resource. Use of vCard is recommended."@en ;
                    rdfs:isDefinedBy        <http://purl.org/dc/terms/> ;
                    dcterms:issued          "2004-06-14"^^xsd:date ;
                    dcterms:relation        schema:copyrightHolder ,
                                            dcat:contactPoint ;
                    pav:derivedFrom         <http://www.isibang.ac.in/ns/mod/1.2> ;
                    pav:importedOn          "2017-07-06"^^xsd:dateTime ;
                    
            #OPTIONAL STATEMENTS
                    prov:wasInfluencedBy    "MIRO guidelines: A.2" , 
                                            "FAIR principle: R1.1" ;
            
            #OTHER ORIGINAL STATEMENTS IF ANY 
                    <http://purl.org/dc/dcam/rangeIncludes>     dcterms:Agent .


                 
##########################################
########## Grouping properties ##########
##########################################


### http://purl.org/dc/terms/subject
dcterms:subject     rdf:type                rdf:Property ;
                    rdfs:subPropertyOf      dc:subject ;
                    rdfs:label              "subject"@en ,
                                            "sujet"@fr ;
                    dcterms:description     "DCTERMS: The topic of the resource. OMV: Typically, the domain can refer to established topic hierarchies such as the general purpose topic hierarchy DMOZ or the domain specific topic hierarchy ACM for the computer science domain. SCHEMA: The subject matter of the content. DCAT: A main category of the resource. A resource can have multiple themes. FOAF: A topic of some page or document."@en ;
                    rdfs:isDefinedBy        <http://purl.org/dc/terms/> ;
                    dcterms:issued          "2008-01-14"^^xsd:date ;
                    dcterms:relation        omv:hasDomain ,
                                            schema:about ,
                                            dcat:theme ,
                                            foaf:topic ;
                    pav:derivedFrom         <http://www.isibang.ac.in/ns/mod/1.0> ;
                    pav:importedOn          "2015-08-05"^^xsd:dateTime ;
                    
            #OPTIONAL STATEMENTS
                    prov:wasInfluencedBy    "MIRO guidelines: C.1" , 
                                            "FAIR principle: F2" .



### https://w3id.org/mod#group
mod:group           rdf:type                owl:ObjectProperty ;
                    rdfs:label              "group"@en ,
                                            "groupe"@fr ;
                    rdfs:domain             mod:SemanticArtefact ;
                    rdfs:range              mod:Group ;
                    dcterms:description     "MOD: A group of ontologies that the ontology is usually considered into."@en ;
                    rdfs:isDefinedBy        <https://w3id.org/mod> ;
                    dcterms:issued          "2017-07-06"^^xsd:date ;
                    pav:derivedFrom         <http://www.isibang.ac.in/ns/mod/1.2> ;
                    pav:importedOn          "2017-07-06"^^xsd:dateTime ;
            
            #OPTIONAL STATEMENTS
                    prov:wasInfluencedBy    "FAIR principle: R1.3" .
            


##########################################
########## Relation properties ##########
##########################################

### http://www.w3.org/2002/07/owl#imports
owl:imports         rdf:type                owl:OntologyProperty  ;
                    rdfs:label              "imports"@en ,
                                            "importe"@fr ;
                    rdfs:domain             owl:Ontology ;
                    rdfs:range              owl:Ontology ;
                    dcterms:description     "OWL: References another OWL ontology containing definitions, whose meaning is considered to be part of the meaning of the importing ontology. OMV: References another ontology metadata instance that describes an ontology containing definitions, whose meaning is considered to be part of the meaning of the ontology described by this ontology metadata instance. DCTERMS: A related resource that is required by the described resource to support its function, delivery, or coherence. VOAF: Indicates that the subject vocabulary extends the expressivity of the object vocabulary by declaring subsumption relationships, using object vocabulary class as domain or range of a subject vocabulary property, defining local restrictions etc ...."@en ;  
                    rdfs:isDefinedBy        <http://www.w3.org/2002/07/owl#> ;
                    dcterms:issued          "2004-02-10"^^xsd:date ;
                    dcterms:relation        omv:useImports ,
                                            dcterms:requires ,
                                            voaf:extends ;
                    pav:derivedFrom         <http://www.isibang.ac.in/ns/mod/1.2> ;
                    pav:importedOn          "2017-07-06"^^xsd:dateTime ;
        
            #OPTIONAL STATEMENTS
                    prov:wasInfluencedBy    "MIRO guidelines: E.4" ,
                                            "FAIR principle: I2" .



### http://www.w3.org/2002/07/owl#PriorVersion
owl:PriorVersion    rdf:type                owl:AnnotationProperty, owl:OntologyProperty  ;
                    rdfs:label              "prior version"@en ,
                                            "version précédente"@fr ;
                    rdfs:domain             owl:Ontology ;
                    rdfs:range              owl:Ontology ; 
                    dcterms:description     "OWL:  This identifies the specified ontology as a prior version of the containing ontology. OMV: Contains a reference to another ontology metadata instance. DCTERMS: A related resource of which the described resource is a version, edition, or adaptation. PROV: A revision is a derivation for which the resulting entity is a revised version of some original. The implication here is that the resulting entity contains substantial content from the original. DOOR: Prior version relation from OWL. ADMS: A link to the previous version of the Asset."@en ;  
                    rdfs:isDefinedBy        <http://www.w3.org/2002/07/owl#> ;
                    dcterms:issued          "2004-02-10"^^xsd:date ;
                    dcterms:relation        omv:hasPriorVersion ,
                                            dcterms:isVersionOf ,
                                            prov:wasRevisionOf ,
                                            door:priorVersion ,
                                            adms:prev ;
                    pav:derivedFrom         <http://www.isibang.ac.in/ns/mod/1.2> ;
                    pav:importedOn          "2017-07-06"^^xsd:dateTime ;
        
            #OPTIONAL STATEMENTS
                    prov:wasInfluencedBy    "MIRO guidelines: A.5" ,
                                            "FAIR principle: I2" .



### http://www.w3.org/2002/07/owl#backwardCompatibleWith
owl:backwardCompatibleWith
                    rdf:type                owl:AnnotationProperty, owl:OntologyProperty  ;
                    rdfs:label              "backward compatible"@en ,
                                            "rétrocompatible"@fr ;
                    rdfs:domain             owl:Ontology ;
                    rdfs:range              owl:Ontology ; 
                    dcterms:description     "OWL: This identifies the specified ontology as a prior version of the containing ontology, and further indicates that it is backward compatible with it. OMV: The ontology metadata instance which describes an ontology that is a compatible prior version of the ontology described by this ontology metadata Instance. DOOR: The relation of being a compatible new version from owl."@en ;  
                    rdfs:isDefinedBy        <http://www.w3.org/2002/07/owl#> ;
                    dcterms:issued          "2004-02-10"^^xsd:date ;
                    dcterms:relation        omv:isBackwardCompatibleWith ,
                                            door:backwardCompatibleWith ;
                    pav:derivedFrom         <http://www.isibang.ac.in/ns/mod/1.2> ;
                    pav:importedOn          "2017-07-06"^^xsd:dateTime ;
        
            #OPTIONAL STATEMENTS
                    prov:wasInfluencedBy    "MIRO guidelines: E.8,E.10" ,
                                            "FAIR principle: I2" .



### http://www.w3.org/2002/07/owl#incompatibleWith
owl:incompatibleWith
                    rdf:type                owl:AnnotationProperty, owl:OntologyProperty  ;
                    rdfs:label              "incompatible"@en ,
                                            "incomaptible"@fr ;
                    rdfs:domain             owl:Ontology ;
                    rdfs:range              owl:Ontology ; 
                    dcterms:description     "OWL: This indicates that the containing ontology is a later version of the referenced ontology, but is not backward compatible with it. OMV: The described ontology is a later version of the ontology described by the metadata specified, but is not backward compatible with it. It can be used to explicitly state that ontology cannot upgrade to use the new version without checking whether changes are required. "@en ;  
                    rdfs:isDefinedBy        <http://www.w3.org/2002/07/owl#> ;
                    dcterms:issued          "2004-02-10"^^xsd:date ;
                    dcterms:relation        omv:isIncompatibleWith ,
                                            door:owlIncompatibleWith ;
                    pav:derivedFrom         <http://www.isibang.ac.in/ns/mod/1.2> ;
                    pav:importedOn          "2017-07-06"^^xsd:dateTime ;
        
            #OPTIONAL STATEMENTS
                    prov:wasInfluencedBy    "FAIR principle: I2" .
            
            

### http://purl.org/dc/terms/isPartOf
dcterms:isPartOf    rdf:type                rdf:Property ;
                    rdfs:subPropertyOf      dc:relation , dcterms:relation ;
                    rdfs:label              "is part of (view of)"@en ,
                                            "est partie (une vue) de"@fr ;
                    dcterms:description     "DCTERMS: A related resource in which the described resource is physically or logically included. MOD: Shall be used to identify a subset or a view of an ontology. DOOR: An ontology is included in another if its model is contained in the one of the other ontology. SCHEMA: Indicates an item or CreativeWork that this item, or CreativeWork (in some sense), is part of."@en ;
                    rdfs:isDefinedBy        <http://purl.org/dc/terms/> ;
                    dcterms:issued          "2000-07-11"^^xsd:date ;
                    dcterms:relation        door:includedIn ,
                                            void:subset , 
                                            schema:isPartOf ,
                                            <http://www.isibang.ac.in/ns/mod/1.1/module> ;
                    pav:derivedFrom         <http://www.isibang.ac.in/ns/mod/1.0> ;
                    pav:importedOn          "2015-08-05"^^xsd:dateTime ;
                    
            #OPTIONAL STATEMENTS
                    prov:wasInfluencedBy    "FAIR principle: F2" .
            


### http://purl.org/dc/terms/hasPart
dcterms:hasPart     rdf:type                rdf:Property ;
                    rdfs:subPropertyOf      dc:relation , dcterms:relation ;
                    rdfs:label              "has part (has view)"@en ,
                                            "a pour partie (vue)"@fr ;
                    dcterms:description     "DCTERMS: A related resource that is included either physically or logically in the described resource. SCHEMA: Indicates an item or CreativeWork that is part of this item, or CreativeWork (in some sense). ADMS: Links to a sample of an Asset (which is itself an Asset)."@en ;
                    rdfs:isDefinedBy        <http://purl.org/dc/terms/> ;
                    dcterms:issued          "2000-07-11"^^xsd:date ;
                    dcterms:relation        schema:hasPart ,
                                            adms:sample , 
                                            oboinowl:hasSubset ;
                    pav:derivedFrom        <http://www.isibang.ac.in/ns/mod/1.0> ;
                    pav:importedOn          "2015-08-05"^^xsd:dateTime ;
                    
            #OPTIONAL STATEMENTS
                    prov:wasInfluencedBy    "FAIR principle: F2" .



### http://purl.org/dc/terms/hasVersion
dcterms:hasVersion  rdf:type                rdf:Property ;
                    rdfs:subPropertyOf      dc:relation , dcterms:relation ;
                    rdfs:label              "has version"@en ,
                                            "a pour version"@fr ;
                    dcterms:description     "DCTERMS: a related resource that is a version, edition, or adaptation of the described resource. MOD: A related ontology that is a version, edition, or adtapation of the described ontology. PAV: This resource has a more specific, versioned resource."@en ;
                    rdfs:isDefinedBy        <http://purl.org/dc/terms/> ;
                    dcterms:issued          "2000-07-11"^^xsd:date ;
                    dcterms:relation        schema:hasPart ,
                                            pav:hasVersion , 
                                            <http://www.isibang.ac.in/ns/mod/1.2/version> ;
                    pav:derivedFrom         <http://www.isibang.ac.in/ns/mod/1.2> ;
                    pav:importedOn          "2017-07-06"^^xsd:dateTime ;
                    
            #OPTIONAL STATEMENTS
                    prov:wasInfluencedBy    "FAIR principle: A2,R1.2" .
            


### http://purl.org/dc/terms/isFormatOf
dcterms:isFormatOf  rdf:type                rdf:Property ;
                    rdfs:subPropertyOf      dc:relation , dcterms:relation ;
                    rdfs:label              "is format of"@en ,
                                            "est le format de"@fr ;
                    dcterms:description     "DCTERMS: A related resource that is substantially the same as the described resource, but in another format."@en ;
                    rdfs:isDefinedBy        <http://purl.org/dc/terms/> ;
                    dcterms:issued          "2000-07-11"^^xsd:date ;
                    dcterms:relation        schema:hasPart ,
                                            <http://www.isibang.ac.in/ns/mod/1.2/syntax> ;
                    pav:derivedFrom         <http://www.isibang.ac.in/ns/mod/1.2> ;
                    pav:importedOn          "2017-07-06"^^xsd:dateTime ;
                    
            #OPTIONAL STATEMENTS
                    prov:wasInfluencedBy    "FAIR principle: I1" .



### http://purl.org/dc/terms/hasFormat
dcterms:hasFormat   rdf:type                rdf:Property ;
                    rdfs:subPropertyOf      dc:relation , dcterms:relatio ;
                    rdfs:label              "has format"@en ,
                                            " pour format"@fr ;
                    dcterms:description     "DCTERMS: A related resource that is substantially the same as the pre-existing described resource, but in another format."@en ;
                    rdfs:isDefinedBy        <http://purl.org/dc/terms/> ;
                    dcterms:issued          "2000-07-11"^^xsd:date ;
                    dcterms:relation        schema:hasPart ,
                                            <http://www.isibang.ac.in/ns/mod/1.2/syntax> ;
                    pav:derivedFrom         <http://www.isibang.ac.in/ns/mod/1.2> ;
                    pav:importedOn          "2017-07-06"^^xsd:dateTime ;
                    
            #OPTIONAL STATEMENTS
                    prov:wasInfluencedBy    "FAIR principle: I1" .



### http://purl.org/dc/terms/relation
dcterms:relation    rdf:type                rdf:Property ;
                    rdfs:subPropertyOf      dc:relation ;
                    rdfs:label              "relation"@en ,
                                            "relation"@fr ;
                    dcterms:description     "DCTERMS: A related resource."@en ;
                    rdfs:isDefinedBy        <http://purl.org/dc/terms/> ;
                    dcterms:issued          "2008-01-14"^^xsd:date ;
                    pav:derivedFrom         <http://www.isibang.ac.in/ns/mod/1.0> ;
                    pav:importedOn          "2015-08-05"^^xsd:dateTime ;
                    
            #OPTIONAL STATEMENTS
                    prov:wasInfluencedBy    "FAIR principle: I2" .



### https://w3id.org/mod#semanticArtefactRelation
mod:semanticArtefactRelation 
                    rdf:type                owl:ObjectProperty ;
                    rdfs:subPropertyOf      dcterms:relation ;
                    rdfs:label              "generally related to"@en ,
                                            "relation générale avec"@fr ;
                    rdfs:domain             mod:SemanticArtefact ;
                    rdfs:range              mod:SemanticArtefact ;
                    dcterms:description     "MOD: A general property for semantic artefact relations. DOOR: An ontology is related to another if one of the DOOR relations is satisfied."@en ;
                    rdfs:isDefinedBy        <https://w3id.org/mod/2.0> ;
                    dcterms:issued          "2021-12-06"^^xsd:date ;
                    dcterms:relation        door:ontologyRelatedTo ; 
                    pav:derivedFrom         <http://www.isibang.ac.in/ns/mod/2.0> ;
                    pav:importedOn          "2021-12-06"^^xsd:dateTime ;

            #OPTIONAL STATEMENTS
                    prov:wasInfluencedBy    "FAIR principle: I2" .



### https://w3id.org/mod#reliesOn
mod:reliesOn        rdf:type                owl:ObjectProperty ;
                    rdfs:subPropertyOf      mod:semanticArtefactRelation ;
                    owl:inverseOf           mod:usedBy ;
                    rdfs:label              "relies on or reuses"@en ,
                                            "se repose sur ou réutilise"@fr ;
                    dcterms:description     "MOD: A general property for different kind of case when a semantic resource relies or reuses another one. VOAF: Indicates that the subject vocabulary uses or extends some class or property of the object vocabulary. VOID: A vocabulary that is used in the dataset."@en ;
                    rdfs:isDefinedBy        <http://purl.org/vocommons/voaf> ;
                    dcterms:issued          "2013-05-24"^^xsd:date ;
                    dcterms:relation        voaf:reliesOn ,
                                            void:vocabulary  ;
                    pav:derivedFrom         <http://www.isibang.ac.in/ns/mod/2.0> ;
                    pav:importedOn          "2021-12-06"^^xsd:dateTime ;
            
            #OPTIONAL STATEMENTS
                    skos:historyNote        "This property had been originally defined by VOAF metadata vocabulary. Now, it has been adopted and redefined in the MOD namespace."@en ;
                    prov:wasInfluencedBy    "FAIR principle: I2" .



## https://w3id.org/mod#usedBy
mod:usedBy          rdf:type                owl:ObjectProperty ;
                    rdfs:subPropertyOf      mod:semanticArtefactRelation ;
                    owl:inverseOf           mod:reliesOn ;
                    rdfs:label              "used by"@en ,
                                            "utilisé par"@fr ;
                    dcterms:description     "VOAF: Indicates that the subject vocabulary is used by the object vocabulary. NKOS: Agent using the described KOS."@en ;
                    rdfs:isDefinedBy        <http://purl.org/vocommons/voaf> ;
                    dcterms:issued          "2013-05-23"^^xsd:date ;
                    dcterms:relation        voaf:usedBy ,
                                            nkos:usedBy ;
                    pav:derivedFrom         <http://www.isibang.ac.in/ns/mod/1.4> ;
                    pav:importedOn          "2018-08-02"^^xsd:dateTime ;
            
            #OPTIONAL STATEMENTS
                    skos:historyNote        "This property had been originally defined by VOAF metadata vocabulary. Now, it has been adopted and redefined in the MOD namespace."@en ;
                    prov:wasInfluencedBy    "FAIR principle: I2" .



### https://w3id.org/mod#specializes
mod:specializes     rdf:type                owl:ObjectProperty ;
                    rdfs:subPropertyOf      mod:semanticArtefactRelation ;
                    owl:inverseOf           mod:generalizes ;
                    rdfs:label              "specializes"@en ,
                                            "spécialise"@fr ;
                    dcterms:description     "DOOR: Evolution which involves a only at the syntactic level. PROV: An entity that is a specialization of another shares all aspects of the latter, and additionally presents more specific aspects of the same thing as the latter. VOAF:Indicates that the subject vocabulary defines some subclasses or subproperties of the object vocabulary, or local restrictions on those."@en ;
                    rdfs:isDefinedBy        <http://purl.org/vocommons/voaf> ;
                    dcterms:issued          "2013-05-23"^^xsd:date ;
                    dcterms:relation        door:explanationEvolution ,
                                            voaf:specializes ,
                                            prov:specializationOf ;
                    pav:derivedFrom         <http://www.isibang.ac.in/ns/mod/1.2> ;
                    pav:importedOn          "2017-07-06"^^xsd:dateTime ;
            
            #OPTIONAL STATEMENTS
                    skos:historyNote        "This property had been originally defined by VOAF metadata vocabulary. Now, it has been adopted and redefined in the MOD namespace."@en ;
                    prov:wasInfluencedBy    "FAIR principle: I2" .
            


### https://w3id.org/mod#generalizes
mod:generalizes     rdf:type                owl:ObjectProperty ;
                    rdfs:subPropertyOf      mod:semanticArtefactRelation ;
                    owl:inverseOf           mod:specializes ;
                    rdfs:label              "generalizes"@en ,
                                            "généralise"@fr ;
                    dcterms:description     "VOAF: Indicates that the subject vocabulary generalizes by some superclasses or superproperties the object vocabulary. PROV: Inverse property of specializationOf."@en ;
                    rdfs:isDefinedBy        <http://purl.org/vocommons/voaf> ;
                    dcterms:issued          "2013-05-23"^^xsd:date ;
                    dcterms:relation        voaf:generalizes ,
                                            prov:generalizationOf ;
                    pav:derivedFrom         <http://www.isibang.ac.in/ns/mod/1.4> ;
                    pav:importedOn          "2018-08-02"^^xsd:dateTime ;
            
            #OPTIONAL STATEMENTS
                    skos:historyNote        "This property had been originally defined by VOAF metadata vocabulary. Now, it has been adopted and redefined in the MOD namespace."@en ;
                    prov:wasInfluencedBy    "FAIR principle: I2" .
            


## http://schema.org/workTranslation
schema:workTranslation
                    rdf:type                rdf:Property ;
                    rdfs:label              "work translation"@en ,
                                            "a pour traduction"@fr ;
                    dcterms:description     "MOD: A pointer to the translated ontology(ies) for an existing ontology. SCHEMA: A work that is a translation of the content of this work. ADMS: Links Assets that are translations of each other."@en ;
                    rdfs:isDefinedBy        <http://schema.org/> ;
                    dcterms:issued          "2012-04-21"^^xsd:date ;
                    dcterms:relation        adms:translation ,
                                            <http://www.isibang.ac.in/ns/mod/1.0/translation> ;
                    pav:derivedFrom         <http://www.isibang.ac.in/ns/mod/1.0> ;
                    pav:importedOn          "2015-08-05"^^xsd:dateTime ;
            
            #OTHER ORIGINAL STATEMENTS IF ANY 
                    schema:domainIncludes   schema:CreativeWork ;
                    schema:rangeIncludes    schema:CreativeWork ;
                    schema:inverseOf        schema:translationOfWork ;
                    schema:isPartOf         <https://bib.schema.org> .
    


## http://schema.org/translationOfWork
schema:translationOfWork
                    rdf:type                rdf:Property ;
                    rdfs:label              "translation of"@en ,
                                            "traduction de"@fr ;
                    dcterms:description     "SCHEMA: The work that this work has been translated from. ADMS: Links Assets that are translations of each other."@en ;
                    rdfs:isDefinedBy        <http://schema.org/> ;
                    dcterms:issued          "2012-04-21"^^xsd:date ;
                    dcterms:relation        adms:translation  ;
                    pav:derivedFrom         <http://www.isibang.ac.in/ns/mod/1.4> ;
                    pav:importedOn          "2018-08-02"^^xsd:dateTime ;

            #OTHER ORIGINAL STATEMENTS IF ANY 
                    schema:domainIncludes   schema:CreativeWork ;
                    schema:rangeIncludes    schema:CreativeWork ;
                    schema:inverseOf        schema:workTranslation ;
                    schema:isPartOf         <https://bib.schema.org> .
    


###  https://w3id.org/mod#comesFromTheSameDomain
mod:comesFromTheSameDomain
                    rdf:type                owl:ObjectProperty , owl:SymmetricProperty , owl:TransitiveProperty ;
                    rdfs:subPropertyOf      mod:semanticArtefactRelation ;
                    rdfs:label              "comes from the same domain"@en ,
                                            "vient du même domaine"@fr ;
                    dcterms:description     "DOOR: If the two ontologies come from the same domain (without any other details)."@en ;
                    rdfs:isDefinedBy        <http://kannel.open.ac.uk/ontology> ;
                    dcterms:issued          "2009-10-06"^^xsd:date ;
                    dcterms:relation        <http://kannel.open.ac.uk/ontology/comesFromTheSameDomain> ;
                    pav:derivedFrom         <http://www.isibang.ac.in/ns/mod/1.4> ;
                    pav:importedOn          "2018-08-02"^^xsd:dateTime ;
            
            #OPTIONAL STATEMENTS
                    skos:historyNote        "This property had been originally defined by DOOR metadata vocabulary. Now, it has been adopted and redefined in the MOD namespace."@en ;
                    prov:wasInfluencedBy    "MIRO guidelines: B.2" ,
                                            "FAIR principle: I2" .
             


### https://w3id.org/mod#similar
mod:similar     rdf:type                    owl:ObjectProperty ;
                    rdfs:subPropertyOf      mod:semanticArtefactRelation ;
                    rdfs:label              "similar to"@en ,
                                            "similaire à"@fr ;
                    dcterms:description     "VOAF: Used to assert that two vocabularies are similar in scope and objectives, independently of the fact that they otherwise refer to each other. DOOR: Represents the meaning of 'how an ontology overlap/cover parts of the same area of interest of another ontology.'"@en ;
                    rdfs:isDefinedBy        <http://purl.org/vocommons/voaf> ;
                    dcterms:issued          "2013-05-23"^^xsd:date ;
                    dcterms:relation        <http://kannel.open.ac.uk/ontology/similarTo> ,
                                            voaf:similar ;
                    pav:derivedFrom         <http://www.isibang.ac.in/ns/mod/1.4> ;
                    pav:importedOn          "2018-08-02"^^xsd:dateTime ;
            
            #OPTIONAL STATEMENTS
                    skos:historyNote        "This property had been originally defined by VOAF metadata vocabulary. Now, it has been adopted and redefined in the MOD namespace."@en ;
                    prov:wasInfluencedBy    "MIRO guidelines: B.2",
                                            "FAIR principle: I2" .



## https://w3id.org/mod#hasEquivalencesWith
mod:hasEquivalencesWith
                    rdf:type                owl:ObjectProperty ;
                    rdfs:subPropertyOf      mod:reliesOn ;
                    rdfs:label              "has equivalences with"@en ,
                                            "a des équivalences avec"@fr ;
                    dcterms:description     "VOAF: Indicates that the subject vocabulary declares some equivalent classes or properties with the object vocabulary. DOOR: Links two ontologies if there exists an alignment which covers a substantial part of the vocabulary (i.e., a proportion greater than a threshold). NKOS: A related resource with which the described resource is aligned."@en ;
                    rdfs:isDefinedBy        <http://purl.org/vocommons/voaf> ;
                    dcterms:issued          "2013-05-23"^^xsd:date ;
                    dcterms:relation        door:isAlignedTo ,
                                            voaf:hasEquivalencesWith ,
                                            nkos:alignedWith ;
                    pav:derivedFrom         <http://www.isibang.ac.in/ns/mod/1.4> ;
                    pav:importedOn          "2018-08-02"^^xsd:dateTime ;
            
            #OPTIONAL STATEMENTS
                    skos:historyNote        "This property had been originally defined by VOAF metadata vocabulary. Now, it has been adopted and redefined in the MOD namespace."@en ;
                    prov:wasInfluencedBy    "MIRO guidelines: E.4",
                                            "FAIR principle: I2" .



###  https://w3id.org/mod#hasDisparateModelling
mod:hasDisparateModelling
                    rdf:type                owl:ObjectProperty ;
                    rdfs:subPropertyOf      mod:semanticArtefactRelation ;
                    rdfs:label              "disparate modelling with"@en ,
                                            "différences de modélisation avec"@fr ;
                    dcterms:description     "DOOR: Disagreements related  to  the  conceptualization  of  the  ontologies. Two ontologies are considered to have disparate modeling if they represent corresponding entities in different ways, e.g.  as an instance in one case and a class in the other."@en ;
                    rdfs:isDefinedBy        <http://kannel.open.ac.uk/ontology> ;
                    dcterms:issued          "2009-10-06"^^xsd:date ;
                    dcterms:relation        <http://kannel.open.ac.uk/ontology/hasDisparateModelling> ;
                    pav:derivedFrom         <http://www.isibang.ac.in/ns/mod/1.4> ;
                    pav:importedOn          "2018-08-02"^^xsd:dateTime ;
            
            #OPTIONAL STATEMENTS
                    skos:historyNote        "This property had been originally defined by DOOR metadata vocabulary. Now, it has been adopted and redefined in the MOD namespace."@en ;
                    prov:wasInfluencedBy    "MIRO guidelines: B.2" ,
                                            "FAIR principle: I2" ;
            #OTHER ORIGINAL STATEMENTS IF ANY 
                    rdfs:subPropertyOf      door:disagreesWith .



## https://w3id.org/mod#hasDisjunctionsWith
mod:hasDisjunctionsWith
                    rdf:type                owl:ObjectProperty ;
                    rdfs:subPropertyOf      mod:semanticArtefactRelation ;
                    rdfs:label              "has disjunctions with"@en ,
                                            "a des disjopnctions avec"@fr ;
                    dcterms:description     "VOAF: Indicates that the subject vocabulary declares some disjunct classes with the object vocabulary."@en ;
                    rdfs:isDefinedBy        <http://purl.org/vocommons/voaf> ;
                    dcterms:issued          "2013-05-23"^^xsd:date ;
                    dcterms:relation        voaf:hasDisjunctionsWith ;
                    pav:derivedFrom         <http://www.isibang.ac.in/ns/mod/1.4> ;
                    pav:importedOn          "2018-08-02"^^xsd:dateTime ;
            
            #OPTIONAL STATEMENTS
                    skos:historyNote        "This property had been originally defined by VOAF metadata vocabulary. Now, it has been adopted and redefined in the MOD namespace."@en ;
                    prov:wasInfluencedBy    "MIRO guidelines: E.4",
                                            "FAIR principle: I2" .



##########################################
########## Content properties ##########
##########################################

### http://xmlns.com/foaf/0.1/
foaf:primaryTopic   rdf:type                owl:ObjectProperty , owl:FunctionalProperty ;
                    rdfs:label              "primary topic"@en ,
                                            "sujet principal"@fr ;
                    rdfs:domain             foaf:Document ;
                    rdfs:range              owl:Thing ;
                    dcterms:description     ""@en ;
                    rdfs:isDefinedBy        <http://xmlns.com/foaf/0.1/> ;
                    dcterms:issued          "2014-01-14"^^xsd:date ;
                    dcterms:relation        omv:keyClasses ,
                                            schema:mainEntity ;
                    pav:derivedFrom         <http://www.isibang.ac.in/ns/mod/1.2> ;
                    pav:importedOn          "2017-07-06"^^xsd:dateTime ;
            
            #OPTIONAL STATEMENTS
                    prov:wasInfluencedBy    "FAIR principle: F2" ;
        
            #OTHER ORIGINAL STATEMENTS IF ANY 
                    owl:inverseOf           foaf:isPrimaryTopicOf .



### http://rdfs.org/ns/void#rootResource
void:rootResource   rdf:type                rdf:Property ;
                    rdfs:label              "root resource"@en ,
                                            "ressource racine"@fr ;
                    rdfs:domain             void:Dataset ;
                    rdfs:range              rdfs:Resource ;
                    dcterms:description     "VOID: A top concept or entry point for a void:Dataset that is structured in a tree-like fashion. All resources in a dataset can be reached by following links from its root resources in a small number of steps. MOD: This property is to provide the root class(es) of an ontology. This is automatically populated by taking the direct subclasses of owl:Thing. If the ontology is also defined as a unique skos:ConceptScheme, then this property should become equivalent of skos:hasTopConcept. SKOS: The property skos:hasTopConcept is, by convention, used to link a concept scheme to the SKOS concept(s) which are topmost in the hierarchical relations for that scheme."@en ;
                    rdfs:isDefinedBy        <http://vocab.deri.ie/void> ;
                    dcterms:issued          "2010-01-26"^^xsd:date ;
                    dcterms:relation        skos:hasTopConcept ,
                                            <http://www.isibang.ac.in/ns/mod/1.0/rootClasses> ;
                    pav:derivedFrom         <http://www.isibang.ac.in/ns/mod/1.0> ;
                    pav:importedOn          "2015-08-05"^^xsd:dateTime ;
                    
            #OPTIONAL STATEMENTS
                    prov:wasInfluencedBy    "FAIR principle: F2" .


###  https://w3id.org/mod#browsingUI
mod:browsingUI      rdf:type                owl:DatatypeProperty ;
                    rdfs:label              "browsing user interface"@en ,
                                            "interface de navigation"@fr ;
                    rdfs:domain             mod:SemanticArtefact ;
                    rdfs:range              xsd:anyURI ;
                    dcterms:description     "MOD: The user interface (URL) where the ontology may be browsed or searched."@en ;
                    rdfs:isDefinedBy        <https://w3id.org/mod> ;
                    dcterms:issued          "2017-07-06"^^xsd:date ;
                    pav:derivedFrom         <http://www.isibang.ac.in/ns/mod/1.2> ;
                    pav:importedOn          "2017-07-06"^^xsd:dateTime ;
            
            #OPTIONAL STATEMENTS
                    prov:wasInfluencedBy    "FAIR principle: F2" .


### http://www.w3.org/ns/sparql-service-description#endpoint
sd:endpoint         rdf:type                rdf:Property , owl:InverseFunctionalProperty ; 
                    rdfs:label              "SPARQL endpoint"@en ,
                                           "point de requêtage SPARQL"@fr ;
                    rdfs:domain             sd:Service ;
                    dcterms:description     "SD: Relates an instance of sd:Service to a SPARQL endpoint that implements the SPARQL Protocol service for the service. The object of the sd:endpoint property is an IRI. VOID: A SPARQL protocol endpoint that allows SPARQL query access to a void:Dataset."@en ;
                    rdfs:isDefinedBy        <ttp://www.w3.org/ns/sparql-service-description> ;
                    dcterms:issued          "2013-03-21"^^xsd:date ;
                    dcterms:relation        void:sparqlEndpoint ;
                    pav:derivedFrom         <http://www.isibang.ac.in/ns/mod/1.2> ;
                    pav:importedOn          "2017-07-06"^^xsd:dateTime ;
                    
            #OPTIONAL STATEMENTS
                    prov:wasInfluencedBy    "FAIR principle: A1" .
            


### https://w3id.org/mod#metadataVoc
mod:metadataVoc     rdf:type                owl:ObjectProperty ;
                    rdfs:subPropertyOf      mod:reliesOn ;
                    rdfs:label              "metadata vocabulary used"@en ,
                                            "vocabulaires de métadonnées utilisés"@fr;
                    dcterms:description     "VOAF: Indicates that the subject vocabulary uses the object vocabulary in metadata at vocabulary or element level. SCHEMA: Indicates (by URL or string) a particular version of a schema used in some CreativeWork. ADMS: A schema according to which the Asset Repository can provide data about its content, e.g. ADMS. MOD: A vocabulary(ies) that is used and/or referred to create the current ontology."@en ;    
                    rdfs:isDefinedBy        <http://purl.org/vocommons/voaf> ;
                    dcterms:issued          "2013-05-23"^^xsd:date ;
                    dcterms:relation        voaf:metadataVoc ,
                                            schema:schemaVersion ,
                                            adms:supportedSchema ,
                                            <http://www.isibang.ac.in/ns/mod/1.0/vocabularyUsed> ;
                    pav:derivedFrom         <http://www.isibang.ac.in/ns/mod/1.0> ;
                    pav:importedOn          "2015-08-05"^^xsd:dateTime ;
                    
            #OPTIONAL STATEMENTS
                    skos:historyNote        "This property had been originally defined by VOAF metadata vocabulary. Now, it has been adopted and redefined in the MOD namespace."@en ;
                    prov:wasInfluencedBy    "MIRO guidelines: E.4,E9" ,
                                            "FAIR principle: I2" .



### https://w3id.org/mod#sampleQueries
mod:sampleQueries   rdf:type                owl:DatatypeProperty ;
                    rdfs:label              "sample queries"@en ,
                                            "exemples de requêtes"@fr;
                    rdfs:domain             mod:SemanticArtefactDistribution ;
                    rdfs:range              xsd:string ;
                    dcterms:description     "MOD: A set of queries (may be SPARQL, DL Queries) that are provided along with an ontology."@en ;    
                    rdfs:isDefinedBy        <https://w3id.org/mod> ;
                    dcterms:issued          "2015-08-05"^^xsd:date ;
                    pav:derivedFrom         <http://www.isibang.ac.in/ns/mod/1.0> ;
                    pav:importedOn          "2015-08-05"^^xsd:dateTime ;
                    
            #OPTIONAL STATEMENTS
                    prov:wasInfluencedBy    "FAIR principle: F2" .



### http://rdfs.org/ns/void#propertyPartition
void:propertyPartition
                    rdf:type                rdf:Property ;
                    rdfs:label              "property partition"@en ,
                                            "partition des propriétés"@fr ;
                    rdfs:domain             void:Dataset ;
                    rdfs:range              void:Dataset ;
                    dcterms:description     "VOID: A subset of a void:Dataset that contains only the triples of a certain rdf:Property."@en ;
                    rdfs:isDefinedBy        <http://vocab.deri.ie/void> ;
                    dcterms:issued          "2010-01-26"^^xsd:date ;
                    pav:derivedFrom         <http://www.isibang.ac.in/ns/mod/1.4> ;
                    pav:importedOn          "2018-08-02"^^xsd:dateTime ;
                    
            #OPTIONAL STATEMENTS
                    prov:wasInfluencedBy    "FAIR principle: F2" ;

            #OTHER ORIGINAL STATEMENTS IF ANY 
                    rdfs:subPropertyOf       void:subset .



### http://rdfs.org/ns/void#classPartition
void:classPartition
                    rdf:type                rdf:Property ;
                    rdfs:label              "class partition"@en ,
                                            "partition des classes"@fr ;
                    rdfs:domain             void:Dataset ;
                    rdfs:range              void:Dataset ;
                    dcterms:description     "VOID: A subset of a void:Dataset that contains only the entities of a certain rdfs:Class."@en ;
                    rdfs:isDefinedBy        <http://vocab.deri.ie/void> ;
                    dcterms:issued          "2010-01-26"^^xsd:date ;
                    pav:derivedFrom         <http://www.isibang.ac.in/ns/mod/1.4> ;
                    pav:importedOn          "2018-08-02"^^xsd:dateTime ;
                    
            #OPTIONAL STATEMENTS
                    prov:wasInfluencedBy    "FAIR principle: F2" ;

            #OTHER ORIGINAL STATEMENTS IF ANY 
                    rdfs:subPropertyOf       void:subset .



### http://www.w3.org/ns/dcat#downloadURL
dcat:downloadURL    rdf:type                rdf:Property , owl:ObjectProperty ;
                    rdfs:label              "download URL"@en ,
                                            "URL de téléchargement"@fr ;
                    rdfs:domain             dcat:Distribution ;
                    rdfs:range              rdfs:Resource ;
                    dcterms:description     "DCAT: The URL of the downloadable file in a given format. E.g. CSV file or RDF file. The format is indicated by the distribution's dct:format and/or dcat:mediaType. VOID: An RDF dump, partial or complete, of a void:Dataset. DOAP: Mirror of software download web page. SCHEMA: A downloadable form of this dataset, at a specific location, in a specific format."@en ; 
                    rdfs:isDefinedBy        <http://www.w3.org/TR/vocab-dcat/> ;
                    dcterms:issued          "2014-01-16"^^xsd:date ;
                    dcterms:relation        void:dataDump ,
                                            doap:download-mirror ,
                                            schema:distribution ;
                   pav:derivedFrom          <http://www.isibang.ac.in/ns/mod/1.4> ;
                    pav:importedOn          "2018-08-02"^^xsd:dateTime ;
            
            #OPTIONAL STATEMENTS
                    prov:wasInfluencedBy    "FAIR principle: F2" ;

            #OTHER ORIGINAL STATEMENTS IF ANY 
                    skos:scopeNote "dcat:downloadURL SHOULD be used for the address at which this distribution is available directly, typically through a HTTP Get request."@en .
  
        

### http://rdfs.org/ns/void#openSearchDescription
void:openSearchDescription
                    rdf:type                rdf:Property ;
                    rdfs:label              "free-text search endpoint"@en ,
                                            "service de requêtage en texte libre"@fr ;
                    rdfs:domain             void:Dataset ;
                    rdfs:range              foaf:Document ;
                    dcterms:description     "VOID: An OpenSearch description document for a free-text search service over a void:Dataset. DOAP: The URI of a web service endpoint where software as a service may be accessed."@en ;
                    rdfs:isDefinedBy        <http://vocab.deri.ie/void> ;
                    dcterms:issued          "2010-01-26"^^xsd:date ;
                    pav:derivedFrom         <http://www.isibang.ac.in/ns/mod/1.4> ;
                    pav:importedOn          "2018-08-02"^^xsd:dateTime ;
                    
            #OPTIONAL STATEMENTS
                    prov:wasInfluencedBy    "FAIR principle: F2" .



### http://rdfs.org/ns/void#uriLookupEndpoint
void:uriLookupEndpoint
                    rdf:type                rdf:Property ;
                    rdfs:label              "URI lookup endpoint"@en ,
                                            "service de requêtage des URI"@fr ;
                    rdfs:domain             void:Dataset ;
                    rdfs:range              xsd:anyURI ;
                    dcterms:description     "VOID: A protocol endpoint for simple URI lookups for a void:Dataset."@en ;
                    rdfs:isDefinedBy        <http://vocab.deri.ie/void> ;
                    dcterms:issued          "2010-01-26"^^xsd:date ;
                    pav:derivedFrom         <http://www.isibang.ac.in/ns/mod/1.4> ;
                    pav:importedOn          "2018-08-02"^^xsd:dateTime ;
                    
            #OPTIONAL STATEMENTS
                    prov:wasInfluencedBy    "FAIR principle: F2" .



##########################################
########## Community properties ##########
##########################################

###  https://w3id.org/mod#knownUsage
mod:knownUsage      rdf:type                owl:DatatypeProperty ;
                    rdfs:label              "known usage"@en ,
                                            "usage connu"@fr ;
                    rdfs:domain             mod:SemanticArtefact ;
                    rdfs:range              xsd:string ;
                    dcterms:description     "OMV: The applications where the ontology is being used."@en ;
                    rdfs:isDefinedBy        <http://omv.ontoware.org/2005/05/ontology> ;
                    dcterms:issued          "2009-12-24"^^xsd:date ;
                    dcterms:relation        omv:knownUsage ;
                    pav:derivedFrom         <http://www.isibang.ac.in/ns/mod/1.2> ;
                    pav:importedOn          "2017-07-06"^^xsd:dateTime ;
            
            #OPTIONAL STATEMENTS
                    skos:historyNote        "This property has been adopted from OMV Ontology Metadata Vocabulary and redefined in the MOD namespace."@en ;
                    prov:wasInfluencedBy    "MIRO guidelines: B.3" ,
                                            "FAIR principle: F2" .
    


###  https://w3id.org/mod#endorsedBy
mod:endorsedBy      rdf:type                owl:ObjectProperty ;
                    rdfs:label              "endorsed by"@en ,
                                            "approuvé par"@fr ;
                    rdfs:domain             mod:SemanticArtefact ;
                    rdfs:range              dcterms:Agent ;
                    dcterms:description     "MOD: An ontology endorsed by an agent. OMV: The parties that have expressed support or approval to this ontology."@en ;
                    rdfs:isDefinedBy        <http://omv.ontoware.org/2005/05/ontology> ;
                    dcterms:issued          "2009-12-24"^^xsd:date ;
                    dcterms:relation        omv:endorsedBy ;
                    pav:derivedFrom         <http://www.isibang.ac.in/ns/mod/1.2> ;
                    pav:importedOn          "2017-07-06"^^xsd:dateTime ;
            
            #OPTIONAL STATEMENTS
                    skos:historyNote        "This property has been adopted from OMV Ontology Metadata Vocabulary and redefined in the MOD namespace."@en ;
                    prov:wasInfluencedBy    "MIRO guidelines: G.4" ,
                                            "FAIR principle: I3" .
    


### https://w3id.org/mod#usedInProject
mod:usedInProject   rdf:type                owl:ObjectProperty ;
                    rdfs:label              "used in project"@en ,
                                            "utilisé dans le projet"@fr ;
                    rdfs:domain             mod:SemanticArtefact ;
                    rdfs:range              foaf:Project ;
                    dcterms:description     "MOD: An ontology that is used in a project."@en ; 
                    rdfs:isDefinedBy        <https://w3id.org/mod> ;
                    dcterms:issued          "2015-08-05"^^xsd:date ;
                    dcterms:relation        <http://www.isibang.ac.in/ns/mod/1.0/ontologyInUse> ;
                    pav:derivedFrom         <http://www.isibang.ac.in/ns/mod/1.0> ;
                    pav:importedOn          "2015-08-05"^^xsd:dateTime ;
                    
            #OPTIONAL STATEMENTS
                    prov:wasInfluencedBy    "MIRO guidelines: B.3,G.5" ,
                                            "FAIR principle: I3" .



### http://purl.org/dc/terms/audience
dcterms:audience    rdf:type                rdf:Property ;
                    rdfs:subPropertyOf      dc:audience ;
                    rdfs:label              "target audience"@en ,
                                            "audience cible"@fr ;
                    dcterms:description     "DCTERMS: a class of entity for whom the resource is intended or useful (public visé ou recommandé pour la ressource). DOAP: Description of target user base. SCHEMA: An intended audience, i.e. a group for whom something was created."@en ;
                    rdfs:isDefinedBy        <http://purl.org/dc/terms/> ;
                    dcterms:issued          "2001-05-21"^^xsd:date ; 
                    dcterms:relation        doap:audience ,
                                            schema:audience ;
                    pav:derivedFrom         <http://www.isibang.ac.in/ns/mod/1.2> ;
                    pav:importedOn          "2017-07-06"^^xsd:dateTime ;
                    
            #OPTIONAL STATEMENTS
                    prov:wasInfluencedBy    "MIRO guidelines: B.3" ,
                                            "FAIR principle: F2" ;
            
            #OTHER ORIGINAL STATEMENTS IF ANY 
                    <http://purl.org/dc/dcam/rangeIncludes>      dcterms:AgentClass .


### http://xmlns.com/foaf/0.1/fundedBy
foaf:fundedBy       rdf:type                rdf:Property , owl:ObjectProperty ;
                    rdfs:label              "funded or sponsored by"@en ,
                                            "financé ou sponsorisé par"@fr ;
                    rdfs:domain             owl:Thing ;
                    rdfs:range              owl:Thing ;
                    dcterms:description     "MOD: An ontology that is sponsored by and developed under a project. FOAF: An organization funding a project or person. SCHEMA: The Organization on whose behalf the creator was working."@en ;
                    rdfs:isDefinedBy        <http://xmlns.com/foaf/0.1/> ;
                    dcterms:issued          "2014-01-14"^^xsd:date ;
                    dcterms:relation        schema:sourceOrganization ,
                                            <http://www.isibang.ac.in/ns/mod/1.0/sponsoredBy> ;
                    pav:derivedFrom          <http://www.isibang.ac.in/ns/mod/1.0> ;
                    pav:importedOn          "2015-08-05"^^xsd:dateTime ;
                    
            #OPTIONAL STATEMENTS
                    prov:wasInfluencedBy    "FAIR principle: R1.2" .
     



### http://usefulinc.com/ns/doap/repository
doap:repository     rdf:type                rdf:Property ;
                    rdfs:label              "repository"@en ,
                                            "entrepôt"@fr ;
                    rdfs:domain             doap:Project ;
                    rdfs:range              doap:Repository ;
                    dcterms:description     "DOAP: Source code repository."@en ;
                    rdfs:isDefinedBy        <http://usefulinc.com/ns/doap#> ;
                    dcterms:issued          "2004"^^xsd:date ;
                    pav:derivedFrom          <http://www.isibang.ac.in/ns/mod/1.2> ;
                    pav:importedOn          "2017-07-06"^^xsd:dateTime ;
                    
            #OPTIONAL STATEMENTS
                    prov:wasInfluencedBy    "MIRO guidelines: A.5" , 
                                            "FAIR principle: R1.2" .
            


### http://usefulinc.com/ns/doap/bug-database
doap:bug-database    rdf:type                rdf:Property ;
                    rdfs:label              "bug database"@en ,
                                            "repertoire de bogues"@fr ;
                    rdfs:domain             doap:Project ;
                    dcterms:description     "DOAP: Bug tracker for a project."@en ;
                    rdfs:isDefinedBy        <http://usefulinc.com/ns/doap#> ;
                    dcterms:issued          "2004"^^xsd:date ;
                    pav:derivedFrom          <http://www.isibang.ac.in/ns/mod/1.2> ;
                    pav:importedOn          "2017-07-06"^^xsd:dateTime ;
                    
            #OPTIONAL STATEMENTS
                    prov:wasInfluencedBy    "MIRO guidelines: C.3" , 
                                            "FAIR principle: F2" .

            

### http://usefulinc.com/ns/doap/mailing-list
doap:mailing-list   rdf:type                rdf:Property ;
                    rdfs:label              "mailing list"@en ,
                                            "liste de diffusion"@fr ;
                    rdfs:domain             doap:Project ;
                    dcterms:description     "DOAP: Mailing list home page or email address."@en ;
                    rdfs:isDefinedBy        <http://usefulinc.com/ns/doap#> ;
                    dcterms:issued          "2004"^^xsd:date ;
                    pav:derivedFrom          <http://www.isibang.ac.in/ns/mod/1.2> ;
                    pav:importedOn          "2017-07-06"^^xsd:dateTime ;
                    
            #OPTIONAL STATEMENTS
                    prov:wasInfluencedBy    "MIRO guidelines: C.3" , 
                                            "FAIR principle: F2" .
            


### https://w3id.org/mod#hasEvaluation
mod:hasEvaluation   rdf:type                owl:ObjectProperty ;
                    rdfs:label              "evaluation"@en ,
                                            "évaluation"@fr ;
                    rdfs:domain             mod:SemanticArtefact ;
                    rdfs:range              mod:Evaluation ;
                    dcterms:description     "MOD: This property makes a relationship between an ontology and its evaluation result."@en ; 
                    rdfs:isDefinedBy        <https://w3id.org/mod> ;
                    dcterms:issued          "2015-08-05"^^xsd:date ;
                    dcterms:relation        schema:review ;
                    pav:derivedFrom         <http://www.isibang.ac.in/ns/mod/1.0> ;
                    pav:importedOn          "2015-08-05"^^xsd:dateTime ;
                    
            #OPTIONAL STATEMENTS
                    prov:wasInfluencedBy    "MIRO guidelines: G.2" ,
                                            "FAIR principle: F2" .


              
### http://schema.org/comment
schema:comment      rdf:type                rdf:Property ;
                    rdfs:label              "user notes or reviews"@en ,
                                            "commentaires ou avis d'utilisateurs"@fr ;
                    dcterms:description     "SCHEMA: Comments, typically from users."@en ;
                    rdfs:isDefinedBy        <http://schema.org/> ;
                    dcterms:issued          "2012-04-21"^^xsd:date ;
                    pav:derivedFrom         <http://www.isibang.ac.in/ns/mod/1.4> ;
                    pav:importedOn          "2018-08-02"^^xsd:dateTime ;
                    
            #OPTIONAL STATEMENTS
                    prov:wasInfluencedBy    "FAIR principle: F4, A1.1, A1.2" ;
            
            #OTHER ORIGINAL STATEMENTS IF ANY 
                    schema:domainIncludes   schema:CreativeWork ;
                    schema:rangeIncludes    schema:Comment .
    


### https://w3id.org/mod#analytics
mod:analytics       rdf:type                owl:ObjectProperty ;
                    rdfs:label              "analytics"@en ,
                                            "analytique"@fr ;
                    rdfs:domain             mod:SemanticArtefact ;
                    rdfs:range              mod:Analytics ;
                    dcterms:description     "MOD: This property shall be used to store any analytics for an ontology. E.g., number of visits an ontology received in a portal, number of downloads, etc."@en ; 
                    rdfs:isDefinedBy        <https://w3id.org/mod> ;
                    dcterms:issued          "2018-08-02"^^xsd:date ;
                    pav:derivedFrom         <http://www.isibang.ac.in/ns/mod/1.4> ;
                    pav:importedOn          "2018-08-02"^^xsd:dateTime ;
                    
            #OPTIONAL STATEMENTS
                    prov:wasInfluencedBy    "MIRO guidelines: G.2" ,
                                            "FAIR principle: F2" .



##########################################
########## Date properties ##########
##########################################


### http://purl.org/dc/terms/created
dcterms:created     rdf:type                rdf:Property ;
                    rdfs:subPropertyOf      dc:date , dcterms:date ;
                    rdfs:label              "creation date"@en ,
                                            "date de création"@fr ;
                    rdfs:range              rdfs:Literal ; 
                    dcterms:description     "DCTERMS:date : A point or period of time associated with an event in the lifecycle of the resource. DCTERMS:created : Date of creation of the resource. DCTERMS:issued Date of formal issuance (e.g., publication) of the resource. PROV: Generation is the completion of production of a new entity by an activity. This entity did not exist before generation and becomes available for usage after this generation. PAV: The date this resource was authored. PAV: The date this resource was contributed to. PAV: The date of creation of the resource representation. DOAP: Date when something was created, in YYYY-MM-DD form. e.g. 2004-04-05. SCHEMA: The date on which the CreativeWork was created or the item was added to a DataFeed. DOAP: Date when something was created, in YYYY-MM-DD form. e.g. 2004-04-05."@en ;
                    rdfs:isDefinedBy        <http://purl.org/dc/terms/> ;
                    dcterms:issued          "2000-07-11"^^xsd:date ; 
                    dcterms:relation        omv:creationDate ,
                                            dcterms:issued ,
                                            pav:authoredOn ,
                                            pav:contributedOn ,
                                            pav:createdOn ,
                                            schema:dateCreated ,
                                            doap:created ,
                                            oboinowl:date ,
                                            oboinowl:hasDate ,
                                            prov:generatedAtTime ,
                                            <http://www.isibang.ac.in/ns/mod/1.1/creationDate> ;
                    pav:derivedFrom         <http://www.isibang.ac.in/ns/mod/1.2> ;
                    pav:importedOn          "2017-07-06"^^xsd:dateTime ;
                    
            #OPTIONAL STATEMENTS
                    prov:wasInfluencedBy    "FAIR principle: F2" .
            


### http://purl.org/dc/terms/modified
dcterms:modified    rdf:type                rdf:Property ; 
                    rdfs:subPropertyOf      dc:date , dcterms:date ;
                    rdfs:label              "modification date"@en ,
                                            "date de modification"@fr ;
                    rdfs:range              rdfs:Literal ; 
                    dcterms:description     "OMV: Date of the last modification made to the ontology. DCTERMS:Date on which the resource was changed. PAV: The date of the last update of the resource. An update is a change which did not warrant making a new resource related using pav:previousVersion, for instance correcting a spelling mistake. SCHEMA: The date on which the CreativeWork was most recently modified or when the item's entry was modified within a DataFeed."@en ;
                    rdfs:isDefinedBy        <http://purl.org/dc/terms/> ;
                    dcterms:issued          "2000-07-11"^^xsd:date ; 
                    dcterms:relation        omv:modificationDate ,
                                            schema:dateModified ,
                                            pav:lastUpdateOn ,
                                            <http://www.isibang.ac.in/ns/mod/1.1/creationDate> ;
                    pav:derivedFrom         <http://www.isibang.ac.in/ns/mod/1.2> ;
                    pav:importedOn          "2017-07-06"^^xsd:dateTime ;
                    
            #OPTIONAL STATEMENTS
                    prov:wasInfluencedBy    "FAIR principle: F2" .
            


### http://purl.org/dc/terms/valid
dcterms:valid       rdf:type                rdf:Property ; 
                    rdfs:subPropertyOf      dc:date , dcterms:date ;
                    rdfs:label              "validity date"@en ,
                                            "date de validité"@fr ;
                    rdfs:range              rdfs:Literal ; 
                    dcterms:description     "DCTERMS: Date (often a range) of validity of a resource. PROV: Invalidation is the start of the destruction, cessation, or expiry of an existing entity by an activity. The entity is no longer available for use (or further invalidation) after invalidation. Any generation or usage of an entity precedes its invalidation. SCHEMA: The end date and time of the item (in ISO 8601 date format)."@en ;
                    rdfs:isDefinedBy        <http://purl.org/dc/terms/> ;
                    dcterms:issued          "2000-07-11"^^xsd:date ; 
                    dcterms:relation        schema:endDate ,
                                            prov:invalidatedAtTime ;
                    pav:derivedFrom         <http://www.isibang.ac.in/ns/mod/1.2> ;
                    pav:importedOn          "2017-07-06"^^xsd:dateTime ;
                    
            #OPTIONAL STATEMENTS
                    prov:wasInfluencedBy    "FAIR principle: F2" .     

         

### http://purl.org/dc/terms/dateSubmitted
dcterms:dateSubmitted
                    rdf:type                rdf:Property ; 
                    rdfs:subPropertyOf      dc:date , dcterms:date ;
                    rdfs:label              "date submitted"@en ,
                                            "date de soumission"@fr ;
                    rdfs:range              rdfs:Literal ; 
                    dcterms:description     "DCTERMS: Date of submission of the resource. SCHEMA: Date of first broadcast/publication."@en ;
                    rdfs:isDefinedBy        <http://purl.org/dc/terms/> ;
                    dcterms:issued          "2002-07-13"^^xsd:date ; 
                    dcterms:relation        schema:datePublished ;
                    pav:derivedFrom         <http://www.isibang.ac.in/ns/mod/1.2> ;
                    pav:importedOn          "2017-07-06"^^xsd:dateTime ;
                    
            #OPTIONAL STATEMENTS
                    prov:wasInfluencedBy    "FAIR principle: F2" .     



### http://purl.org/pav/curatedOn
mod:curatedOn       rdf:type                owl:DatatypeProperty ;
                    rdfs:subPropertyOf      pav:contributedOn ;
                    rdfs:label              "curation date"@en ,
                                            "date de contrôle de qualité"@fr ;
                    rdfs:range              xsd:dateTime ;
                    dcterms:description     ""@en ;
                    rdfs:isDefinedBy        <http://purl.org/pav/> ;
                    dcterms:issued          "2014-08-28"^^xsd:date ;
                    pav:derivedFrom         <http://www.isibang.ac.in/ns/mod/1.2> ;
                    pav:importedOn          "2017-07-06"^^xsd:dateTime ;
            
            #OPTIONAL STATEMENTS
                    prov:wasInfluencedBy    "FAIR principle: F2" ;

            #OTHER ORIGINAL STATEMENTS IF ANY 
                    rdfs:seeAlso            pav:curatedBy .

             

##########################################
########## Metrics properties ##########
##########################################

### https://w3id.org/mod#metrics
mod:metrics         rdf:type                owl:DatatypeProperty ;
                    rdfs:label              "metrics"@en ,
                                            "métriques"@fr ;
                    rdfs:domain             mod:SemanticArtefactDistribution ;
                    dcterms:description     "MOD: A generic property to store any metrics related to the ontology."@en ;
                    rdfs:isDefinedBy        <https://w3id.org/mod> ;
                    dcterms:issued          "2018-08-02"^^xsd:date ;
                    pav:derivedFrom         <http://www.isibang.ac.in/ns/mod/1.4> ;
                    pav:importedOn          "2018-08-02"^^xsd:dateTime ;
                    
            #OPTIONAL STATEMENTS
                    prov:wasInfluencedBy    "MIRO guidelines: E.3" ,
                                            "FAIR principle: F2" .



###  https://w3id.org/mod#numberOfClasses
mod:numberOfClasses rdf:type                owl:DatatypeProperty ;
                    rdfs:subPropertyOf      mod:metrics ;
                    rdfs:label              "number of classes"@en ,
                                            "nombre de classes"@fr ;
                    rdfs:range              xsd:nonNegativeInteger ;
                    dcterms:description     "MOD: The total number of classes in an ontology. OMV: Number of classes in the ontology. VOAF: The number of classes defined in the vocabulary namespace. Classes imported from other namespaces are not taken into account. VOID: The total number of distinct classes in a void:Dataset. In other words, the number of distinct resources occuring as objects of rdf:type."@en ;
                    rdfs:isDefinedBy        <http://omv.ontoware.org/2005/05/ontology> ;
                    dcterms:issued          "2009-12-24"^^xsd:date ;
                    dcterms:relation        omv:numberOfClasses ,
                                            voaf:classNumber ,
                                            void:classes ,
                                            <http://www.isibang.ac.in/ns/mod/1.0/noOfClasses> ;
                    pav:derivedFrom         <http://www.isibang.ac.in/ns/mod/1.0> ;
                    pav:importedOn          "2015-08-05"^^xsd:dateTime ;
            
            #OPTIONAL STATEMENTS
                    skos:historyNote        "This property has been adopted from OMV Ontology Metadata Vocabulary and redefined in the MOD namespace."@en ;
                    prov:wasInfluencedBy    "MIRO guidelines:  E.3" ,
                                            "FAIR principle: F2" .
        


###  https://w3id.org/mod#numberOfIndividuals
mod:numberOfIndividuals
                    rdf:type                owl:DatatypeProperty ;
                    rdfs:subPropertyOf      mod:metrics ;
                    rdfs:label              "number of individuals"@en ,
                                            "nombre d'individus"@fr ;
                    rdfs:range              xsd:nonNegativeInteger ;
                    dcterms:description     "MOD: The total number of individuals in an ontology. OMV: Number of individuals in the ontology. VOID: The total number of entities that are described in a void:Dataset."@en ;
                    rdfs:isDefinedBy        <http://omv.ontoware.org/2005/05/ontology> ;
                    dcterms:issued          "2009-12-24"^^xsd:date ;
                    dcterms:relation        omv:numberOfIndividuals ,
                                            void:entities ,
                                            <http://www.isibang.ac.in/ns/mod/1.0/noOfIndividuals> ;
                    pav:derivedFrom         <http://www.isibang.ac.in/ns/mod/1.0> ;
                    pav:importedOn          "2015-08-05"^^xsd:dateTime ;
            
            #OPTIONAL STATEMENTS
                    skos:historyNote        "This property has been adopted from OMV Ontology Metadata Vocabulary and redefined in the MOD namespace."@en ;
                    prov:wasInfluencedBy    "MIRO guidelines:  E.3" ,
                                            "FAIR principle: F2" .



###  https://w3id.org/mod#numberOfProperties
mod:numberOfProperties
                    rdf:type                owl:DatatypeProperty ;
                    rdfs:subPropertyOf      mod:metrics ;
                    rdfs:label              "number of properties"@en ,
                                            "nombre de propriétés"@fr ;
                    rdfs:range              xsd:nonNegativeInteger ;
                    dcterms:description     "MOD: The total number of properties in an ontology. OMV: Number of properties in the ontology. VOAF: The number of properties defined in the vocabulary namespace. Properties imported from other namespaces are not taken into account. VOID: The total number of distinct properties in a void:Dataset. In other words, the number of distinct resources that occur in the predicate position of triples in the dataset."@en ;
                    rdfs:isDefinedBy        <http://omv.ontoware.org/2005/05/ontology> ;
                    dcterms:issued          "2009-12-24"^^xsd:date ;
                    dcterms:relation        omv:numberOfProperties ,
                                            voaf:propertyNumber ,
                                            void:properties ,
                                            <http://www.isibang.ac.in/ns/mod/1.0/noOfProperties> ;
                    pav:derivedFrom         <http://www.isibang.ac.in/ns/mod/1.0> ;
                    pav:importedOn          "2015-08-05"^^xsd:dateTime ;
            
            #OPTIONAL STATEMENTS
                    skos:historyNote        "This property has been adopted from OMV Ontology Metadata Vocabulary and redefined in the MOD namespace."@en ;
                    prov:wasInfluencedBy    "MIRO guidelines:  E.3" ,
                                            "FAIR principle: F2" .



###  https://w3id.org/mod#numberOfObjectProperties
mod:numberOfObjectProperties
                    rdf:type                owl:DatatypeProperty ;
                    rdfs:subPropertyOf      mod:numberOfProperties ;
                    rdfs:label              "number of object properties"@en ,
                                            "nombre de propriétés d'objet"@fr ;
                    rdfs:range              xsd:nonNegativeInteger ;
                    dcterms:description     "MOD: The total number of object properties in an ontology."@en ;
                    rdfs:isDefinedBy        <https://w3id.org/mod> ;
                    dcterms:issued          "2017-07-06"^^xsd:date ;
                    pav:derivedFrom         <http://www.isibang.ac.in/ns/mod/1.2> ;
                    pav:importedOn          "2017-07-06"^^xsd:dateTime ;
            
            #OPTIONAL STATEMENTS
                    prov:wasInfluencedBy    "MIRO guidelines:  E.3" ,
                                            "FAIR principle: F2" .



###  https://w3id.org/mod#numberOfDataProperties
mod:numberOfDataProperties
                    rdf:type                owl:DatatypeProperty ;
                    rdfs:subPropertyOf      mod:numberOfProperties ;
                    rdfs:label              "number of data properties"@en ,
                                            "nombre de propriétés de données"@fr ;
                    rdfs:range              xsd:nonNegativeInteger ;
                    dcterms:description     "MOD: The total number of data properties in an ontology."@en ;
                    rdfs:isDefinedBy        <https://w3id.org/mod> ;
                    dcterms:issued          "2017-07-06"^^xsd:date ;
                    pav:derivedFrom         <http://www.isibang.ac.in/ns/mod/1.2> ;
                    pav:importedOn          "2017-07-06"^^xsd:dateTime ;
            
            #OPTIONAL STATEMENTS
                    prov:wasInfluencedBy    "MIRO guidelines:  E.3" ,
                                            "FAIR principle: F2" .



###  https://w3id.org/mod#numberOfAxioms
mod:numberOfAxioms
                    rdf:type                owl:DatatypeProperty ;
                    rdfs:subPropertyOf      mod:metrics ;
                    rdfs:label              "number of axioms or triples"@en ,
                                            "nombre d'axiomes ou de triples"@fr ;
                    rdfs:range              xsd:nonNegativeInteger ;
                    dcterms:description     "MOD: The total number of axioms in an ontology. OMV: Number of axioms in the ontology."@en ;
                    rdfs:isDefinedBy        <http://omv.ontoware.org/2005/05/ontology> ;
                    dcterms:issued          "2009-12-24"^^xsd:date ;
                    dcterms:relation        omv:numberOfAxioms ,
                                            <http://www.isibang.ac.in/ns/mod/1.0/noOfAxioms> ;
                    pav:derivedFrom         <http://www.isibang.ac.in/ns/mod/1.0> ;
                    pav:importedOn          "2015-08-05"^^xsd:dateTime ;
            
            #OPTIONAL STATEMENTS
                    skos:historyNote        "This property has been adopted from OMV Ontology Metadata Vocabulary and redefined in the MOD namespace."@en ;
                    prov:wasInfluencedBy    "MIRO guidelines:  E.3" ,
                                            "FAIR principle: F2" .



###  https://w3id.org/mod#numberOfLabels
mod:numberOfLabels
                    rdf:type                owl:DatatypeProperty ;
                    rdfs:subPropertyOf      mod:metrics ;
                    rdfs:label              "number of data properties"@en ,
                                            "nombre de propriétés de données"@fr ;
                    rdfs:range              xsd:nonNegativeInteger ;
                    dcterms:description     "MOD: Number of defined labels for any resources in an ontology (classes, properties, etc)."@en ;
                    rdfs:isDefinedBy        <https://w3id.org/mod> ;
                    dcterms:issued          "2017-07-06"^^xsd:date ;
                    pav:derivedFrom         <http://www.isibang.ac.in/ns/mod/1.2> ;
                    pav:importedOn          "2017-07-06"^^xsd:dateTime ;
            
            #OPTIONAL STATEMENTS
                    prov:wasInfluencedBy    "MIRO guidelines:  E.3" ,
                                            "FAIR principle: F2" .



### http://www.w3.org/ns/dcat#byteSize
dcat:byteSize       rdf:type                rdf:Property , owl:DatatypeProperty ;
                    rdfs:label              "byte size"@en ,
                                            "taille en octets"@fr ;
                    rdfs:domain             dcat:Distribution ;
                    rdfs:range              rdfs:Literal ;
                    dcterms:description     "DCAT: The size of a distribution in bytes. MOD: The byte size of an ontology."@en ;
                    rdfs:isDefinedBy        <http://www.w3.org/TR/vocab-dcat/> ;
                    dcterms:issued          "2014-01-16"^^xsd:date ;
                    dcterms:relation        <http://www.isibang.ac.in/ns/mod/1.0/size> ,
                                            <http://www.isibang.ac.in/ns/mod/1.0/byteSize> ;
                    pav:derivedFrom         <http://www.isibang.ac.in/ns/mod/1.0> ;
                    pav:importedOn          "2015-08-05"^^xsd:dateTime ;
                    
            #OPTIONAL STATEMENTS
                    prov:wasInfluencedBy    "MIRO guidelines: E.3" ,
                                            "FAIR principle: F2" ;
            
            #OTHER ORIGINAL STATEMENTS IF ANY 
                    skos:scopeNote          "The size in bytes can be approximated when the precise size is not known. The literal value of dcat:byteSize should by typed as xsd:decimal."@en .



###  https://w3id.org/mod#maxDepth
mod:maxDepth        rdf:type                owl:DatatypeProperty ;
                    rdfs:subPropertyOf      mod:metrics ;
                    rdfs:label              "maximum depth of the hierachy"@en ,
                                            "profondeur maximum de la hierachie"@fr ;
                    rdfs:range              xsd:nonNegativeInteger ;
                    dcterms:description     "MOD: Maximum depth of the hierarchy tree (BioPortal definition)."@en ;
                    rdfs:isDefinedBy        <https://w3id.org/mod> ;
                    dcterms:issued          "2017-07-06"^^xsd:date ;
                    pav:derivedFrom         <http://www.isibang.ac.in/ns/mod/1.4> ;
                    pav:importedOn          "2018-08-02"^^xsd:dateTime ;
            
            #OPTIONAL STATEMENTS
                    prov:wasInfluencedBy    "FAIR principle: R1" .


###  https://w3id.org/mod#maxChildCount
mod:maxDepth        rdf:type                owl:DatatypeProperty ;
                    rdfs:subPropertyOf      mod:metrics ;
                    rdfs:label              "maximum number of children per class"@en ,
                                            "nombre maximum d'enfant par classe"@fr ;
                    rdfs:range              xsd:nonNegativeInteger ;
                    dcterms:description     "MOD: Maximum number of children per class (BioPortal definition)."@en ;
                    rdfs:isDefinedBy        <https://w3id.org/mod> ;
                    dcterms:issued          "2017-07-06"^^xsd:date ;
                    pav:derivedFrom         <http://www.isibang.ac.in/ns/mod/1.4> ;
                    pav:importedOn          "2018-08-02"^^xsd:dateTime ;
            
            #OPTIONAL STATEMENTS
                    prov:wasInfluencedBy    "FAIR principle: R1" .



###  https://w3id.org/mod#averageChildCount
mod:maxDepth        rdf:type                owl:DatatypeProperty ;
                    rdfs:subPropertyOf      mod:metrics ;
                    rdfs:label              "average number of children per class"@en ,
                                            "nombre moyen d'enfant par classe"@fr ;
                    rdfs:range              xsd:nonNegativeInteger ;
                    dcterms:description     "MOD: Average number of children per class (BioPortal definition)."@en ;
                    rdfs:isDefinedBy        <https://w3id.org/mod> ;
                    dcterms:issued          "2017-07-06"^^xsd:date ;
                    pav:derivedFrom         <http://www.isibang.ac.in/ns/mod/1.4> ;
                    pav:importedOn          "2018-08-02"^^xsd:dateTime ;
            
            #OPTIONAL STATEMENTS
                    prov:wasInfluencedBy    "FAIR principle: R1" .



###  https://w3id.org/mod#classesWithOneChild
mod:maxDepth        rdf:type                owl:DatatypeProperty ;
                    rdfs:subPropertyOf      mod:metrics ;
                    rdfs:label              "number of classes with a single child"@en ,
                                            "nombre de classes avec un seul enfant"@fr ;
                    rdfs:range              xsd:nonNegativeInteger ;
                    dcterms:description     "MOD: Number of classes that have only one subclass in the is-a hierarchy (BioPortal definition)."@en ;
                    rdfs:isDefinedBy        <https://w3id.org/mod> ;
                    dcterms:issued          "2017-07-06"^^xsd:date ;
                    pav:derivedFrom         <http://www.isibang.ac.in/ns/mod/1.4> ;
                    pav:importedOn          "2018-08-02"^^xsd:dateTime ;
            
            #OPTIONAL STATEMENTS
                    prov:wasInfluencedBy    "FAIR principle: R1" .



###  https://w3id.org/mod#classesWithMoreThan25Children
mod:maxDepth        rdf:type                owl:DatatypeProperty ;
                    rdfs:subPropertyOf      mod:metrics ;
                    rdfs:label              "number of classes with more than 25 children"@en ,
                                            "nombre de classes avec plus de 25 enfants"@fr ;
                    rdfs:range              xsd:nonNegativeInteger ;
                    dcterms:description     "MOD: Number of classes that have more than 25 direct subclasses (BioPortal definition)."@en ;
                    rdfs:isDefinedBy        <https://w3id.org/mod> ;
                    dcterms:issued          "2017-07-06"^^xsd:date ;
                    pav:derivedFrom         <http://www.isibang.ac.in/ns/mod/1.4> ;
                    pav:importedOn          "2018-08-02"^^xsd:dateTime ;
            
            #OPTIONAL STATEMENTS
                    prov:wasInfluencedBy    "FAIR principle: R1" .



###  https://w3id.org/mod#classesWithNoDefinition
mod:maxDepth        rdf:type                owl:DatatypeProperty ;
                    rdfs:subPropertyOf      mod:metrics ;
                    rdfs:label              "number of classes with no definition"@en ,
                                            "nombre de classes sans définition"@fr ;
                    rdfs:range              xsd:nonNegativeInteger ;
                    dcterms:description     "MOD: Number of classes that have no value for the definition property (BioPortal definition). For ontologies in OBO and RRF formats, the property for definition is part of the language. For OWL ontologies, the authors specify this property as part of the ontology metadata (the default is skos:definition)."@en ;
                    rdfs:isDefinedBy        <https://w3id.org/mod> ;
                    dcterms:issued          "2017-07-06"^^xsd:date ;
                    pav:derivedFrom         <http://www.isibang.ac.in/ns/mod/1.4> ;
                    pav:importedOn          "2018-08-02"^^xsd:dateTime ;
            
            #OPTIONAL STATEMENTS
                    prov:wasInfluencedBy    "FAIR principle: R1" .



##########################################
########## Provenance properties ##########
##########################################

## http://purl.org/dc/terms/source
dcterms:source      rdf:type                rdf:Property ;
                    rdfs:subPropertyOf      dc:source , dcterms:relation ;
                    rdfs:label             "source"@en ,
                                            "source"@fr ;
                    dcterms:description     "DCTERMS: A related resource from which the described resource is derived. MOD: The ontology(ies) referred to while creating the present ontology. PROV: Influence is the capacity of an entity, activity, or agent to have an effect on the character, development, or behavior of another by means of usage, start, end, generation, invalidation, communication, derivation, attribution, association, or delegation. PROV: A derivation is a transformation of an entity into another, an update of an entity resulting in a new one, or the construction of a new entity based on a pre-existing entity. PAV: Derived from a different resource. NKOS: A resource used as the source for a derivative resource."@en ;
                    rdfs:isDefinedBy        <http://purl.org/dc/terms/> ;
                    dcterms:issued          "2008-01-14"^^xsd:date ;
                    dcterms:relation        schema:isBasedOn ,
                                            nkos:basedOn ,
                                            prov:wasDerivedFrom , 
                                            prov:wasInfluencedBy ,
                                            pav:derivedFrom ,
                                            <http://www.isibang.ac.in/ns/mod/1.0/sourceOntology> ;
                    pav:derivedFrom         <http://www.isibang.ac.in/ns/mod/1.0> ;
                    pav:importedOn          "2015-08-05"^^xsd:dateTime ;
                    
            #OPTIONAL STATEMENTS
                    prov:wasInfluencedBy    "MIRO guidelines: D.2" ,
                                            "FAIR principle: R1.2" .



### http://www.w3.org/ns/prov#wasGeneratedBy
prov:wasGeneratedBy rdf:type                owl:ObjectProperty ;
                    rdfs:subPropertyOf      prov:wasInfluencedBy ;
                    rdfs:label              "was generated by"@en ,
                                            "a été généré par"@fr ;
                    rdfs:domain             prov:Entity ;
                    rdfs:range              prov:Activity ;
                    dcterms:description     "PROV: Generation is the completion of production of a new entity by an activity. This entity did not exist before generation and becomes available for usage after this generation."@en ;
                    rdfs:isDefinedBy        <http://www.w3.org/ns/prov-o#> ;
                    dcterms:issued          "2013-04-30"^^xsd:date ;
                    pav:derivedFrom         <http://www.isibang.ac.in/ns/mod/1.2> ;
                    pav:importedOn          "2017-07-06"^^xsd:dateTime ;
                    
            #OPTIONAL STATEMENTS
                    prov:wasInfluencedBy    "MIRO guidelines: D.1" ,
                                            "FAIR principle: R1.2" ;
            
            #OTHER ORIGINAL STATEMENTS IF ANY 
                    prov:inverse            prov:generated .



### http://www.w3.org/ns/prov#wasinvalidatedBy
prov:wasinvalidatedBy
                    rdf:type                owl:ObjectProperty ;
                    rdfs:subPropertyOf      prov:wasInfluencedBy ;
                    rdfs:label              "was invalidated by"@en ,
                                            "a été invalidé par"@fr ;
                    rdfs:domain             prov:Entity ;
                    rdfs:range              prov:Activity ;
                    dcterms:description     "PROV: Invalidation is the start of the destruction, cessation, or expiry of an existing entity by an activity. The entity is no longer available for use (or further invalidation) after invalidation. Any generation or usage of an entity precedes its invalidation."@en ;
                    rdfs:isDefinedBy        <http://www.w3.org/ns/prov-o#> ;
                    dcterms:issued          "2013-04-30"^^xsd:date ;
                    pav:derivedFrom         <http://www.isibang.ac.in/ns/mod/1.2> ;
                    pav:importedOn          "2017-07-06"^^xsd:dateTime ;
                    
            #OPTIONAL STATEMENTS
                    prov:wasInfluencedBy    "FAIR principle: R1.2" ;
            
            #OTHER ORIGINAL STATEMENTS IF ANY 
                    prov:inverse            prov:invalidated .
                  


### http://purl.org/dc/terms/accrualMethod
dcterms:accrualMethod
                    rdf:type                rdf:Property ;
                    rdfs:label              "accrual method"@en ,
                                            "méthode d'ajout"@fr ;
                    rdfs:domain             <http://purl.org/dc/dcmitype/Collection> ;
                    dcterms:description     "DCTERMS: The method by which items are added to a collection. Recommended practice is to use a value from the Collection Description Accrual Method Vocabulary."@en ;
                    rdfs:isDefinedBy        <http://purl.org/dc/terms/> ;
                    dcterms:issued          "2005-06-13"^^xsd:date ;
                    pav:derivedFrom         <http://www.isibang.ac.in/ns/mod/1.2> ;
                    pav:importedOn          "2017-07-06"^^xsd:dateTime ;
                    
            #OPTIONAL STATEMENTS
                    prov:wasInfluencedBy    "MIRO guidelines: D.3, F.2" ,
                                            "FAIR principle: R1.2" ;
            
            #OTHER ORIGINAL STATEMENTS IF ANY 
                    <http://purl.org/dc/dcam/rangeIncludes>     dcterms:MethodOfAccrual .



### http://purl.org/dc/terms/accrualPeriodicity
dcterms:accrualPeriodicity
                    rdf:type                rdf:Property ;
                    rdfs:label              "accrual periodicity"@en ,
                                            "fréquence des ajouts"@fr ;
                    rdfs:domain             <http://purl.org/dc/dcmitype/Collection> ;
                    dcterms:description     "DCTERMS: The frequency with which items are added to a collection. Recommended practice is to use a value from the Collection Description Frequency Vocabulary."@en ;
                    rdfs:isDefinedBy        <http://purl.org/dc/terms/> ;
                    dcterms:issued          "2005-06-13"^^xsd:date ;
                    pav:derivedFrom         <http://www.isibang.ac.in/ns/mod/1.2> ;
                    pav:importedOn          "2017-07-06"^^xsd:dateTime ;
                    
            #OPTIONAL STATEMENTS
                    prov:wasInfluencedBy    "MIRO guidelines: F.2" ,
                                            "FAIR principle: R1.2" ;
            
            #OTHER ORIGINAL STATEMENTS IF ANY 
                    <http://purl.org/dc/dcam/rangeIncludes>     dcterms:Frequency .
                  
    

### http://purl.org/dc/terms/accrualPolicy
dcterms:accrualPolicy
                    rdf:type                rdf:Property ;
                    rdfs:label              "accrual policy"@en ,
                                            "politique des ajouts"@fr ;
                    rdfs:domain             <http://purl.org/dc/dcmitype/Collection> ;
                    dcterms:description     "DCTERMS: The policy governing the addition of items to a collection. Recommended practice is to use a value from the Collection Description Accrual Policy Vocabulary."@en ;
                    rdfs:isDefinedBy        <http://purl.org/dc/terms/> ;
                    dcterms:issued          "2005-06-13"^^xsd:date ;
                    pav:derivedFrom         <http://www.isibang.ac.in/ns/mod/1.2> ;
                    pav:importedOn          "2017-07-06"^^xsd:dateTime ;
                    
            #OPTIONAL STATEMENTS
                    prov:wasInfluencedBy    "MIRO guidelines: F.2, F.3" ,
                                            "FAIR principle: R1.2" ;
            
            #OTHER ORIGINAL STATEMENTS IF ANY 
                    <http://purl.org/dc/dcam/rangeIncludes>     dcterms:Policy .
        

############################################################################################# 
############################################################################################# 
#################################################################
#   END OF MOD2 profile PROPERTIES
#################################################################
############################################################################################# 
############################################################################################# 







