<?xml version="1.0" encoding="UTF-8"?>
<?xml-stylesheet href="view_vocabulary.xsl" type="text/xsl"?>

<rdf:RDF
    xmlns:rdf="http://www.w3.org/1999/02/22-rdf-syntax-ns#"
    xmlns="http://identifiers.org/idot#"
    xmlns:owl="http://www.w3.org/2002/07/owl#"
    xmlns:xsd="http://www.w3.org/2001/XMLSchema#"
    xmlns:rdfs="http://www.w3.org/2000/01/rdf-schema#"
  xml:base="http://identifiers.org/idot">
  <owl:Ontology rdf:about=".">
    <rdfs:label>Identifiers.org Terms</rdfs:label>
    <rdfs:comment>Identifiers.org Terms (idot) is an RDF vocabulary providing useful terms for describing datasets. To reference those terms, please use URIs of the form: http://identifiers.org/idot/[term].</rdfs:comment>
    <owl:versionInfo>2014-03-04</owl:versionInfo>
    <owl:imports rdf:resource="http://purl.org/dc/dcmitype/"/>
  </owl:Ontology>
  <rdfs:Class rdf:ID="AccessPattern">
    <rdfs:subClassOf rdf:resource="http://www.w3.org/2000/01/rdf-schema#Class"/>
    <rdfs:comment>May be used to specify how to access specific formats provided by a given resource.</rdfs:comment>
  </rdfs:Class>
  <rdf:Property rdf:ID="accessPattern">
    <rdfs:range rdf:resource="#AccessPattern"/>
    <rdfs:domain rdf:resource="http://purl.org/dc/dcmitype/Dataset"/>
    <rdfs:label>accessPattern</rdfs:label>
    <rdfs:comment>Specifies how to access specific formats of the resources.</rdfs:comment>
  </rdf:Property>
  <rdf:Property rdf:ID="alternatePrefix">
    <rdfs:domain rdf:resource="http://purl.org/dc/dcmitype/Dataset"/>
    <rdfs:range rdf:resource="http://www.w3.org/2001/XMLSchema#string"/>
    <rdfs:label>alternatePrefix</rdfs:label>
    <rdfs:comment>A short label that is used by some communities to refer to a dataset (see 'preferredPrefix').</rdfs:comment>
  </rdf:Property>
  <rdf:Property rdf:ID="exampleIdentifier">
    <rdfs:domain rdf:resource="http://purl.org/dc/dcmitype/Dataset"/>
    <rdfs:range rdf:resource="http://www.w3.org/2001/XMLSchema#string"/>
    <rdfs:label>exampleIdentifier</rdfs:label>
    <rdfs:comment>An example identifier used by one item (or record) from a dataset.</rdfs:comment>
  </rdf:Property>
  <rdf:Property rdf:ID="identifierPattern">
    <rdfs:domain rdf:resource="http://purl.org/dc/dcmitype/Dataset"/>
    <rdfs:range rdf:resource="http://www.w3.org/2001/XMLSchema#string"/>
    <rdfs:label>identifierPattern</rdfs:label>
    <rdfs:comment>Regular expression describing alphanumeric strings used to identify items (or records) in a dataset.</rdfs:comment>
  </rdf:Property>
  <rdf:Property rdf:ID="obsolete">
    <rdfs:domain rdf:resource="http://purl.org/dc/dcmitype/Dataset"/>
    <rdfs:range rdf:resource="http://www.w3.org/2001/XMLSchema#string"/>
    <rdfs:label>obsolete</rdfs:label>
    <rdfs:comment>Indicates if the current dataset is obsolete (not provided any more to the public community). Value can either be 'true' or 'false' (xsd:boolean). The statement is usually omitted if 'false'.</rdfs:comment>
  </rdf:Property>
  <rdf:Property rdf:ID="preferredPrefix">
    <rdfs:domain rdf:resource="http://purl.org/dc/dcmitype/Dataset"/>
    <rdfs:range rdf:resource="http://www.w3.org/2001/XMLSchema#string"/>
    <rdfs:label>preferredPrefix</rdfs:label>
    <rdfs:comment>Short label that is commonly used to refer to the dataset. Often utilised to identify the dataset in IRIs for specific items (or records). This may also stand in place of the base IRI of the dataset (e.g. see http://prefix.cc).</rdfs:comment>
  </rdf:Property>
  <rdf:Property rdf:ID="primarySource">
    <rdfs:domain rdf:resource="#AccessPattern"/>
    <rdfs:range rdf:resource="http://www.w3.org/2001/XMLSchema#boolean"/>
    <rdfs:label>primarySource</rdfs:label>
    <rdfs:comment>Indicates the primary (or official)    TO COMPLETE   source for the dataset. Value can either be 'true' or 'false' (xsd:boolean). The statement is usually omitted if 'false'.</rdfs:comment>
  </rdf:Property>
  <rdf:Property rdf:ID="reliability">
    <rdfs:domain rdf:resource="#AccessPattern"/>
    <rdfs:range rdf:resource="http://www.w3.org/2001/XMLSchema#string"/>
    <rdfs:label>reliability</rdfs:label>
    <rdfs:comment>Reliability of a resource (physical location providing access to data or information about the identified entity). This is a number (xsd:decimal) which represents a percentage of uptime.</rdfs:comment>
  </rdf:Property>
  <rdf:Property rdf:ID="state">
    <rdfs:domain rdf:resource="#AccessPattern"/>
    <rdfs:range rdf:resource="http://www.w3.org/2001/XMLSchema#string"/>
    <rdfs:label>state</rdfs:label>
    <rdfs:comment>State of a resource (physical location providing access to data or information about the identified entity). This is should be based on a recent manual or automatic check of the resource. Possible values are: 'up', 'down', 'probably up', 'obsolete resource', 'restricted access' and 'unknown'.</rdfs:comment>
  </rdf:Property>
</rdf:RDF>

<!-- Created with TopBraid -->
